src/specs/VerifyQuotientEvaluation.ec
@@ -1,3 +1,5 @@
+require import AllCore.
+require import IntDiv.
 require        Constants.
 require import EvaluateLagrangePolyOutOfDomain.
 require import LookupQuotientContribution.
@@ -53,6 +55,107 @@ module VerifyQuotientEvaluation = {
       RevertWithMessage.low(W256.of_int 27, W256.of_int STRING);
     }
   }
+
+  proc mid (
+      stateAlpha
+      stateBeta
+      stateBetaLookup
+      stateGamma
+      stateGammaLookup
+      stateZ
+      proofPublicInput
+      proofCopyPermutationPolys0OpeningAtZ
+      proofCopyPermutationPolys1OpeningAtZ
+      proofCopyPermutationPolys2OpeningAtZ
+      proofStatePolys0OpeningAtZ
+      proofStatePolys1OpeningAtZ
+      proofStatePolys2OpeningAtZ
+      proofStatePolys3OpeningAtZ
+      proofLookupSPolyOpeningAtZOmega
+      proofLookupGrandProductOpeningAtZOmega
+      proofGateSelectors0OpeningAtZ
+      proofLinearisationPolyOpeningAtZ
+      proofCopyPermutationGrandProductOpeningAtZOmega
+      stateZInDomainSize
+      proofQuotientPolyOpeningAtZ : int) :
+  (bool option * int * int * int * int * int * int * int * int * int * int * int * int) = {
+    var r, elpodL0, elpodLn, stateT, pgsT, pqc, pqcR, lqc, lqcR, plpo, vanishing, lhs;
+    var statePowerOfAlpha2, statePowerOfAlpha3, statePowerOfAlpha4, statePowerOfAlpha5,
+        statePowerOfAlpha6, statePowerOfAlpha7, statePowerOfAlpha8 : int;
+    var stateL0AtZ, stateLnMinusOneAtZ, stateBetaPlusOne,
+        stateBetaGammaPlusGamma, stateZMinusLastOmega : int;
+
+    statePowerOfAlpha2 <- stateAlpha^2 %% Constants.R;
+    statePowerOfAlpha3 <- stateAlpha^3 %% Constants.R;
+    statePowerOfAlpha4 <- stateAlpha^4 %% Constants.R;
+    statePowerOfAlpha5 <- stateAlpha^5 %% Constants.R;
+    statePowerOfAlpha6 <- stateAlpha^6 %% Constants.R;
+    statePowerOfAlpha7 <- stateAlpha^7 %% Constants.R;
+    statePowerOfAlpha8 <- stateAlpha^8 %% Constants.R;
+
+    elpodL0 <@ EvaluateLagrangePolyOutOfDomain.mid(0, stateZ);
+    
+    if (elpodL0 = None) {
+      r <- None;
+    } else {
+      stateL0AtZ <- oget(elpodL0);
+      elpodLn <@ EvaluateLagrangePolyOutOfDomain.mid((Constants.DOMAIN_SIZE - 1), stateZ);
+
+      (* Since the fist one didn't failed neither the second will *)
+      stateLnMinusOneAtZ <- oget(elpodLn);
+      stateT <- (stateL0AtZ * proofPublicInput) %% Constants.R;
+      pgsT <- (stateT * proofGateSelectors0OpeningAtZ) %% Constants.R;
+      pqc <@ PermutationQuotientContribution.mid(
+                statePowerOfAlpha4,
+                statePowerOfAlpha5,
+                proofCopyPermutationGrandProductOpeningAtZOmega,
+                stateBeta,
+                stateGamma,
+                proofCopyPermutationPolys0OpeningAtZ,
+                proofCopyPermutationPolys1OpeningAtZ,
+                proofCopyPermutationPolys2OpeningAtZ,
+                proofStatePolys0OpeningAtZ,
+                proofStatePolys1OpeningAtZ,
+                proofStatePolys2OpeningAtZ,
+                proofStatePolys3OpeningAtZ,
+                stateL0AtZ);
+      pqcR <- (pgsT + pqc) %% Constants.R;  
+
+      (lqc, stateBetaPlusOne, stateBetaGammaPlusGamma, stateZMinusLastOmega) <@
+        LookupQuotientContribution.mid(
+           stateBetaLookup,
+           stateGammaLookup,
+           statePowerOfAlpha6,
+           statePowerOfAlpha7,
+           statePowerOfAlpha8,
+           proofLookupSPolyOpeningAtZOmega,
+           proofLookupGrandProductOpeningAtZOmega,
+           stateZ,
+           stateL0AtZ,
+           stateLnMinusOneAtZ);
+
+      lqcR <- (pqcR + lqc) %% Constants.R;
+      plpo <- (proofLinearisationPolyOpeningAtZ + lqcR) %% Constants.R;
+      vanishing <- (stateZInDomainSize + (Constants.R - 1)) %% Constants.R;
+      lhs <- (proofQuotientPolyOpeningAtZ * vanishing) %% Constants.R;
+      r <- Some (lhs = plpo);
+    }
+    
+    return (r,
+      statePowerOfAlpha2,
+      statePowerOfAlpha3,
+      statePowerOfAlpha4,
+      statePowerOfAlpha5,
+      statePowerOfAlpha6, 
+      statePowerOfAlpha7,
+      statePowerOfAlpha8,
+      stateL0AtZ,
+      stateLnMinusOneAtZ,
+      stateBetaPlusOne,
+      stateBetaGammaPlusGamma,
+      stateZMinusLastOmega
+    );
+  }
 }.
 
 lemma verifyQuotientEvaluation_extracted_equiv_low:
@@ -81,12 +184,2952 @@ lemma verifyQuotientEvaluation_extracted_equiv_low:
     skip.
     by progress.
   qed.
+  
+import MemoryMap PurePrimops.
 
+op verifyQuotientEvaluation_memory_footprint (m: mem)
+(a2 a3 a4 a5 a6 a7 a8 : uint256)
+(sl0az slnm1az : uint256)
+(bpo bgpg zmlo : uint256)
+(v1 v2 v3 v4 v5 v6 v7 v8 : uint256) =
+let m2 = store m  STATE_POWER_OF_ALPHA_2_SLOT a2 in
+let m3 = store m2 STATE_POWER_OF_ALPHA_3_SLOT a3 in
+let m4 = store m3 STATE_POWER_OF_ALPHA_4_SLOT a4 in
+let m5 = store m4 STATE_POWER_OF_ALPHA_5_SLOT a5 in
+let m6 = store m5 STATE_POWER_OF_ALPHA_6_SLOT a6 in
+let m7 = store m6 STATE_POWER_OF_ALPHA_7_SLOT a7 in
+let m8 = store m7 STATE_POWER_OF_ALPHA_8_SLOT a8 in
+let m9 = lagrange_memory_footprint m8 v1 v2 v3 in
+let m10 = store m9 STATE_L_0_AT_Z_SLOT sl0az in
+let m11 = lagrange_memory_footprint m10 v4 v5 v6 in
+let m12 = store m11 STATE_L_N_MINUS_ONE_AT_Z_SLOT slnm1az in
+let m13 = lookupQuotientContribution_memory_footprint m12 v7 bpo bgpg zmlo v8 in
+m13.
 
+lemma VerifyQuotientEvaluation_low_equiv_mid (m : mem) (
+      stateAlphaG
+      stateBetaG
+      stateBetaLookupG
+      stateGammaG
+      stateGammaLookupG
+      stateZG
+      proofPublicInputG
+      proofCopyPermutationPolys0OpeningAtZG
+      proofCopyPermutationPolys1OpeningAtZG
+      proofCopyPermutationPolys2OpeningAtZG
+      proofStatePolys0OpeningAtZG
+      proofStatePolys1OpeningAtZG
+      proofStatePolys2OpeningAtZG
+      proofStatePolys3OpeningAtZG
+      proofLookupSPolyOpeningAtZOmegaG
+      proofLookupGrandProductOpeningAtZOmegaG
+      proofGateSelectors0OpeningAtZG
+      proofLinearisationPolyOpeningAtZG
+      proofCopyPermutationGrandProductOpeningAtZOmegaG
+      stateZInDomainSizeG
+      proofQuotientPolyOpeningAtZG
+) :
+equiv [VerifyQuotientEvaluation.low ~ VerifyQuotientEvaluation.mid :
+arg{2} =
+  (stateAlphaG, stateBetaG, stateBetaLookupG, stateGammaG, stateGammaLookupG, stateZG,
+   proofPublicInputG, proofCopyPermutationPolys0OpeningAtZG,
+   proofCopyPermutationPolys1OpeningAtZG, proofCopyPermutationPolys2OpeningAtZG,
+   proofStatePolys0OpeningAtZG, proofStatePolys1OpeningAtZG,
+   proofStatePolys2OpeningAtZG, proofStatePolys3OpeningAtZG,
+   proofLookupSPolyOpeningAtZOmegaG, proofLookupGrandProductOpeningAtZOmegaG,
+   proofGateSelectors0OpeningAtZG, proofLinearisationPolyOpeningAtZG,
+   proofCopyPermutationGrandProductOpeningAtZOmegaG, stateZInDomainSizeG,
+   proofQuotientPolyOpeningAtZG) /\
+Primops.memory{1} = m /\
+!Primops.reverted{1} /\  
+W256.to_uint (mload m STATE_ALPHA_SLOT) = stateAlphaG /\
+W256.to_uint (mload m STATE_BETA_SLOT) = stateBetaG /\
+W256.to_uint (mload m STATE_BETA_LOOKUP_SLOT) = stateBetaLookupG /\
+W256.to_uint (mload m STATE_GAMMA_SLOT) = stateGammaG /\
+W256.to_uint (mload m STATE_GAMMA_LOOKUP_SLOT) = stateGammaLookupG /\
+W256.to_uint (mload m STATE_Z_SLOT) = stateZG /\
+W256.to_uint (mload m PROOF_PUBLIC_INPUT) = proofPublicInputG /\
+W256.to_uint (mload m PROOF_COPY_PERMUTATION_POLYS_0_OPENING_AT_Z_SLOT) = proofCopyPermutationPolys0OpeningAtZG /\
+W256.to_uint (mload m PROOF_COPY_PERMUTATION_POLYS_1_OPENING_AT_Z_SLOT) = proofCopyPermutationPolys1OpeningAtZG /\
+W256.to_uint (mload m PROOF_COPY_PERMUTATION_POLYS_2_OPENING_AT_Z_SLOT) = proofCopyPermutationPolys2OpeningAtZG /\
+W256.to_uint (mload m PROOF_STATE_POLYS_0_OPENING_AT_Z_SLOT) = proofStatePolys0OpeningAtZG /\
+W256.to_uint (mload m PROOF_STATE_POLYS_1_OPENING_AT_Z_SLOT) = proofStatePolys1OpeningAtZG /\
+W256.to_uint (mload m PROOF_STATE_POLYS_2_OPENING_AT_Z_SLOT) = proofStatePolys2OpeningAtZG /\
+W256.to_uint (mload m PROOF_STATE_POLYS_3_OPENING_AT_Z_SLOT) = proofStatePolys3OpeningAtZG /\
+W256.to_uint (mload m PROOF_LOOKUP_S_POLY_OPENING_AT_Z_OMEGA_SLOT) = proofLookupSPolyOpeningAtZOmegaG /\
+W256.to_uint (mload m PROOF_LOOKUP_GRAND_PRODUCT_OPENING_AT_Z_OMEGA_SLOT) = proofLookupGrandProductOpeningAtZOmegaG /\
+W256.to_uint (mload m PROOF_GATE_SELECTORS_0_OPENING_AT_Z_SLOT) = proofGateSelectors0OpeningAtZG /\
+W256.to_uint (mload m PROOF_LINEARISATION_POLY_OPENING_AT_Z_SLOT) = proofLinearisationPolyOpeningAtZG /\
+W256.to_uint (mload m PROOF_COPY_PERMUTATION_GRAND_PRODUCT_OPENING_AT_Z_OMEGA_SLOT) = proofCopyPermutationGrandProductOpeningAtZOmegaG /\
+W256.to_uint (mload m STATE_Z_IN_DOMAIN_SIZE) = stateZInDomainSizeG /\
+W256.to_uint (mload m PROOF_QUOTIENT_POLY_OPENING_AT_Z_SLOT) = proofQuotientPolyOpeningAtZG
+==>
+(Primops.reverted{1} /\
+  (((stateZG^Constants.DOMAIN_SIZE) - 1) %% Constants.R = 0 /\ res{2}.`1 = None)
+    \/
+   (((stateZG^Constants.DOMAIN_SIZE) - 1) %% Constants.R <> 0 /\ res{2}.`1 = Some false))
+\/
+(!Primops.reverted{1} /\
+  ((stateZG^Constants.DOMAIN_SIZE) - 1) %% Constants.R <> 0 /\
+  exists (v1 v2 v3 v4 v5 v6 v7 v8 : uint256),
+  Primops.memory{1} = verifyQuotientEvaluation_memory_footprint m 
+  (W256.of_int res{2}.`2) (W256.of_int res{2}.`3) (W256.of_int res{2}.`4) (W256.of_int res{2}.`5) 
+  (W256.of_int res{2}.`6) (W256.of_int res{2}.`7) (W256.of_int res{2}.`8)
+  (W256.of_int res{2}.`9) (W256.of_int res{2}.`10)
+  (W256.of_int res{2}.`11) (W256.of_int res{2}.`12) (W256.of_int res{2}.`13)
+  v1 v2 v3 v4 v5 v6 v7 v8 /\
+  res{2}.`1 = Some true /\
+  0 <= res{2}.`2 < Constants.R /\
+  0 <= res{2}.`3 < Constants.R /\
+  0 <= res{2}.`4 < Constants.R /\
+  0 <= res{2}.`5 < Constants.R /\
+  0 <= res{2}.`6 < Constants.R /\
+  0 <= res{2}.`7 < Constants.R /\
+  0 <= res{2}.`8 < Constants.R /\
+  0 <= res{2}.`9 < Constants.R /\
+  0 <= res{2}.`10 < Constants.R /\
+  0 <= res{2}.`11 < Constants.R /\
+  0 <= res{2}.`12 < Constants.R /\
+  0 <= res{2}.`13 < Constants.R)
+].
+proof. proc.
 
+seq 1 0: (#pre /\ to_uint alpha{1} = stateAlpha{2}).
+call{1} (ConcretePrimops.mload_pspec m STATE_ALPHA_SLOT). skip. by progress. 
 
+seq 1 1: (#pre /\ to_uint currentAlpha{1} = statePowerOfAlpha2{2} /\ statePowerOfAlpha2{2} = (stateAlpha{2} * stateAlpha{2}) %% Constants.R).
+wp. skip. rewrite /mulmod. progress. rewrite H0. smt(@W256 @Utils).
+exists* statePowerOfAlpha2{2}. elim*=> a2.
+pose m2 := store m STATE_POWER_OF_ALPHA_2_SLOT (W256.of_int a2).
+seq 1 0: (
+(stateAlpha{2}, stateBeta{2}, stateBetaLookup{2}, stateGamma{2},
+ stateGammaLookup{2}, stateZ{2}, proofPublicInput{2},
+ proofCopyPermutationPolys0OpeningAtZ{2},
+ proofCopyPermutationPolys1OpeningAtZ{2},
+ proofCopyPermutationPolys2OpeningAtZ{2}, proofStatePolys0OpeningAtZ{2},
+ proofStatePolys1OpeningAtZ{2}, proofStatePolys2OpeningAtZ{2},
+ proofStatePolys3OpeningAtZ{2}, proofLookupSPolyOpeningAtZOmega{2},
+ proofLookupGrandProductOpeningAtZOmega{2},
+ proofGateSelectors0OpeningAtZ{2}, proofLinearisationPolyOpeningAtZ{2},
+ proofCopyPermutationGrandProductOpeningAtZOmega{2},
+ stateZInDomainSize{2}, proofQuotientPolyOpeningAtZ{2}) =
+(stateAlphaG, stateBetaG, stateBetaLookupG, stateGammaG,
+ stateGammaLookupG, stateZG, proofPublicInputG,
+ proofCopyPermutationPolys0OpeningAtZG,
+ proofCopyPermutationPolys1OpeningAtZG,
+ proofCopyPermutationPolys2OpeningAtZG, proofStatePolys0OpeningAtZG,
+ proofStatePolys1OpeningAtZG, proofStatePolys2OpeningAtZG,
+ proofStatePolys3OpeningAtZG, proofLookupSPolyOpeningAtZOmegaG,
+ proofLookupGrandProductOpeningAtZOmegaG, proofGateSelectors0OpeningAtZG,
+ proofLinearisationPolyOpeningAtZG,
+ proofCopyPermutationGrandProductOpeningAtZOmegaG, stateZInDomainSizeG,
+ proofQuotientPolyOpeningAtZG) /\
+W256.to_uint (mload m STATE_ALPHA_SLOT) = stateAlphaG /\
+W256.to_uint (mload m STATE_BETA_SLOT) = stateBetaG /\
+W256.to_uint (mload m STATE_BETA_LOOKUP_SLOT) = stateBetaLookupG /\
+W256.to_uint (mload m STATE_GAMMA_SLOT) = stateGammaG /\
+W256.to_uint (mload m STATE_GAMMA_LOOKUP_SLOT) = stateGammaLookupG /\
+W256.to_uint (mload m STATE_Z_SLOT) = stateZG /\
+W256.to_uint (mload m PROOF_PUBLIC_INPUT) = proofPublicInputG /\
+W256.to_uint (mload m PROOF_COPY_PERMUTATION_POLYS_0_OPENING_AT_Z_SLOT) = proofCopyPermutationPolys0OpeningAtZG /\
+W256.to_uint (mload m PROOF_COPY_PERMUTATION_POLYS_1_OPENING_AT_Z_SLOT) = proofCopyPermutationPolys1OpeningAtZG /\
+W256.to_uint (mload m PROOF_COPY_PERMUTATION_POLYS_2_OPENING_AT_Z_SLOT) = proofCopyPermutationPolys2OpeningAtZG /\
+W256.to_uint (mload m PROOF_STATE_POLYS_0_OPENING_AT_Z_SLOT) = proofStatePolys0OpeningAtZG /\
+W256.to_uint (mload m PROOF_STATE_POLYS_1_OPENING_AT_Z_SLOT) = proofStatePolys1OpeningAtZG /\
+W256.to_uint (mload m PROOF_STATE_POLYS_2_OPENING_AT_Z_SLOT) = proofStatePolys2OpeningAtZG /\
+W256.to_uint (mload m PROOF_STATE_POLYS_3_OPENING_AT_Z_SLOT) = proofStatePolys3OpeningAtZG /\
+W256.to_uint (mload m PROOF_LOOKUP_S_POLY_OPENING_AT_Z_OMEGA_SLOT) = proofLookupSPolyOpeningAtZOmegaG /\
+W256.to_uint (mload m PROOF_LOOKUP_GRAND_PRODUCT_OPENING_AT_Z_OMEGA_SLOT) = proofLookupGrandProductOpeningAtZOmegaG /\
+W256.to_uint (mload m PROOF_GATE_SELECTORS_0_OPENING_AT_Z_SLOT) = proofGateSelectors0OpeningAtZG /\
+W256.to_uint (mload m PROOF_LINEARISATION_POLY_OPENING_AT_Z_SLOT) = proofLinearisationPolyOpeningAtZG /\
+W256.to_uint (mload m PROOF_COPY_PERMUTATION_GRAND_PRODUCT_OPENING_AT_Z_OMEGA_SLOT) = proofCopyPermutationGrandProductOpeningAtZOmegaG /\
+W256.to_uint (mload m STATE_Z_IN_DOMAIN_SIZE) = stateZInDomainSizeG /\
+W256.to_uint (mload m PROOF_QUOTIENT_POLY_OPENING_AT_Z_SLOT) = proofQuotientPolyOpeningAtZG /\
+    !Primops.reverted{1} /\
+    to_uint alpha{1} = stateAlpha{2} /\
+    to_uint currentAlpha{1} = statePowerOfAlpha2{2} /\
+    a2 = statePowerOfAlpha2{2} /\
+    statePowerOfAlpha2{2} = (stateAlpha{2} * stateAlpha{2}) %% Constants.R /\
+    Primops.memory{1} = m2
+).
+call{1} (ConcretePrimops.mstore_pspec m STATE_POWER_OF_ALPHA_2_SLOT (W256.of_int a2)).
+skip. by progress.
 
+seq 1 1: (
+(stateAlpha{2}, stateBeta{2}, stateBetaLookup{2}, stateGamma{2},
+ stateGammaLookup{2}, stateZ{2}, proofPublicInput{2},
+ proofCopyPermutationPolys0OpeningAtZ{2},
+ proofCopyPermutationPolys1OpeningAtZ{2},
+ proofCopyPermutationPolys2OpeningAtZ{2}, proofStatePolys0OpeningAtZ{2},
+ proofStatePolys1OpeningAtZ{2}, proofStatePolys2OpeningAtZ{2},
+ proofStatePolys3OpeningAtZ{2}, proofLookupSPolyOpeningAtZOmega{2},
+ proofLookupGrandProductOpeningAtZOmega{2},
+ proofGateSelectors0OpeningAtZ{2}, proofLinearisationPolyOpeningAtZ{2},
+ proofCopyPermutationGrandProductOpeningAtZOmega{2},
+ stateZInDomainSize{2}, proofQuotientPolyOpeningAtZ{2}) =
+(stateAlphaG, stateBetaG, stateBetaLookupG, stateGammaG,
+ stateGammaLookupG, stateZG, proofPublicInputG,
+ proofCopyPermutationPolys0OpeningAtZG,
+ proofCopyPermutationPolys1OpeningAtZG,
+ proofCopyPermutationPolys2OpeningAtZG, proofStatePolys0OpeningAtZG,
+ proofStatePolys1OpeningAtZG, proofStatePolys2OpeningAtZG,
+ proofStatePolys3OpeningAtZG, proofLookupSPolyOpeningAtZOmegaG,
+ proofLookupGrandProductOpeningAtZOmegaG, proofGateSelectors0OpeningAtZG,
+ proofLinearisationPolyOpeningAtZG,
+ proofCopyPermutationGrandProductOpeningAtZOmegaG, stateZInDomainSizeG,
+ proofQuotientPolyOpeningAtZG) /\
+W256.to_uint (mload m STATE_ALPHA_SLOT) = stateAlphaG /\
+W256.to_uint (mload m STATE_BETA_SLOT) = stateBetaG /\
+W256.to_uint (mload m STATE_BETA_LOOKUP_SLOT) = stateBetaLookupG /\
+W256.to_uint (mload m STATE_GAMMA_SLOT) = stateGammaG /\
+W256.to_uint (mload m STATE_GAMMA_LOOKUP_SLOT) = stateGammaLookupG /\
+W256.to_uint (mload m STATE_Z_SLOT) = stateZG /\
+W256.to_uint (mload m PROOF_PUBLIC_INPUT) = proofPublicInputG /\
+W256.to_uint (mload m PROOF_COPY_PERMUTATION_POLYS_0_OPENING_AT_Z_SLOT) = proofCopyPermutationPolys0OpeningAtZG /\
+W256.to_uint (mload m PROOF_COPY_PERMUTATION_POLYS_1_OPENING_AT_Z_SLOT) = proofCopyPermutationPolys1OpeningAtZG /\
+W256.to_uint (mload m PROOF_COPY_PERMUTATION_POLYS_2_OPENING_AT_Z_SLOT) = proofCopyPermutationPolys2OpeningAtZG /\
+W256.to_uint (mload m PROOF_STATE_POLYS_0_OPENING_AT_Z_SLOT) = proofStatePolys0OpeningAtZG /\
+W256.to_uint (mload m PROOF_STATE_POLYS_1_OPENING_AT_Z_SLOT) = proofStatePolys1OpeningAtZG /\
+W256.to_uint (mload m PROOF_STATE_POLYS_2_OPENING_AT_Z_SLOT) = proofStatePolys2OpeningAtZG /\
+W256.to_uint (mload m PROOF_STATE_POLYS_3_OPENING_AT_Z_SLOT) = proofStatePolys3OpeningAtZG /\
+W256.to_uint (mload m PROOF_LOOKUP_S_POLY_OPENING_AT_Z_OMEGA_SLOT) = proofLookupSPolyOpeningAtZOmegaG /\
+W256.to_uint (mload m PROOF_LOOKUP_GRAND_PRODUCT_OPENING_AT_Z_OMEGA_SLOT) = proofLookupGrandProductOpeningAtZOmegaG /\
+W256.to_uint (mload m PROOF_GATE_SELECTORS_0_OPENING_AT_Z_SLOT) = proofGateSelectors0OpeningAtZG /\
+W256.to_uint (mload m PROOF_LINEARISATION_POLY_OPENING_AT_Z_SLOT) = proofLinearisationPolyOpeningAtZG /\
+W256.to_uint (mload m PROOF_COPY_PERMUTATION_GRAND_PRODUCT_OPENING_AT_Z_OMEGA_SLOT) = proofCopyPermutationGrandProductOpeningAtZOmegaG /\
+W256.to_uint (mload m STATE_Z_IN_DOMAIN_SIZE) = stateZInDomainSizeG /\
+W256.to_uint (mload m PROOF_QUOTIENT_POLY_OPENING_AT_Z_SLOT) = proofQuotientPolyOpeningAtZG /\
+!Primops.reverted{1} /\
+Primops.memory{1} = store m STATE_POWER_OF_ALPHA_2_SLOT (W256.of_int statePowerOfAlpha2{2}) /\
+    to_uint alpha{1} = stateAlpha{2} /\
+    a2 = statePowerOfAlpha2{2} /\
+    statePowerOfAlpha2{2} = (stateAlpha{2} * stateAlpha{2}) %% Constants.R /\
+    to_uint currentAlpha{1} = statePowerOfAlpha3{2} /\
+    statePowerOfAlpha3{2} = (statePowerOfAlpha2{2} * stateAlpha{2}) %% Constants.R
+).
+wp. skip. rewrite /mulmod. progress. rewrite H1 -H0.
+rewrite W256.to_uint_small. progress. smt(@W256 @Utils). smt(@W256 @Utils). 
+rewrite W256.to_uint_small. progress. smt(@W256 @Utils). rewrite H1 -H0. smt().
+exists* statePowerOfAlpha3{2}. elim*=> a3.
+pose m3 := store m2 STATE_POWER_OF_ALPHA_3_SLOT (W256.of_int a3).
+seq 1 0: (
+(stateAlpha{2}, stateBeta{2}, stateBetaLookup{2}, stateGamma{2},
+ stateGammaLookup{2}, stateZ{2}, proofPublicInput{2},
+ proofCopyPermutationPolys0OpeningAtZ{2},
+ proofCopyPermutationPolys1OpeningAtZ{2},
+ proofCopyPermutationPolys2OpeningAtZ{2}, proofStatePolys0OpeningAtZ{2},
+ proofStatePolys1OpeningAtZ{2}, proofStatePolys2OpeningAtZ{2},
+ proofStatePolys3OpeningAtZ{2}, proofLookupSPolyOpeningAtZOmega{2},
+ proofLookupGrandProductOpeningAtZOmega{2},
+ proofGateSelectors0OpeningAtZ{2}, proofLinearisationPolyOpeningAtZ{2},
+ proofCopyPermutationGrandProductOpeningAtZOmega{2},
+ stateZInDomainSize{2}, proofQuotientPolyOpeningAtZ{2}) =
+(stateAlphaG, stateBetaG, stateBetaLookupG, stateGammaG,
+ stateGammaLookupG, stateZG, proofPublicInputG,
+ proofCopyPermutationPolys0OpeningAtZG,
+ proofCopyPermutationPolys1OpeningAtZG,
+ proofCopyPermutationPolys2OpeningAtZG, proofStatePolys0OpeningAtZG,
+ proofStatePolys1OpeningAtZG, proofStatePolys2OpeningAtZG,
+ proofStatePolys3OpeningAtZG, proofLookupSPolyOpeningAtZOmegaG,
+ proofLookupGrandProductOpeningAtZOmegaG, proofGateSelectors0OpeningAtZG,
+ proofLinearisationPolyOpeningAtZG,
+ proofCopyPermutationGrandProductOpeningAtZOmegaG, stateZInDomainSizeG,
+ proofQuotientPolyOpeningAtZG) /\
+W256.to_uint (mload m STATE_ALPHA_SLOT) = stateAlphaG /\
+W256.to_uint (mload m STATE_BETA_SLOT) = stateBetaG /\
+W256.to_uint (mload m STATE_BETA_LOOKUP_SLOT) = stateBetaLookupG /\
+W256.to_uint (mload m STATE_GAMMA_SLOT) = stateGammaG /\
+W256.to_uint (mload m STATE_GAMMA_LOOKUP_SLOT) = stateGammaLookupG /\
+W256.to_uint (mload m STATE_Z_SLOT) = stateZG /\
+W256.to_uint (mload m PROOF_PUBLIC_INPUT) = proofPublicInputG /\
+W256.to_uint (mload m PROOF_COPY_PERMUTATION_POLYS_0_OPENING_AT_Z_SLOT) = proofCopyPermutationPolys0OpeningAtZG /\
+W256.to_uint (mload m PROOF_COPY_PERMUTATION_POLYS_1_OPENING_AT_Z_SLOT) = proofCopyPermutationPolys1OpeningAtZG /\
+W256.to_uint (mload m PROOF_COPY_PERMUTATION_POLYS_2_OPENING_AT_Z_SLOT) = proofCopyPermutationPolys2OpeningAtZG /\
+W256.to_uint (mload m PROOF_STATE_POLYS_0_OPENING_AT_Z_SLOT) = proofStatePolys0OpeningAtZG /\
+W256.to_uint (mload m PROOF_STATE_POLYS_1_OPENING_AT_Z_SLOT) = proofStatePolys1OpeningAtZG /\
+W256.to_uint (mload m PROOF_STATE_POLYS_2_OPENING_AT_Z_SLOT) = proofStatePolys2OpeningAtZG /\
+W256.to_uint (mload m PROOF_STATE_POLYS_3_OPENING_AT_Z_SLOT) = proofStatePolys3OpeningAtZG /\
+W256.to_uint (mload m PROOF_LOOKUP_S_POLY_OPENING_AT_Z_OMEGA_SLOT) = proofLookupSPolyOpeningAtZOmegaG /\
+W256.to_uint (mload m PROOF_LOOKUP_GRAND_PRODUCT_OPENING_AT_Z_OMEGA_SLOT) = proofLookupGrandProductOpeningAtZOmegaG /\
+W256.to_uint (mload m PROOF_GATE_SELECTORS_0_OPENING_AT_Z_SLOT) = proofGateSelectors0OpeningAtZG /\
+W256.to_uint (mload m PROOF_LINEARISATION_POLY_OPENING_AT_Z_SLOT) = proofLinearisationPolyOpeningAtZG /\
+W256.to_uint (mload m PROOF_COPY_PERMUTATION_GRAND_PRODUCT_OPENING_AT_Z_OMEGA_SLOT) = proofCopyPermutationGrandProductOpeningAtZOmegaG /\
+W256.to_uint (mload m STATE_Z_IN_DOMAIN_SIZE) = stateZInDomainSizeG /\
+W256.to_uint (mload m PROOF_QUOTIENT_POLY_OPENING_AT_Z_SLOT) = proofQuotientPolyOpeningAtZG /\
+!Primops.reverted{1} /\
+    to_uint alpha{1} = stateAlpha{2} /\
+    a2 = statePowerOfAlpha2{2} /\
+    a3 = statePowerOfAlpha3{2} /\
+    statePowerOfAlpha2{2} = (stateAlpha{2} * stateAlpha{2}) %% Constants.R /\
+    statePowerOfAlpha3{2} = (statePowerOfAlpha2{2} * stateAlpha{2}) %% Constants.R /\
+    to_uint currentAlpha{1} = statePowerOfAlpha3{2} /\
+    Primops.memory{1} = m3
+).
+call{1} (ConcretePrimops.mstore_pspec m2 STATE_POWER_OF_ALPHA_3_SLOT (W256.of_int a3)).
+skip. by progress.
 
+seq 1 1: (
+(stateAlpha{2}, stateBeta{2}, stateBetaLookup{2}, stateGamma{2},
+ stateGammaLookup{2}, stateZ{2}, proofPublicInput{2},
+ proofCopyPermutationPolys0OpeningAtZ{2},
+ proofCopyPermutationPolys1OpeningAtZ{2},
+ proofCopyPermutationPolys2OpeningAtZ{2}, proofStatePolys0OpeningAtZ{2},
+ proofStatePolys1OpeningAtZ{2}, proofStatePolys2OpeningAtZ{2},
+ proofStatePolys3OpeningAtZ{2}, proofLookupSPolyOpeningAtZOmega{2},
+ proofLookupGrandProductOpeningAtZOmega{2},
+ proofGateSelectors0OpeningAtZ{2}, proofLinearisationPolyOpeningAtZ{2},
+ proofCopyPermutationGrandProductOpeningAtZOmega{2},
+ stateZInDomainSize{2}, proofQuotientPolyOpeningAtZ{2}) =
+(stateAlphaG, stateBetaG, stateBetaLookupG, stateGammaG,
+ stateGammaLookupG, stateZG, proofPublicInputG,
+ proofCopyPermutationPolys0OpeningAtZG,
+ proofCopyPermutationPolys1OpeningAtZG,
+ proofCopyPermutationPolys2OpeningAtZG, proofStatePolys0OpeningAtZG,
+ proofStatePolys1OpeningAtZG, proofStatePolys2OpeningAtZG,
+ proofStatePolys3OpeningAtZG, proofLookupSPolyOpeningAtZOmegaG,
+ proofLookupGrandProductOpeningAtZOmegaG, proofGateSelectors0OpeningAtZG,
+ proofLinearisationPolyOpeningAtZG,
+ proofCopyPermutationGrandProductOpeningAtZOmegaG, stateZInDomainSizeG,
+ proofQuotientPolyOpeningAtZG) /\
+W256.to_uint (mload m STATE_ALPHA_SLOT) = stateAlphaG /\
+W256.to_uint (mload m STATE_BETA_SLOT) = stateBetaG /\
+W256.to_uint (mload m STATE_BETA_LOOKUP_SLOT) = stateBetaLookupG /\
+W256.to_uint (mload m STATE_GAMMA_SLOT) = stateGammaG /\
+W256.to_uint (mload m STATE_GAMMA_LOOKUP_SLOT) = stateGammaLookupG /\
+W256.to_uint (mload m STATE_Z_SLOT) = stateZG /\
+W256.to_uint (mload m PROOF_PUBLIC_INPUT) = proofPublicInputG /\
+W256.to_uint (mload m PROOF_COPY_PERMUTATION_POLYS_0_OPENING_AT_Z_SLOT) = proofCopyPermutationPolys0OpeningAtZG /\
+W256.to_uint (mload m PROOF_COPY_PERMUTATION_POLYS_1_OPENING_AT_Z_SLOT) = proofCopyPermutationPolys1OpeningAtZG /\
+W256.to_uint (mload m PROOF_COPY_PERMUTATION_POLYS_2_OPENING_AT_Z_SLOT) = proofCopyPermutationPolys2OpeningAtZG /\
+W256.to_uint (mload m PROOF_STATE_POLYS_0_OPENING_AT_Z_SLOT) = proofStatePolys0OpeningAtZG /\
+W256.to_uint (mload m PROOF_STATE_POLYS_1_OPENING_AT_Z_SLOT) = proofStatePolys1OpeningAtZG /\
+W256.to_uint (mload m PROOF_STATE_POLYS_2_OPENING_AT_Z_SLOT) = proofStatePolys2OpeningAtZG /\
+W256.to_uint (mload m PROOF_STATE_POLYS_3_OPENING_AT_Z_SLOT) = proofStatePolys3OpeningAtZG /\
+W256.to_uint (mload m PROOF_LOOKUP_S_POLY_OPENING_AT_Z_OMEGA_SLOT) = proofLookupSPolyOpeningAtZOmegaG /\
+W256.to_uint (mload m PROOF_LOOKUP_GRAND_PRODUCT_OPENING_AT_Z_OMEGA_SLOT) = proofLookupGrandProductOpeningAtZOmegaG /\
+W256.to_uint (mload m PROOF_GATE_SELECTORS_0_OPENING_AT_Z_SLOT) = proofGateSelectors0OpeningAtZG /\
+W256.to_uint (mload m PROOF_LINEARISATION_POLY_OPENING_AT_Z_SLOT) = proofLinearisationPolyOpeningAtZG /\
+W256.to_uint (mload m PROOF_COPY_PERMUTATION_GRAND_PRODUCT_OPENING_AT_Z_OMEGA_SLOT) = proofCopyPermutationGrandProductOpeningAtZOmegaG /\
+W256.to_uint (mload m STATE_Z_IN_DOMAIN_SIZE) = stateZInDomainSizeG /\
+W256.to_uint (mload m PROOF_QUOTIENT_POLY_OPENING_AT_Z_SLOT) = proofQuotientPolyOpeningAtZG /\
+!Primops.reverted{1} /\
+    to_uint alpha{1} = stateAlpha{2} /\
+    a2 = statePowerOfAlpha2{2} /\
+    a3 = statePowerOfAlpha3{2} /\
+    statePowerOfAlpha2{2} = (stateAlpha{2} * stateAlpha{2}) %% Constants.R /\
+    statePowerOfAlpha3{2} = (statePowerOfAlpha2{2} * stateAlpha{2}) %% Constants.R /\
+    statePowerOfAlpha4{2} = (statePowerOfAlpha3{2} * stateAlpha{2}) %% Constants.R /\
+    to_uint currentAlpha{1} = statePowerOfAlpha4{2} /\
+    Primops.memory{1} = m3
+).
+wp. skip. rewrite /mulmod. progress. smt(). rewrite H1 -H0.
+rewrite W256.to_uint_small. progress. smt(@W256 @Utils). smt(@W256 @Utils).
+rewrite W256.to_uint_small. progress. smt(@W256 @Utils).
+exists* statePowerOfAlpha4{2}. elim*=> a4.
+pose m4 := store m3 STATE_POWER_OF_ALPHA_4_SLOT (W256.of_int a4).
+seq 1 0: (
+(stateAlpha{2}, stateBeta{2}, stateBetaLookup{2}, stateGamma{2},
+ stateGammaLookup{2}, stateZ{2}, proofPublicInput{2},
+ proofCopyPermutationPolys0OpeningAtZ{2},
+ proofCopyPermutationPolys1OpeningAtZ{2},
+ proofCopyPermutationPolys2OpeningAtZ{2}, proofStatePolys0OpeningAtZ{2},
+ proofStatePolys1OpeningAtZ{2}, proofStatePolys2OpeningAtZ{2},
+ proofStatePolys3OpeningAtZ{2}, proofLookupSPolyOpeningAtZOmega{2},
+ proofLookupGrandProductOpeningAtZOmega{2},
+ proofGateSelectors0OpeningAtZ{2}, proofLinearisationPolyOpeningAtZ{2},
+ proofCopyPermutationGrandProductOpeningAtZOmega{2},
+ stateZInDomainSize{2}, proofQuotientPolyOpeningAtZ{2}) =
+(stateAlphaG, stateBetaG, stateBetaLookupG, stateGammaG,
+ stateGammaLookupG, stateZG, proofPublicInputG,
+ proofCopyPermutationPolys0OpeningAtZG,
+ proofCopyPermutationPolys1OpeningAtZG,
+ proofCopyPermutationPolys2OpeningAtZG, proofStatePolys0OpeningAtZG,
+ proofStatePolys1OpeningAtZG, proofStatePolys2OpeningAtZG,
+ proofStatePolys3OpeningAtZG, proofLookupSPolyOpeningAtZOmegaG,
+ proofLookupGrandProductOpeningAtZOmegaG, proofGateSelectors0OpeningAtZG,
+ proofLinearisationPolyOpeningAtZG,
+ proofCopyPermutationGrandProductOpeningAtZOmegaG, stateZInDomainSizeG,
+ proofQuotientPolyOpeningAtZG) /\
+W256.to_uint (mload m STATE_ALPHA_SLOT) = stateAlphaG /\
+W256.to_uint (mload m STATE_BETA_SLOT) = stateBetaG /\
+W256.to_uint (mload m STATE_BETA_LOOKUP_SLOT) = stateBetaLookupG /\
+W256.to_uint (mload m STATE_GAMMA_SLOT) = stateGammaG /\
+W256.to_uint (mload m STATE_GAMMA_LOOKUP_SLOT) = stateGammaLookupG /\
+W256.to_uint (mload m STATE_Z_SLOT) = stateZG /\
+W256.to_uint (mload m PROOF_PUBLIC_INPUT) = proofPublicInputG /\
+W256.to_uint (mload m PROOF_COPY_PERMUTATION_POLYS_0_OPENING_AT_Z_SLOT) = proofCopyPermutationPolys0OpeningAtZG /\
+W256.to_uint (mload m PROOF_COPY_PERMUTATION_POLYS_1_OPENING_AT_Z_SLOT) = proofCopyPermutationPolys1OpeningAtZG /\
+W256.to_uint (mload m PROOF_COPY_PERMUTATION_POLYS_2_OPENING_AT_Z_SLOT) = proofCopyPermutationPolys2OpeningAtZG /\
+W256.to_uint (mload m PROOF_STATE_POLYS_0_OPENING_AT_Z_SLOT) = proofStatePolys0OpeningAtZG /\
+W256.to_uint (mload m PROOF_STATE_POLYS_1_OPENING_AT_Z_SLOT) = proofStatePolys1OpeningAtZG /\
+W256.to_uint (mload m PROOF_STATE_POLYS_2_OPENING_AT_Z_SLOT) = proofStatePolys2OpeningAtZG /\
+W256.to_uint (mload m PROOF_STATE_POLYS_3_OPENING_AT_Z_SLOT) = proofStatePolys3OpeningAtZG /\
+W256.to_uint (mload m PROOF_LOOKUP_S_POLY_OPENING_AT_Z_OMEGA_SLOT) = proofLookupSPolyOpeningAtZOmegaG /\
+W256.to_uint (mload m PROOF_LOOKUP_GRAND_PRODUCT_OPENING_AT_Z_OMEGA_SLOT) = proofLookupGrandProductOpeningAtZOmegaG /\
+W256.to_uint (mload m PROOF_GATE_SELECTORS_0_OPENING_AT_Z_SLOT) = proofGateSelectors0OpeningAtZG /\
+W256.to_uint (mload m PROOF_LINEARISATION_POLY_OPENING_AT_Z_SLOT) = proofLinearisationPolyOpeningAtZG /\
+W256.to_uint (mload m PROOF_COPY_PERMUTATION_GRAND_PRODUCT_OPENING_AT_Z_OMEGA_SLOT) = proofCopyPermutationGrandProductOpeningAtZOmegaG /\
+W256.to_uint (mload m STATE_Z_IN_DOMAIN_SIZE) = stateZInDomainSizeG /\
+W256.to_uint (mload m PROOF_QUOTIENT_POLY_OPENING_AT_Z_SLOT) = proofQuotientPolyOpeningAtZG /\
+!Primops.reverted{1} /\
+    to_uint alpha{1} = stateAlpha{2} /\
+    a2 = statePowerOfAlpha2{2} /\
+    a3 = statePowerOfAlpha3{2} /\
+    a4 = statePowerOfAlpha4{2} /\
+    statePowerOfAlpha2{2} = (stateAlpha{2} * stateAlpha{2}) %% Constants.R /\
+    statePowerOfAlpha3{2} = (statePowerOfAlpha2{2} * stateAlpha{2}) %% Constants.R /\
+    statePowerOfAlpha4{2} = (statePowerOfAlpha3{2} * stateAlpha{2}) %% Constants.R /\
+    to_uint currentAlpha{1} = statePowerOfAlpha4{2} /\
+    Primops.memory{1} = m4
+).
+call{1} (ConcretePrimops.mstore_pspec m3 STATE_POWER_OF_ALPHA_4_SLOT (W256.of_int a4)).
+skip. progress. smt(@W256 @Utils).
 
+seq 1 1: (
+(stateAlpha{2}, stateBeta{2}, stateBetaLookup{2}, stateGamma{2},
+ stateGammaLookup{2}, stateZ{2}, proofPublicInput{2},
+ proofCopyPermutationPolys0OpeningAtZ{2},
+ proofCopyPermutationPolys1OpeningAtZ{2},
+ proofCopyPermutationPolys2OpeningAtZ{2}, proofStatePolys0OpeningAtZ{2},
+ proofStatePolys1OpeningAtZ{2}, proofStatePolys2OpeningAtZ{2},
+ proofStatePolys3OpeningAtZ{2}, proofLookupSPolyOpeningAtZOmega{2},
+ proofLookupGrandProductOpeningAtZOmega{2},
+ proofGateSelectors0OpeningAtZ{2}, proofLinearisationPolyOpeningAtZ{2},
+ proofCopyPermutationGrandProductOpeningAtZOmega{2},
+ stateZInDomainSize{2}, proofQuotientPolyOpeningAtZ{2}) =
+(stateAlphaG, stateBetaG, stateBetaLookupG, stateGammaG,
+ stateGammaLookupG, stateZG, proofPublicInputG,
+ proofCopyPermutationPolys0OpeningAtZG,
+ proofCopyPermutationPolys1OpeningAtZG,
+ proofCopyPermutationPolys2OpeningAtZG, proofStatePolys0OpeningAtZG,
+ proofStatePolys1OpeningAtZG, proofStatePolys2OpeningAtZG,
+ proofStatePolys3OpeningAtZG, proofLookupSPolyOpeningAtZOmegaG,
+ proofLookupGrandProductOpeningAtZOmegaG, proofGateSelectors0OpeningAtZG,
+ proofLinearisationPolyOpeningAtZG,
+ proofCopyPermutationGrandProductOpeningAtZOmegaG, stateZInDomainSizeG,
+ proofQuotientPolyOpeningAtZG) /\
+W256.to_uint (mload m STATE_ALPHA_SLOT) = stateAlphaG /\
+W256.to_uint (mload m STATE_BETA_SLOT) = stateBetaG /\
+W256.to_uint (mload m STATE_BETA_LOOKUP_SLOT) = stateBetaLookupG /\
+W256.to_uint (mload m STATE_GAMMA_SLOT) = stateGammaG /\
+W256.to_uint (mload m STATE_GAMMA_LOOKUP_SLOT) = stateGammaLookupG /\
+W256.to_uint (mload m STATE_Z_SLOT) = stateZG /\
+W256.to_uint (mload m PROOF_PUBLIC_INPUT) = proofPublicInputG /\
+W256.to_uint (mload m PROOF_COPY_PERMUTATION_POLYS_0_OPENING_AT_Z_SLOT) = proofCopyPermutationPolys0OpeningAtZG /\
+W256.to_uint (mload m PROOF_COPY_PERMUTATION_POLYS_1_OPENING_AT_Z_SLOT) = proofCopyPermutationPolys1OpeningAtZG /\
+W256.to_uint (mload m PROOF_COPY_PERMUTATION_POLYS_2_OPENING_AT_Z_SLOT) = proofCopyPermutationPolys2OpeningAtZG /\
+W256.to_uint (mload m PROOF_STATE_POLYS_0_OPENING_AT_Z_SLOT) = proofStatePolys0OpeningAtZG /\
+W256.to_uint (mload m PROOF_STATE_POLYS_1_OPENING_AT_Z_SLOT) = proofStatePolys1OpeningAtZG /\
+W256.to_uint (mload m PROOF_STATE_POLYS_2_OPENING_AT_Z_SLOT) = proofStatePolys2OpeningAtZG /\
+W256.to_uint (mload m PROOF_STATE_POLYS_3_OPENING_AT_Z_SLOT) = proofStatePolys3OpeningAtZG /\
+W256.to_uint (mload m PROOF_LOOKUP_S_POLY_OPENING_AT_Z_OMEGA_SLOT) = proofLookupSPolyOpeningAtZOmegaG /\
+W256.to_uint (mload m PROOF_LOOKUP_GRAND_PRODUCT_OPENING_AT_Z_OMEGA_SLOT) = proofLookupGrandProductOpeningAtZOmegaG /\
+W256.to_uint (mload m PROOF_GATE_SELECTORS_0_OPENING_AT_Z_SLOT) = proofGateSelectors0OpeningAtZG /\
+W256.to_uint (mload m PROOF_LINEARISATION_POLY_OPENING_AT_Z_SLOT) = proofLinearisationPolyOpeningAtZG /\
+W256.to_uint (mload m PROOF_COPY_PERMUTATION_GRAND_PRODUCT_OPENING_AT_Z_OMEGA_SLOT) = proofCopyPermutationGrandProductOpeningAtZOmegaG /\
+W256.to_uint (mload m STATE_Z_IN_DOMAIN_SIZE) = stateZInDomainSizeG /\
+W256.to_uint (mload m PROOF_QUOTIENT_POLY_OPENING_AT_Z_SLOT) = proofQuotientPolyOpeningAtZG /\
+!Primops.reverted{1} /\
+    to_uint alpha{1} = stateAlpha{2} /\
+    a2 = statePowerOfAlpha2{2} /\
+    a3 = statePowerOfAlpha3{2} /\
+    a4 = statePowerOfAlpha4{2} /\
+    statePowerOfAlpha2{2} = (stateAlpha{2} * stateAlpha{2}) %% Constants.R /\
+    statePowerOfAlpha3{2} = (statePowerOfAlpha2{2} * stateAlpha{2}) %% Constants.R /\
+    statePowerOfAlpha4{2} = (statePowerOfAlpha3{2} * stateAlpha{2}) %% Constants.R /\
+    statePowerOfAlpha5{2} = (statePowerOfAlpha4{2} * stateAlpha{2}) %% Constants.R /\
+    to_uint currentAlpha{1} = statePowerOfAlpha5{2} /\
+    Primops.memory{1} = m4
+).
+wp. skip. rewrite /mulmod. progress. smt(). rewrite H1 -H0.
+rewrite W256.to_uint_small. progress. smt(@W256 @Utils). smt(@W256 @Utils).
+rewrite W256.to_uint_small. progress. smt(@W256 @Utils).
+exists* statePowerOfAlpha5{2}. elim*=> a5.
+pose m5 := store m4 STATE_POWER_OF_ALPHA_5_SLOT (W256.of_int a5).
+seq 1 0: (
+(stateAlpha{2}, stateBeta{2}, stateBetaLookup{2}, stateGamma{2},
+ stateGammaLookup{2}, stateZ{2}, proofPublicInput{2},
+ proofCopyPermutationPolys0OpeningAtZ{2},
+ proofCopyPermutationPolys1OpeningAtZ{2},
+ proofCopyPermutationPolys2OpeningAtZ{2}, proofStatePolys0OpeningAtZ{2},
+ proofStatePolys1OpeningAtZ{2}, proofStatePolys2OpeningAtZ{2},
+ proofStatePolys3OpeningAtZ{2}, proofLookupSPolyOpeningAtZOmega{2},
+ proofLookupGrandProductOpeningAtZOmega{2},
+ proofGateSelectors0OpeningAtZ{2}, proofLinearisationPolyOpeningAtZ{2},
+ proofCopyPermutationGrandProductOpeningAtZOmega{2},
+ stateZInDomainSize{2}, proofQuotientPolyOpeningAtZ{2}) =
+(stateAlphaG, stateBetaG, stateBetaLookupG, stateGammaG,
+ stateGammaLookupG, stateZG, proofPublicInputG,
+ proofCopyPermutationPolys0OpeningAtZG,
+ proofCopyPermutationPolys1OpeningAtZG,
+ proofCopyPermutationPolys2OpeningAtZG, proofStatePolys0OpeningAtZG,
+ proofStatePolys1OpeningAtZG, proofStatePolys2OpeningAtZG,
+ proofStatePolys3OpeningAtZG, proofLookupSPolyOpeningAtZOmegaG,
+ proofLookupGrandProductOpeningAtZOmegaG, proofGateSelectors0OpeningAtZG,
+ proofLinearisationPolyOpeningAtZG,
+ proofCopyPermutationGrandProductOpeningAtZOmegaG, stateZInDomainSizeG,
+ proofQuotientPolyOpeningAtZG) /\
+W256.to_uint (mload m STATE_ALPHA_SLOT) = stateAlphaG /\
+W256.to_uint (mload m STATE_BETA_SLOT) = stateBetaG /\
+W256.to_uint (mload m STATE_BETA_LOOKUP_SLOT) = stateBetaLookupG /\
+W256.to_uint (mload m STATE_GAMMA_SLOT) = stateGammaG /\
+W256.to_uint (mload m STATE_GAMMA_LOOKUP_SLOT) = stateGammaLookupG /\
+W256.to_uint (mload m STATE_Z_SLOT) = stateZG /\
+W256.to_uint (mload m PROOF_PUBLIC_INPUT) = proofPublicInputG /\
+W256.to_uint (mload m PROOF_COPY_PERMUTATION_POLYS_0_OPENING_AT_Z_SLOT) = proofCopyPermutationPolys0OpeningAtZG /\
+W256.to_uint (mload m PROOF_COPY_PERMUTATION_POLYS_1_OPENING_AT_Z_SLOT) = proofCopyPermutationPolys1OpeningAtZG /\
+W256.to_uint (mload m PROOF_COPY_PERMUTATION_POLYS_2_OPENING_AT_Z_SLOT) = proofCopyPermutationPolys2OpeningAtZG /\
+W256.to_uint (mload m PROOF_STATE_POLYS_0_OPENING_AT_Z_SLOT) = proofStatePolys0OpeningAtZG /\
+W256.to_uint (mload m PROOF_STATE_POLYS_1_OPENING_AT_Z_SLOT) = proofStatePolys1OpeningAtZG /\
+W256.to_uint (mload m PROOF_STATE_POLYS_2_OPENING_AT_Z_SLOT) = proofStatePolys2OpeningAtZG /\
+W256.to_uint (mload m PROOF_STATE_POLYS_3_OPENING_AT_Z_SLOT) = proofStatePolys3OpeningAtZG /\
+W256.to_uint (mload m PROOF_LOOKUP_S_POLY_OPENING_AT_Z_OMEGA_SLOT) = proofLookupSPolyOpeningAtZOmegaG /\
+W256.to_uint (mload m PROOF_LOOKUP_GRAND_PRODUCT_OPENING_AT_Z_OMEGA_SLOT) = proofLookupGrandProductOpeningAtZOmegaG /\
+W256.to_uint (mload m PROOF_GATE_SELECTORS_0_OPENING_AT_Z_SLOT) = proofGateSelectors0OpeningAtZG /\
+W256.to_uint (mload m PROOF_LINEARISATION_POLY_OPENING_AT_Z_SLOT) = proofLinearisationPolyOpeningAtZG /\
+W256.to_uint (mload m PROOF_COPY_PERMUTATION_GRAND_PRODUCT_OPENING_AT_Z_OMEGA_SLOT) = proofCopyPermutationGrandProductOpeningAtZOmegaG /\
+W256.to_uint (mload m STATE_Z_IN_DOMAIN_SIZE) = stateZInDomainSizeG /\
+W256.to_uint (mload m PROOF_QUOTIENT_POLY_OPENING_AT_Z_SLOT) = proofQuotientPolyOpeningAtZG /\
+!Primops.reverted{1} /\
+    to_uint alpha{1} = stateAlpha{2} /\
+    a2 = statePowerOfAlpha2{2} /\
+    a3 = statePowerOfAlpha3{2} /\
+    a4 = statePowerOfAlpha4{2} /\
+    a5 = statePowerOfAlpha5{2} /\
+    statePowerOfAlpha2{2} = (stateAlpha{2} * stateAlpha{2}) %% Constants.R /\
+    statePowerOfAlpha3{2} = (statePowerOfAlpha2{2} * stateAlpha{2}) %% Constants.R /\
+    statePowerOfAlpha4{2} = (statePowerOfAlpha3{2} * stateAlpha{2}) %% Constants.R /\
+    statePowerOfAlpha5{2} = (statePowerOfAlpha4{2} * stateAlpha{2}) %% Constants.R /\
+    to_uint currentAlpha{1} = statePowerOfAlpha5{2} /\
+    Primops.memory{1} = m5
+).
+call{1} (ConcretePrimops.mstore_pspec m4 STATE_POWER_OF_ALPHA_5_SLOT (W256.of_int a5)).
+skip. progress. smt(@W256 @Utils). 
 
-    
+seq 1 1: (
+(stateAlpha{2}, stateBeta{2}, stateBetaLookup{2}, stateGamma{2},
+ stateGammaLookup{2}, stateZ{2}, proofPublicInput{2},
+ proofCopyPermutationPolys0OpeningAtZ{2},
+ proofCopyPermutationPolys1OpeningAtZ{2},
+ proofCopyPermutationPolys2OpeningAtZ{2}, proofStatePolys0OpeningAtZ{2},
+ proofStatePolys1OpeningAtZ{2}, proofStatePolys2OpeningAtZ{2},
+ proofStatePolys3OpeningAtZ{2}, proofLookupSPolyOpeningAtZOmega{2},
+ proofLookupGrandProductOpeningAtZOmega{2},
+ proofGateSelectors0OpeningAtZ{2}, proofLinearisationPolyOpeningAtZ{2},
+ proofCopyPermutationGrandProductOpeningAtZOmega{2},
+ stateZInDomainSize{2}, proofQuotientPolyOpeningAtZ{2}) =
+(stateAlphaG, stateBetaG, stateBetaLookupG, stateGammaG,
+ stateGammaLookupG, stateZG, proofPublicInputG,
+ proofCopyPermutationPolys0OpeningAtZG,
+ proofCopyPermutationPolys1OpeningAtZG,
+ proofCopyPermutationPolys2OpeningAtZG, proofStatePolys0OpeningAtZG,
+ proofStatePolys1OpeningAtZG, proofStatePolys2OpeningAtZG,
+ proofStatePolys3OpeningAtZG, proofLookupSPolyOpeningAtZOmegaG,
+ proofLookupGrandProductOpeningAtZOmegaG, proofGateSelectors0OpeningAtZG,
+ proofLinearisationPolyOpeningAtZG,
+ proofCopyPermutationGrandProductOpeningAtZOmegaG, stateZInDomainSizeG,
+ proofQuotientPolyOpeningAtZG) /\
+W256.to_uint (mload m STATE_ALPHA_SLOT) = stateAlphaG /\
+W256.to_uint (mload m STATE_BETA_SLOT) = stateBetaG /\
+W256.to_uint (mload m STATE_BETA_LOOKUP_SLOT) = stateBetaLookupG /\
+W256.to_uint (mload m STATE_GAMMA_SLOT) = stateGammaG /\
+W256.to_uint (mload m STATE_GAMMA_LOOKUP_SLOT) = stateGammaLookupG /\
+W256.to_uint (mload m STATE_Z_SLOT) = stateZG /\
+W256.to_uint (mload m PROOF_PUBLIC_INPUT) = proofPublicInputG /\
+W256.to_uint (mload m PROOF_COPY_PERMUTATION_POLYS_0_OPENING_AT_Z_SLOT) = proofCopyPermutationPolys0OpeningAtZG /\
+W256.to_uint (mload m PROOF_COPY_PERMUTATION_POLYS_1_OPENING_AT_Z_SLOT) = proofCopyPermutationPolys1OpeningAtZG /\
+W256.to_uint (mload m PROOF_COPY_PERMUTATION_POLYS_2_OPENING_AT_Z_SLOT) = proofCopyPermutationPolys2OpeningAtZG /\
+W256.to_uint (mload m PROOF_STATE_POLYS_0_OPENING_AT_Z_SLOT) = proofStatePolys0OpeningAtZG /\
+W256.to_uint (mload m PROOF_STATE_POLYS_1_OPENING_AT_Z_SLOT) = proofStatePolys1OpeningAtZG /\
+W256.to_uint (mload m PROOF_STATE_POLYS_2_OPENING_AT_Z_SLOT) = proofStatePolys2OpeningAtZG /\
+W256.to_uint (mload m PROOF_STATE_POLYS_3_OPENING_AT_Z_SLOT) = proofStatePolys3OpeningAtZG /\
+W256.to_uint (mload m PROOF_LOOKUP_S_POLY_OPENING_AT_Z_OMEGA_SLOT) = proofLookupSPolyOpeningAtZOmegaG /\
+W256.to_uint (mload m PROOF_LOOKUP_GRAND_PRODUCT_OPENING_AT_Z_OMEGA_SLOT) = proofLookupGrandProductOpeningAtZOmegaG /\
+W256.to_uint (mload m PROOF_GATE_SELECTORS_0_OPENING_AT_Z_SLOT) = proofGateSelectors0OpeningAtZG /\
+W256.to_uint (mload m PROOF_LINEARISATION_POLY_OPENING_AT_Z_SLOT) = proofLinearisationPolyOpeningAtZG /\
+W256.to_uint (mload m PROOF_COPY_PERMUTATION_GRAND_PRODUCT_OPENING_AT_Z_OMEGA_SLOT) = proofCopyPermutationGrandProductOpeningAtZOmegaG /\
+W256.to_uint (mload m STATE_Z_IN_DOMAIN_SIZE) = stateZInDomainSizeG /\
+W256.to_uint (mload m PROOF_QUOTIENT_POLY_OPENING_AT_Z_SLOT) = proofQuotientPolyOpeningAtZG /\
+!Primops.reverted{1} /\
+    to_uint alpha{1} = stateAlpha{2} /\
+    a2 = statePowerOfAlpha2{2} /\
+    a3 = statePowerOfAlpha3{2} /\
+    a4 = statePowerOfAlpha4{2} /\
+    a5 = statePowerOfAlpha5{2} /\
+    statePowerOfAlpha2{2} = (stateAlpha{2} * stateAlpha{2}) %% Constants.R /\
+    statePowerOfAlpha3{2} = (statePowerOfAlpha2{2} * stateAlpha{2}) %% Constants.R /\
+    statePowerOfAlpha4{2} = (statePowerOfAlpha3{2} * stateAlpha{2}) %% Constants.R /\
+    statePowerOfAlpha5{2} = (statePowerOfAlpha4{2} * stateAlpha{2}) %% Constants.R /\
+    statePowerOfAlpha6{2} = (statePowerOfAlpha5{2} * stateAlpha{2}) %% Constants.R /\
+    to_uint currentAlpha{1} = statePowerOfAlpha6{2} /\
+    Primops.memory{1} = m5
+).
+wp. skip. rewrite /mulmod. progress. smt(). rewrite H1 -H0.
+rewrite W256.to_uint_small. progress. smt(@W256 @Utils). smt(@W256 @Utils).
+rewrite W256.to_uint_small. progress. smt(@W256 @Utils).
+exists* statePowerOfAlpha6{2}. elim*=> a6.
+pose m6 := store m5 STATE_POWER_OF_ALPHA_6_SLOT (W256.of_int a6).
+seq 1 0: (
+(stateAlpha{2}, stateBeta{2}, stateBetaLookup{2}, stateGamma{2},
+ stateGammaLookup{2}, stateZ{2}, proofPublicInput{2},
+ proofCopyPermutationPolys0OpeningAtZ{2},
+ proofCopyPermutationPolys1OpeningAtZ{2},
+ proofCopyPermutationPolys2OpeningAtZ{2}, proofStatePolys0OpeningAtZ{2},
+ proofStatePolys1OpeningAtZ{2}, proofStatePolys2OpeningAtZ{2},
+ proofStatePolys3OpeningAtZ{2}, proofLookupSPolyOpeningAtZOmega{2},
+ proofLookupGrandProductOpeningAtZOmega{2},
+ proofGateSelectors0OpeningAtZ{2}, proofLinearisationPolyOpeningAtZ{2},
+ proofCopyPermutationGrandProductOpeningAtZOmega{2},
+ stateZInDomainSize{2}, proofQuotientPolyOpeningAtZ{2}) =
+(stateAlphaG, stateBetaG, stateBetaLookupG, stateGammaG,
+ stateGammaLookupG, stateZG, proofPublicInputG,
+ proofCopyPermutationPolys0OpeningAtZG,
+ proofCopyPermutationPolys1OpeningAtZG,
+ proofCopyPermutationPolys2OpeningAtZG, proofStatePolys0OpeningAtZG,
+ proofStatePolys1OpeningAtZG, proofStatePolys2OpeningAtZG,
+ proofStatePolys3OpeningAtZG, proofLookupSPolyOpeningAtZOmegaG,
+ proofLookupGrandProductOpeningAtZOmegaG, proofGateSelectors0OpeningAtZG,
+ proofLinearisationPolyOpeningAtZG,
+ proofCopyPermutationGrandProductOpeningAtZOmegaG, stateZInDomainSizeG,
+ proofQuotientPolyOpeningAtZG) /\
+W256.to_uint (mload m STATE_ALPHA_SLOT) = stateAlphaG /\
+W256.to_uint (mload m STATE_BETA_SLOT) = stateBetaG /\
+W256.to_uint (mload m STATE_BETA_LOOKUP_SLOT) = stateBetaLookupG /\
+W256.to_uint (mload m STATE_GAMMA_SLOT) = stateGammaG /\
+W256.to_uint (mload m STATE_GAMMA_LOOKUP_SLOT) = stateGammaLookupG /\
+W256.to_uint (mload m STATE_Z_SLOT) = stateZG /\
+W256.to_uint (mload m PROOF_PUBLIC_INPUT) = proofPublicInputG /\
+W256.to_uint (mload m PROOF_COPY_PERMUTATION_POLYS_0_OPENING_AT_Z_SLOT) = proofCopyPermutationPolys0OpeningAtZG /\
+W256.to_uint (mload m PROOF_COPY_PERMUTATION_POLYS_1_OPENING_AT_Z_SLOT) = proofCopyPermutationPolys1OpeningAtZG /\
+W256.to_uint (mload m PROOF_COPY_PERMUTATION_POLYS_2_OPENING_AT_Z_SLOT) = proofCopyPermutationPolys2OpeningAtZG /\
+W256.to_uint (mload m PROOF_STATE_POLYS_0_OPENING_AT_Z_SLOT) = proofStatePolys0OpeningAtZG /\
+W256.to_uint (mload m PROOF_STATE_POLYS_1_OPENING_AT_Z_SLOT) = proofStatePolys1OpeningAtZG /\
+W256.to_uint (mload m PROOF_STATE_POLYS_2_OPENING_AT_Z_SLOT) = proofStatePolys2OpeningAtZG /\
+W256.to_uint (mload m PROOF_STATE_POLYS_3_OPENING_AT_Z_SLOT) = proofStatePolys3OpeningAtZG /\
+W256.to_uint (mload m PROOF_LOOKUP_S_POLY_OPENING_AT_Z_OMEGA_SLOT) = proofLookupSPolyOpeningAtZOmegaG /\
+W256.to_uint (mload m PROOF_LOOKUP_GRAND_PRODUCT_OPENING_AT_Z_OMEGA_SLOT) = proofLookupGrandProductOpeningAtZOmegaG /\
+W256.to_uint (mload m PROOF_GATE_SELECTORS_0_OPENING_AT_Z_SLOT) = proofGateSelectors0OpeningAtZG /\
+W256.to_uint (mload m PROOF_LINEARISATION_POLY_OPENING_AT_Z_SLOT) = proofLinearisationPolyOpeningAtZG /\
+W256.to_uint (mload m PROOF_COPY_PERMUTATION_GRAND_PRODUCT_OPENING_AT_Z_OMEGA_SLOT) = proofCopyPermutationGrandProductOpeningAtZOmegaG /\
+W256.to_uint (mload m STATE_Z_IN_DOMAIN_SIZE) = stateZInDomainSizeG /\
+W256.to_uint (mload m PROOF_QUOTIENT_POLY_OPENING_AT_Z_SLOT) = proofQuotientPolyOpeningAtZG /\
+!Primops.reverted{1} /\
+    to_uint alpha{1} = stateAlpha{2} /\
+    a2 = statePowerOfAlpha2{2} /\
+    a3 = statePowerOfAlpha3{2} /\
+    a4 = statePowerOfAlpha4{2} /\
+    a5 = statePowerOfAlpha5{2} /\
+    a6 = statePowerOfAlpha6{2} /\
+    statePowerOfAlpha2{2} = (stateAlpha{2} * stateAlpha{2}) %% Constants.R /\
+    statePowerOfAlpha3{2} = (statePowerOfAlpha2{2} * stateAlpha{2}) %% Constants.R /\
+    statePowerOfAlpha4{2} = (statePowerOfAlpha3{2} * stateAlpha{2}) %% Constants.R /\
+    statePowerOfAlpha5{2} = (statePowerOfAlpha4{2} * stateAlpha{2}) %% Constants.R /\
+    statePowerOfAlpha6{2} = (statePowerOfAlpha5{2} * stateAlpha{2}) %% Constants.R /\
+    to_uint currentAlpha{1} = statePowerOfAlpha6{2} /\
+    Primops.memory{1} = m6
+).
+call{1} (ConcretePrimops.mstore_pspec m5 STATE_POWER_OF_ALPHA_6_SLOT (W256.of_int a6)).
+skip. progress. smt(@W256 @Utils).
+
+seq 1 1: (
+(stateAlpha{2}, stateBeta{2}, stateBetaLookup{2}, stateGamma{2},
+ stateGammaLookup{2}, stateZ{2}, proofPublicInput{2},
+ proofCopyPermutationPolys0OpeningAtZ{2},
+ proofCopyPermutationPolys1OpeningAtZ{2},
+ proofCopyPermutationPolys2OpeningAtZ{2}, proofStatePolys0OpeningAtZ{2},
+ proofStatePolys1OpeningAtZ{2}, proofStatePolys2OpeningAtZ{2},
+ proofStatePolys3OpeningAtZ{2}, proofLookupSPolyOpeningAtZOmega{2},
+ proofLookupGrandProductOpeningAtZOmega{2},
+ proofGateSelectors0OpeningAtZ{2}, proofLinearisationPolyOpeningAtZ{2},
+ proofCopyPermutationGrandProductOpeningAtZOmega{2},
+ stateZInDomainSize{2}, proofQuotientPolyOpeningAtZ{2}) =
+(stateAlphaG, stateBetaG, stateBetaLookupG, stateGammaG,
+ stateGammaLookupG, stateZG, proofPublicInputG,
+ proofCopyPermutationPolys0OpeningAtZG,
+ proofCopyPermutationPolys1OpeningAtZG,
+ proofCopyPermutationPolys2OpeningAtZG, proofStatePolys0OpeningAtZG,
+ proofStatePolys1OpeningAtZG, proofStatePolys2OpeningAtZG,
+ proofStatePolys3OpeningAtZG, proofLookupSPolyOpeningAtZOmegaG,
+ proofLookupGrandProductOpeningAtZOmegaG, proofGateSelectors0OpeningAtZG,
+ proofLinearisationPolyOpeningAtZG,
+ proofCopyPermutationGrandProductOpeningAtZOmegaG, stateZInDomainSizeG,
+ proofQuotientPolyOpeningAtZG) /\
+W256.to_uint (mload m STATE_ALPHA_SLOT) = stateAlphaG /\
+W256.to_uint (mload m STATE_BETA_SLOT) = stateBetaG /\
+W256.to_uint (mload m STATE_BETA_LOOKUP_SLOT) = stateBetaLookupG /\
+W256.to_uint (mload m STATE_GAMMA_SLOT) = stateGammaG /\
+W256.to_uint (mload m STATE_GAMMA_LOOKUP_SLOT) = stateGammaLookupG /\
+W256.to_uint (mload m STATE_Z_SLOT) = stateZG /\
+W256.to_uint (mload m PROOF_PUBLIC_INPUT) = proofPublicInputG /\
+W256.to_uint (mload m PROOF_COPY_PERMUTATION_POLYS_0_OPENING_AT_Z_SLOT) = proofCopyPermutationPolys0OpeningAtZG /\
+W256.to_uint (mload m PROOF_COPY_PERMUTATION_POLYS_1_OPENING_AT_Z_SLOT) = proofCopyPermutationPolys1OpeningAtZG /\
+W256.to_uint (mload m PROOF_COPY_PERMUTATION_POLYS_2_OPENING_AT_Z_SLOT) = proofCopyPermutationPolys2OpeningAtZG /\
+W256.to_uint (mload m PROOF_STATE_POLYS_0_OPENING_AT_Z_SLOT) = proofStatePolys0OpeningAtZG /\
+W256.to_uint (mload m PROOF_STATE_POLYS_1_OPENING_AT_Z_SLOT) = proofStatePolys1OpeningAtZG /\
+W256.to_uint (mload m PROOF_STATE_POLYS_2_OPENING_AT_Z_SLOT) = proofStatePolys2OpeningAtZG /\
+W256.to_uint (mload m PROOF_STATE_POLYS_3_OPENING_AT_Z_SLOT) = proofStatePolys3OpeningAtZG /\
+W256.to_uint (mload m PROOF_LOOKUP_S_POLY_OPENING_AT_Z_OMEGA_SLOT) = proofLookupSPolyOpeningAtZOmegaG /\
+W256.to_uint (mload m PROOF_LOOKUP_GRAND_PRODUCT_OPENING_AT_Z_OMEGA_SLOT) = proofLookupGrandProductOpeningAtZOmegaG /\
+W256.to_uint (mload m PROOF_GATE_SELECTORS_0_OPENING_AT_Z_SLOT) = proofGateSelectors0OpeningAtZG /\
+W256.to_uint (mload m PROOF_LINEARISATION_POLY_OPENING_AT_Z_SLOT) = proofLinearisationPolyOpeningAtZG /\
+W256.to_uint (mload m PROOF_COPY_PERMUTATION_GRAND_PRODUCT_OPENING_AT_Z_OMEGA_SLOT) = proofCopyPermutationGrandProductOpeningAtZOmegaG /\
+W256.to_uint (mload m STATE_Z_IN_DOMAIN_SIZE) = stateZInDomainSizeG /\
+W256.to_uint (mload m PROOF_QUOTIENT_POLY_OPENING_AT_Z_SLOT) = proofQuotientPolyOpeningAtZG /\
+!Primops.reverted{1} /\
+    to_uint alpha{1} = stateAlpha{2} /\
+    a2 = statePowerOfAlpha2{2} /\
+    a3 = statePowerOfAlpha3{2} /\
+    a4 = statePowerOfAlpha4{2} /\
+    a5 = statePowerOfAlpha5{2} /\
+    a6 = statePowerOfAlpha6{2} /\
+    statePowerOfAlpha2{2} = (stateAlpha{2} * stateAlpha{2}) %% Constants.R /\
+    statePowerOfAlpha3{2} = (statePowerOfAlpha2{2} * stateAlpha{2}) %% Constants.R /\
+    statePowerOfAlpha4{2} = (statePowerOfAlpha3{2} * stateAlpha{2}) %% Constants.R /\
+    statePowerOfAlpha5{2} = (statePowerOfAlpha4{2} * stateAlpha{2}) %% Constants.R /\
+    statePowerOfAlpha6{2} = (statePowerOfAlpha5{2} * stateAlpha{2}) %% Constants.R /\
+    statePowerOfAlpha7{2} = (statePowerOfAlpha6{2} * stateAlpha{2}) %% Constants.R /\
+    to_uint currentAlpha{1} = statePowerOfAlpha7{2} /\
+    Primops.memory{1} = m6
+).
+wp. skip. rewrite /mulmod. progress. smt(). rewrite H1 -H0.
+rewrite W256.to_uint_small. progress. smt(@W256 @Utils). smt(@W256 @Utils).
+rewrite W256.to_uint_small. progress. smt(@W256 @Utils).
+exists* statePowerOfAlpha7{2}. elim*=> a7.
+pose m7 := store m6 STATE_POWER_OF_ALPHA_7_SLOT (W256.of_int a7).
+seq 1 0: (
+(stateAlpha{2}, stateBeta{2}, stateBetaLookup{2}, stateGamma{2},
+ stateGammaLookup{2}, stateZ{2}, proofPublicInput{2},
+ proofCopyPermutationPolys0OpeningAtZ{2},
+ proofCopyPermutationPolys1OpeningAtZ{2},
+ proofCopyPermutationPolys2OpeningAtZ{2}, proofStatePolys0OpeningAtZ{2},
+ proofStatePolys1OpeningAtZ{2}, proofStatePolys2OpeningAtZ{2},
+ proofStatePolys3OpeningAtZ{2}, proofLookupSPolyOpeningAtZOmega{2},
+ proofLookupGrandProductOpeningAtZOmega{2},
+ proofGateSelectors0OpeningAtZ{2}, proofLinearisationPolyOpeningAtZ{2},
+ proofCopyPermutationGrandProductOpeningAtZOmega{2},
+ stateZInDomainSize{2}, proofQuotientPolyOpeningAtZ{2}) =
+(stateAlphaG, stateBetaG, stateBetaLookupG, stateGammaG,
+ stateGammaLookupG, stateZG, proofPublicInputG,
+ proofCopyPermutationPolys0OpeningAtZG,
+ proofCopyPermutationPolys1OpeningAtZG,
+ proofCopyPermutationPolys2OpeningAtZG, proofStatePolys0OpeningAtZG,
+ proofStatePolys1OpeningAtZG, proofStatePolys2OpeningAtZG,
+ proofStatePolys3OpeningAtZG, proofLookupSPolyOpeningAtZOmegaG,
+ proofLookupGrandProductOpeningAtZOmegaG, proofGateSelectors0OpeningAtZG,
+ proofLinearisationPolyOpeningAtZG,
+ proofCopyPermutationGrandProductOpeningAtZOmegaG, stateZInDomainSizeG,
+ proofQuotientPolyOpeningAtZG) /\
+W256.to_uint (mload m STATE_ALPHA_SLOT) = stateAlphaG /\
+W256.to_uint (mload m STATE_BETA_SLOT) = stateBetaG /\
+W256.to_uint (mload m STATE_BETA_LOOKUP_SLOT) = stateBetaLookupG /\
+W256.to_uint (mload m STATE_GAMMA_SLOT) = stateGammaG /\
+W256.to_uint (mload m STATE_GAMMA_LOOKUP_SLOT) = stateGammaLookupG /\
+W256.to_uint (mload m STATE_Z_SLOT) = stateZG /\
+W256.to_uint (mload m PROOF_PUBLIC_INPUT) = proofPublicInputG /\
+W256.to_uint (mload m PROOF_COPY_PERMUTATION_POLYS_0_OPENING_AT_Z_SLOT) = proofCopyPermutationPolys0OpeningAtZG /\
+W256.to_uint (mload m PROOF_COPY_PERMUTATION_POLYS_1_OPENING_AT_Z_SLOT) = proofCopyPermutationPolys1OpeningAtZG /\
+W256.to_uint (mload m PROOF_COPY_PERMUTATION_POLYS_2_OPENING_AT_Z_SLOT) = proofCopyPermutationPolys2OpeningAtZG /\
+W256.to_uint (mload m PROOF_STATE_POLYS_0_OPENING_AT_Z_SLOT) = proofStatePolys0OpeningAtZG /\
+W256.to_uint (mload m PROOF_STATE_POLYS_1_OPENING_AT_Z_SLOT) = proofStatePolys1OpeningAtZG /\
+W256.to_uint (mload m PROOF_STATE_POLYS_2_OPENING_AT_Z_SLOT) = proofStatePolys2OpeningAtZG /\
+W256.to_uint (mload m PROOF_STATE_POLYS_3_OPENING_AT_Z_SLOT) = proofStatePolys3OpeningAtZG /\
+W256.to_uint (mload m PROOF_LOOKUP_S_POLY_OPENING_AT_Z_OMEGA_SLOT) = proofLookupSPolyOpeningAtZOmegaG /\
+W256.to_uint (mload m PROOF_LOOKUP_GRAND_PRODUCT_OPENING_AT_Z_OMEGA_SLOT) = proofLookupGrandProductOpeningAtZOmegaG /\
+W256.to_uint (mload m PROOF_GATE_SELECTORS_0_OPENING_AT_Z_SLOT) = proofGateSelectors0OpeningAtZG /\
+W256.to_uint (mload m PROOF_LINEARISATION_POLY_OPENING_AT_Z_SLOT) = proofLinearisationPolyOpeningAtZG /\
+W256.to_uint (mload m PROOF_COPY_PERMUTATION_GRAND_PRODUCT_OPENING_AT_Z_OMEGA_SLOT) = proofCopyPermutationGrandProductOpeningAtZOmegaG /\
+W256.to_uint (mload m STATE_Z_IN_DOMAIN_SIZE) = stateZInDomainSizeG /\
+W256.to_uint (mload m PROOF_QUOTIENT_POLY_OPENING_AT_Z_SLOT) = proofQuotientPolyOpeningAtZG /\
+!Primops.reverted{1} /\
+    to_uint alpha{1} = stateAlpha{2} /\
+    a2 = statePowerOfAlpha2{2} /\
+    a3 = statePowerOfAlpha3{2} /\
+    a4 = statePowerOfAlpha4{2} /\
+    a5 = statePowerOfAlpha5{2} /\
+    a6 = statePowerOfAlpha6{2} /\
+    a7 = statePowerOfAlpha7{2} /\
+    statePowerOfAlpha2{2} = (stateAlpha{2} * stateAlpha{2}) %% Constants.R /\
+    statePowerOfAlpha3{2} = (statePowerOfAlpha2{2} * stateAlpha{2}) %% Constants.R /\
+    statePowerOfAlpha4{2} = (statePowerOfAlpha3{2} * stateAlpha{2}) %% Constants.R /\
+    statePowerOfAlpha5{2} = (statePowerOfAlpha4{2} * stateAlpha{2}) %% Constants.R /\
+    statePowerOfAlpha6{2} = (statePowerOfAlpha5{2} * stateAlpha{2}) %% Constants.R /\
+    statePowerOfAlpha7{2} = (statePowerOfAlpha6{2} * stateAlpha{2}) %% Constants.R /\
+    to_uint currentAlpha{1} = statePowerOfAlpha7{2} /\
+    Primops.memory{1} = m7
+).
+call{1} (ConcretePrimops.mstore_pspec m6 STATE_POWER_OF_ALPHA_7_SLOT (W256.of_int a7)).
+skip. progress. smt(@W256 @Utils).
+
+seq 1 1: (
+(stateAlpha{2}, stateBeta{2}, stateBetaLookup{2}, stateGamma{2},
+ stateGammaLookup{2}, stateZ{2}, proofPublicInput{2},
+ proofCopyPermutationPolys0OpeningAtZ{2},
+ proofCopyPermutationPolys1OpeningAtZ{2},
+ proofCopyPermutationPolys2OpeningAtZ{2}, proofStatePolys0OpeningAtZ{2},
+ proofStatePolys1OpeningAtZ{2}, proofStatePolys2OpeningAtZ{2},
+ proofStatePolys3OpeningAtZ{2}, proofLookupSPolyOpeningAtZOmega{2},
+ proofLookupGrandProductOpeningAtZOmega{2},
+ proofGateSelectors0OpeningAtZ{2}, proofLinearisationPolyOpeningAtZ{2},
+ proofCopyPermutationGrandProductOpeningAtZOmega{2},
+ stateZInDomainSize{2}, proofQuotientPolyOpeningAtZ{2}) =
+(stateAlphaG, stateBetaG, stateBetaLookupG, stateGammaG,
+ stateGammaLookupG, stateZG, proofPublicInputG,
+ proofCopyPermutationPolys0OpeningAtZG,
+ proofCopyPermutationPolys1OpeningAtZG,
+ proofCopyPermutationPolys2OpeningAtZG, proofStatePolys0OpeningAtZG,
+ proofStatePolys1OpeningAtZG, proofStatePolys2OpeningAtZG,
+ proofStatePolys3OpeningAtZG, proofLookupSPolyOpeningAtZOmegaG,
+ proofLookupGrandProductOpeningAtZOmegaG, proofGateSelectors0OpeningAtZG,
+ proofLinearisationPolyOpeningAtZG,
+ proofCopyPermutationGrandProductOpeningAtZOmegaG, stateZInDomainSizeG,
+ proofQuotientPolyOpeningAtZG) /\
+W256.to_uint (mload m STATE_ALPHA_SLOT) = stateAlphaG /\
+W256.to_uint (mload m STATE_BETA_SLOT) = stateBetaG /\
+W256.to_uint (mload m STATE_BETA_LOOKUP_SLOT) = stateBetaLookupG /\
+W256.to_uint (mload m STATE_GAMMA_SLOT) = stateGammaG /\
+W256.to_uint (mload m STATE_GAMMA_LOOKUP_SLOT) = stateGammaLookupG /\
+W256.to_uint (mload m STATE_Z_SLOT) = stateZG /\
+W256.to_uint (mload m PROOF_PUBLIC_INPUT) = proofPublicInputG /\
+W256.to_uint (mload m PROOF_COPY_PERMUTATION_POLYS_0_OPENING_AT_Z_SLOT) = proofCopyPermutationPolys0OpeningAtZG /\
+W256.to_uint (mload m PROOF_COPY_PERMUTATION_POLYS_1_OPENING_AT_Z_SLOT) = proofCopyPermutationPolys1OpeningAtZG /\
+W256.to_uint (mload m PROOF_COPY_PERMUTATION_POLYS_2_OPENING_AT_Z_SLOT) = proofCopyPermutationPolys2OpeningAtZG /\
+W256.to_uint (mload m PROOF_STATE_POLYS_0_OPENING_AT_Z_SLOT) = proofStatePolys0OpeningAtZG /\
+W256.to_uint (mload m PROOF_STATE_POLYS_1_OPENING_AT_Z_SLOT) = proofStatePolys1OpeningAtZG /\
+W256.to_uint (mload m PROOF_STATE_POLYS_2_OPENING_AT_Z_SLOT) = proofStatePolys2OpeningAtZG /\
+W256.to_uint (mload m PROOF_STATE_POLYS_3_OPENING_AT_Z_SLOT) = proofStatePolys3OpeningAtZG /\
+W256.to_uint (mload m PROOF_LOOKUP_S_POLY_OPENING_AT_Z_OMEGA_SLOT) = proofLookupSPolyOpeningAtZOmegaG /\
+W256.to_uint (mload m PROOF_LOOKUP_GRAND_PRODUCT_OPENING_AT_Z_OMEGA_SLOT) = proofLookupGrandProductOpeningAtZOmegaG /\
+W256.to_uint (mload m PROOF_GATE_SELECTORS_0_OPENING_AT_Z_SLOT) = proofGateSelectors0OpeningAtZG /\
+W256.to_uint (mload m PROOF_LINEARISATION_POLY_OPENING_AT_Z_SLOT) = proofLinearisationPolyOpeningAtZG /\
+W256.to_uint (mload m PROOF_COPY_PERMUTATION_GRAND_PRODUCT_OPENING_AT_Z_OMEGA_SLOT) = proofCopyPermutationGrandProductOpeningAtZOmegaG /\
+W256.to_uint (mload m STATE_Z_IN_DOMAIN_SIZE) = stateZInDomainSizeG /\
+W256.to_uint (mload m PROOF_QUOTIENT_POLY_OPENING_AT_Z_SLOT) = proofQuotientPolyOpeningAtZG /\
+!Primops.reverted{1} /\
+    to_uint alpha{1} = stateAlpha{2} /\
+    a2 = statePowerOfAlpha2{2} /\
+    a3 = statePowerOfAlpha3{2} /\
+    a4 = statePowerOfAlpha4{2} /\
+    a5 = statePowerOfAlpha5{2} /\
+    a6 = statePowerOfAlpha6{2} /\
+    a7 = statePowerOfAlpha7{2} /\
+    statePowerOfAlpha2{2} = (stateAlpha{2} * stateAlpha{2}) %% Constants.R /\
+    statePowerOfAlpha3{2} = (statePowerOfAlpha2{2} * stateAlpha{2}) %% Constants.R /\
+    statePowerOfAlpha4{2} = (statePowerOfAlpha3{2} * stateAlpha{2}) %% Constants.R /\
+    statePowerOfAlpha5{2} = (statePowerOfAlpha4{2} * stateAlpha{2}) %% Constants.R /\
+    statePowerOfAlpha6{2} = (statePowerOfAlpha5{2} * stateAlpha{2}) %% Constants.R /\
+    statePowerOfAlpha7{2} = (statePowerOfAlpha6{2} * stateAlpha{2}) %% Constants.R /\
+    statePowerOfAlpha8{2} = (statePowerOfAlpha7{2} * stateAlpha{2}) %% Constants.R /\
+    to_uint currentAlpha{1} = statePowerOfAlpha8{2} /\
+    Primops.memory{1} = m7
+).
+wp. skip. rewrite /mulmod. progress. smt(). rewrite H1 -H0.
+rewrite W256.to_uint_small. progress. smt(@W256 @Utils). smt(@W256 @Utils).
+rewrite W256.to_uint_small. progress. smt(@W256 @Utils).
+exists* statePowerOfAlpha8{2}. elim*=> a8.
+pose m8 := store m7 STATE_POWER_OF_ALPHA_8_SLOT (W256.of_int a8).
+seq 1 0: (
+(stateAlpha{2}, stateBeta{2}, stateBetaLookup{2}, stateGamma{2},
+ stateGammaLookup{2}, stateZ{2}, proofPublicInput{2},
+ proofCopyPermutationPolys0OpeningAtZ{2},
+ proofCopyPermutationPolys1OpeningAtZ{2},
+ proofCopyPermutationPolys2OpeningAtZ{2}, proofStatePolys0OpeningAtZ{2},
+ proofStatePolys1OpeningAtZ{2}, proofStatePolys2OpeningAtZ{2},
+ proofStatePolys3OpeningAtZ{2}, proofLookupSPolyOpeningAtZOmega{2},
+ proofLookupGrandProductOpeningAtZOmega{2},
+ proofGateSelectors0OpeningAtZ{2}, proofLinearisationPolyOpeningAtZ{2},
+ proofCopyPermutationGrandProductOpeningAtZOmega{2},
+ stateZInDomainSize{2}, proofQuotientPolyOpeningAtZ{2}) =
+(stateAlphaG, stateBetaG, stateBetaLookupG, stateGammaG,
+ stateGammaLookupG, stateZG, proofPublicInputG,
+ proofCopyPermutationPolys0OpeningAtZG,
+ proofCopyPermutationPolys1OpeningAtZG,
+ proofCopyPermutationPolys2OpeningAtZG, proofStatePolys0OpeningAtZG,
+ proofStatePolys1OpeningAtZG, proofStatePolys2OpeningAtZG,
+ proofStatePolys3OpeningAtZG, proofLookupSPolyOpeningAtZOmegaG,
+ proofLookupGrandProductOpeningAtZOmegaG, proofGateSelectors0OpeningAtZG,
+ proofLinearisationPolyOpeningAtZG,
+ proofCopyPermutationGrandProductOpeningAtZOmegaG, stateZInDomainSizeG,
+ proofQuotientPolyOpeningAtZG) /\
+W256.to_uint (mload m STATE_ALPHA_SLOT) = stateAlphaG /\
+W256.to_uint (mload m STATE_BETA_SLOT) = stateBetaG /\
+W256.to_uint (mload m STATE_BETA_LOOKUP_SLOT) = stateBetaLookupG /\
+W256.to_uint (mload m STATE_GAMMA_SLOT) = stateGammaG /\
+W256.to_uint (mload m STATE_GAMMA_LOOKUP_SLOT) = stateGammaLookupG /\
+W256.to_uint (mload m STATE_Z_SLOT) = stateZG /\
+W256.to_uint (mload m PROOF_PUBLIC_INPUT) = proofPublicInputG /\
+W256.to_uint (mload m PROOF_COPY_PERMUTATION_POLYS_0_OPENING_AT_Z_SLOT) = proofCopyPermutationPolys0OpeningAtZG /\
+W256.to_uint (mload m PROOF_COPY_PERMUTATION_POLYS_1_OPENING_AT_Z_SLOT) = proofCopyPermutationPolys1OpeningAtZG /\
+W256.to_uint (mload m PROOF_COPY_PERMUTATION_POLYS_2_OPENING_AT_Z_SLOT) = proofCopyPermutationPolys2OpeningAtZG /\
+W256.to_uint (mload m PROOF_STATE_POLYS_0_OPENING_AT_Z_SLOT) = proofStatePolys0OpeningAtZG /\
+W256.to_uint (mload m PROOF_STATE_POLYS_1_OPENING_AT_Z_SLOT) = proofStatePolys1OpeningAtZG /\
+W256.to_uint (mload m PROOF_STATE_POLYS_2_OPENING_AT_Z_SLOT) = proofStatePolys2OpeningAtZG /\
+W256.to_uint (mload m PROOF_STATE_POLYS_3_OPENING_AT_Z_SLOT) = proofStatePolys3OpeningAtZG /\
+W256.to_uint (mload m PROOF_LOOKUP_S_POLY_OPENING_AT_Z_OMEGA_SLOT) = proofLookupSPolyOpeningAtZOmegaG /\
+W256.to_uint (mload m PROOF_LOOKUP_GRAND_PRODUCT_OPENING_AT_Z_OMEGA_SLOT) = proofLookupGrandProductOpeningAtZOmegaG /\
+W256.to_uint (mload m PROOF_GATE_SELECTORS_0_OPENING_AT_Z_SLOT) = proofGateSelectors0OpeningAtZG /\
+W256.to_uint (mload m PROOF_LINEARISATION_POLY_OPENING_AT_Z_SLOT) = proofLinearisationPolyOpeningAtZG /\
+W256.to_uint (mload m PROOF_COPY_PERMUTATION_GRAND_PRODUCT_OPENING_AT_Z_OMEGA_SLOT) = proofCopyPermutationGrandProductOpeningAtZOmegaG /\
+W256.to_uint (mload m STATE_Z_IN_DOMAIN_SIZE) = stateZInDomainSizeG /\
+W256.to_uint (mload m PROOF_QUOTIENT_POLY_OPENING_AT_Z_SLOT) = proofQuotientPolyOpeningAtZG /\
+!Primops.reverted{1} /\
+    to_uint alpha{1} = stateAlpha{2} /\
+    a2 = statePowerOfAlpha2{2} /\
+    a3 = statePowerOfAlpha3{2} /\
+    a4 = statePowerOfAlpha4{2} /\
+    a5 = statePowerOfAlpha5{2} /\
+    a6 = statePowerOfAlpha6{2} /\
+    a7 = statePowerOfAlpha7{2} /\
+    a8 = statePowerOfAlpha8{2} /\
+    statePowerOfAlpha2{2} = (stateAlpha{2} * stateAlpha{2}) %% Constants.R /\
+    statePowerOfAlpha3{2} = (statePowerOfAlpha2{2} * stateAlpha{2}) %% Constants.R /\
+    statePowerOfAlpha4{2} = (statePowerOfAlpha3{2} * stateAlpha{2}) %% Constants.R /\
+    statePowerOfAlpha5{2} = (statePowerOfAlpha4{2} * stateAlpha{2}) %% Constants.R /\
+    statePowerOfAlpha6{2} = (statePowerOfAlpha5{2} * stateAlpha{2}) %% Constants.R /\
+    statePowerOfAlpha7{2} = (statePowerOfAlpha6{2} * stateAlpha{2}) %% Constants.R /\
+    statePowerOfAlpha8{2} = (statePowerOfAlpha7{2} * stateAlpha{2}) %% Constants.R /\
+    to_uint currentAlpha{1} = statePowerOfAlpha8{2} /\
+    Primops.memory{1} = m8
+).
+call{1} (ConcretePrimops.mstore_pspec m7 STATE_POWER_OF_ALPHA_8_SLOT (W256.of_int a8)).
+skip. progress. smt(@W256 @Utils).
+exists* stateAlpha{2}; elim*=> a.
+seq 0 0 :(
+(stateAlpha{2}, stateBeta{2}, stateBetaLookup{2}, stateGamma{2},
+ stateGammaLookup{2}, stateZ{2}, proofPublicInput{2},
+ proofCopyPermutationPolys0OpeningAtZ{2},
+ proofCopyPermutationPolys1OpeningAtZ{2},
+ proofCopyPermutationPolys2OpeningAtZ{2}, proofStatePolys0OpeningAtZ{2},
+ proofStatePolys1OpeningAtZ{2}, proofStatePolys2OpeningAtZ{2},
+ proofStatePolys3OpeningAtZ{2}, proofLookupSPolyOpeningAtZOmega{2},
+ proofLookupGrandProductOpeningAtZOmega{2},
+ proofGateSelectors0OpeningAtZ{2}, proofLinearisationPolyOpeningAtZ{2},
+ proofCopyPermutationGrandProductOpeningAtZOmega{2},
+ stateZInDomainSize{2}, proofQuotientPolyOpeningAtZ{2}) =
+(stateAlphaG, stateBetaG, stateBetaLookupG, stateGammaG,
+ stateGammaLookupG, stateZG, proofPublicInputG,
+ proofCopyPermutationPolys0OpeningAtZG,
+ proofCopyPermutationPolys1OpeningAtZG,
+ proofCopyPermutationPolys2OpeningAtZG, proofStatePolys0OpeningAtZG,
+ proofStatePolys1OpeningAtZG, proofStatePolys2OpeningAtZG,
+ proofStatePolys3OpeningAtZG, proofLookupSPolyOpeningAtZOmegaG,
+ proofLookupGrandProductOpeningAtZOmegaG, proofGateSelectors0OpeningAtZG,
+ proofLinearisationPolyOpeningAtZG,
+ proofCopyPermutationGrandProductOpeningAtZOmegaG, stateZInDomainSizeG,
+ proofQuotientPolyOpeningAtZG) /\
+W256.to_uint (mload m STATE_ALPHA_SLOT) = stateAlphaG /\
+W256.to_uint (mload m STATE_BETA_SLOT) = stateBetaG /\
+W256.to_uint (mload m STATE_BETA_LOOKUP_SLOT) = stateBetaLookupG /\
+W256.to_uint (mload m STATE_GAMMA_SLOT) = stateGammaG /\
+W256.to_uint (mload m STATE_GAMMA_LOOKUP_SLOT) = stateGammaLookupG /\
+W256.to_uint (mload m STATE_Z_SLOT) = stateZG /\
+W256.to_uint (mload m PROOF_PUBLIC_INPUT) = proofPublicInputG /\
+W256.to_uint (mload m PROOF_COPY_PERMUTATION_POLYS_0_OPENING_AT_Z_SLOT) = proofCopyPermutationPolys0OpeningAtZG /\
+W256.to_uint (mload m PROOF_COPY_PERMUTATION_POLYS_1_OPENING_AT_Z_SLOT) = proofCopyPermutationPolys1OpeningAtZG /\
+W256.to_uint (mload m PROOF_COPY_PERMUTATION_POLYS_2_OPENING_AT_Z_SLOT) = proofCopyPermutationPolys2OpeningAtZG /\
+W256.to_uint (mload m PROOF_STATE_POLYS_0_OPENING_AT_Z_SLOT) = proofStatePolys0OpeningAtZG /\
+W256.to_uint (mload m PROOF_STATE_POLYS_1_OPENING_AT_Z_SLOT) = proofStatePolys1OpeningAtZG /\
+W256.to_uint (mload m PROOF_STATE_POLYS_2_OPENING_AT_Z_SLOT) = proofStatePolys2OpeningAtZG /\
+W256.to_uint (mload m PROOF_STATE_POLYS_3_OPENING_AT_Z_SLOT) = proofStatePolys3OpeningAtZG /\
+W256.to_uint (mload m PROOF_LOOKUP_S_POLY_OPENING_AT_Z_OMEGA_SLOT) = proofLookupSPolyOpeningAtZOmegaG /\
+W256.to_uint (mload m PROOF_LOOKUP_GRAND_PRODUCT_OPENING_AT_Z_OMEGA_SLOT) = proofLookupGrandProductOpeningAtZOmegaG /\
+W256.to_uint (mload m PROOF_GATE_SELECTORS_0_OPENING_AT_Z_SLOT) = proofGateSelectors0OpeningAtZG /\
+W256.to_uint (mload m PROOF_LINEARISATION_POLY_OPENING_AT_Z_SLOT) = proofLinearisationPolyOpeningAtZG /\
+W256.to_uint (mload m PROOF_COPY_PERMUTATION_GRAND_PRODUCT_OPENING_AT_Z_OMEGA_SLOT) = proofCopyPermutationGrandProductOpeningAtZOmegaG /\
+W256.to_uint (mload m STATE_Z_IN_DOMAIN_SIZE) = stateZInDomainSizeG /\
+W256.to_uint (mload m PROOF_QUOTIENT_POLY_OPENING_AT_Z_SLOT) = proofQuotientPolyOpeningAtZG /\
+!Primops.reverted{1} /\
+    a = stateAlpha{2} /\
+    a2 = statePowerOfAlpha2{2} /\
+    a3 = statePowerOfAlpha3{2} /\
+    a4 = statePowerOfAlpha4{2} /\
+    a5 = statePowerOfAlpha5{2} /\
+    a6 = statePowerOfAlpha6{2} /\
+    a7 = statePowerOfAlpha7{2} /\
+    a8 = statePowerOfAlpha8{2} /\
+    statePowerOfAlpha2{2} = (stateAlpha{2}^2) %% Constants.R /\
+    statePowerOfAlpha3{2} = (stateAlpha{2}^3) %% Constants.R /\
+    statePowerOfAlpha4{2} = (stateAlpha{2}^4) %% Constants.R /\
+    statePowerOfAlpha5{2} = (stateAlpha{2}^5) %% Constants.R /\
+    statePowerOfAlpha6{2} = (stateAlpha{2}^6) %% Constants.R /\
+    statePowerOfAlpha7{2} = (stateAlpha{2}^7) %% Constants.R /\
+    statePowerOfAlpha8{2} = (stateAlpha{2}^8) %% Constants.R /\
+    Primops.memory{1} = m8
+).
+skip; progress; smt().
+
+seq 1 0 :(#pre /\ to_uint stateZ{1} = stateZ{2}).
+call{1} (ConcretePrimops.mload_pspec m8 STATE_Z_SLOT).
+skip; progress; rewrite /m8 /m7 /m6 /m5 /m4 /m3 /m2 /m1. 
+do 7! (rewrite load_store_diff;
+rewrite /STATE_Z_SLOT
+        /STATE_POWER_OF_ALPHA_8_SLOT
+        /STATE_POWER_OF_ALPHA_7_SLOT
+        /STATE_POWER_OF_ALPHA_6_SLOT
+        /STATE_POWER_OF_ALPHA_5_SLOT
+        /STATE_POWER_OF_ALPHA_4_SLOT
+        /STATE_POWER_OF_ALPHA_3_SLOT 
+        /STATE_POWER_OF_ALPHA_2_SLOT
+; try by progress).
+
+seq 1 1: (
+  (stateAlpha{2}, stateBeta{2}, stateBetaLookup{2}, stateGamma{2},
+    stateGammaLookup{2}, stateZ{2}, proofPublicInput{2},
+    proofCopyPermutationPolys0OpeningAtZ{2},
+    proofCopyPermutationPolys1OpeningAtZ{2},
+    proofCopyPermutationPolys2OpeningAtZ{2}, proofStatePolys0OpeningAtZ{2},
+    proofStatePolys1OpeningAtZ{2}, proofStatePolys2OpeningAtZ{2},
+    proofStatePolys3OpeningAtZ{2}, proofLookupSPolyOpeningAtZOmega{2},
+    proofLookupGrandProductOpeningAtZOmega{2},
+    proofGateSelectors0OpeningAtZ{2}, proofLinearisationPolyOpeningAtZ{2},
+    proofCopyPermutationGrandProductOpeningAtZOmega{2},
+    stateZInDomainSize{2}, proofQuotientPolyOpeningAtZ{2}) =
+   (stateAlphaG, stateBetaG, stateBetaLookupG, stateGammaG,
+    stateGammaLookupG, stateZG, proofPublicInputG,
+    proofCopyPermutationPolys0OpeningAtZG,
+    proofCopyPermutationPolys1OpeningAtZG,
+    proofCopyPermutationPolys2OpeningAtZG, proofStatePolys0OpeningAtZG,
+    proofStatePolys1OpeningAtZG, proofStatePolys2OpeningAtZG,
+    proofStatePolys3OpeningAtZG, proofLookupSPolyOpeningAtZOmegaG,
+    proofLookupGrandProductOpeningAtZOmegaG, proofGateSelectors0OpeningAtZG,
+    proofLinearisationPolyOpeningAtZG,
+    proofCopyPermutationGrandProductOpeningAtZOmegaG, stateZInDomainSizeG,
+    proofQuotientPolyOpeningAtZG) /\
+   to_uint (mload m STATE_ALPHA_SLOT) = stateAlphaG /\
+   to_uint (mload m STATE_BETA_SLOT) = stateBetaG /\
+   to_uint (mload m STATE_BETA_LOOKUP_SLOT) = stateBetaLookupG /\
+   to_uint (mload m STATE_GAMMA_SLOT) = stateGammaG /\
+   to_uint (mload m STATE_GAMMA_LOOKUP_SLOT) = stateGammaLookupG /\
+   to_uint (mload m STATE_Z_SLOT) = stateZG /\
+   to_uint (mload m PROOF_PUBLIC_INPUT) = proofPublicInputG /\
+   to_uint (mload m PROOF_COPY_PERMUTATION_POLYS_0_OPENING_AT_Z_SLOT) =
+   proofCopyPermutationPolys0OpeningAtZG /\
+   to_uint (mload m PROOF_COPY_PERMUTATION_POLYS_1_OPENING_AT_Z_SLOT) =
+   proofCopyPermutationPolys1OpeningAtZG /\
+   to_uint (mload m PROOF_COPY_PERMUTATION_POLYS_2_OPENING_AT_Z_SLOT) =
+   proofCopyPermutationPolys2OpeningAtZG /\
+   to_uint (mload m PROOF_STATE_POLYS_0_OPENING_AT_Z_SLOT) =
+   proofStatePolys0OpeningAtZG /\
+   to_uint (mload m PROOF_STATE_POLYS_1_OPENING_AT_Z_SLOT) =
+   proofStatePolys1OpeningAtZG /\
+   to_uint (mload m PROOF_STATE_POLYS_2_OPENING_AT_Z_SLOT) =
+   proofStatePolys2OpeningAtZG /\
+   to_uint (mload m PROOF_STATE_POLYS_3_OPENING_AT_Z_SLOT) =
+   proofStatePolys3OpeningAtZG /\
+   to_uint (mload m PROOF_LOOKUP_S_POLY_OPENING_AT_Z_OMEGA_SLOT) =
+   proofLookupSPolyOpeningAtZOmegaG /\
+   to_uint (mload m PROOF_LOOKUP_GRAND_PRODUCT_OPENING_AT_Z_OMEGA_SLOT) =
+   proofLookupGrandProductOpeningAtZOmegaG /\
+   to_uint (mload m PROOF_GATE_SELECTORS_0_OPENING_AT_Z_SLOT) =
+   proofGateSelectors0OpeningAtZG /\
+   to_uint (mload m PROOF_LINEARISATION_POLY_OPENING_AT_Z_SLOT) =
+   proofLinearisationPolyOpeningAtZG /\
+   to_uint
+     (mload m PROOF_COPY_PERMUTATION_GRAND_PRODUCT_OPENING_AT_Z_OMEGA_SLOT) =
+   proofCopyPermutationGrandProductOpeningAtZOmegaG /\
+   to_uint (mload m STATE_Z_IN_DOMAIN_SIZE) = stateZInDomainSizeG /\
+   to_uint (mload m PROOF_QUOTIENT_POLY_OPENING_AT_Z_SLOT) =
+   proofQuotientPolyOpeningAtZG /\
+   a = stateAlpha{2} /\
+   a2 = statePowerOfAlpha2{2} /\
+   a3 = statePowerOfAlpha3{2} /\
+   a4 = statePowerOfAlpha4{2} /\
+   a5 = statePowerOfAlpha5{2} /\
+   a6 = statePowerOfAlpha6{2} /\
+   a7 = statePowerOfAlpha7{2} /\
+   a8 = statePowerOfAlpha8{2} /\
+   statePowerOfAlpha2{2} = stateAlpha{2} ^ 2 %% Constants.R /\
+   statePowerOfAlpha3{2} = stateAlpha{2} ^ 3 %% Constants.R /\
+   statePowerOfAlpha4{2} = stateAlpha{2} ^ 4 %% Constants.R /\
+   statePowerOfAlpha5{2} = stateAlpha{2} ^ 5 %% Constants.R /\
+   statePowerOfAlpha6{2} = stateAlpha{2} ^ 6 %% Constants.R /\
+   statePowerOfAlpha7{2} = stateAlpha{2} ^ 7 %% Constants.R /\
+   statePowerOfAlpha8{2} = stateAlpha{2} ^ 8 %% Constants.R /\
+   to_uint stateZ{1} = stateZ{2} /\
+   ((!Primops.reverted{1} /\ ((stateZ{2}^Constants.DOMAIN_SIZE) - 1) %% Constants.R <> 0 /\
+      exists v1 v2 v3, Primops.memory{1} = lagrange_memory_footprint m8 v1 v2 v3 /\
+      elpodL0{2} = Some (W256.to_uint _12{1}) /\ 0 <= (W256.to_uint _12{1}) < Constants.R)
+      \/
+    (Primops.reverted{1} /\ ((stateZ{2}^Constants.DOMAIN_SIZE) - 1) %% Constants.R = 0 /\
+      elpodL0{2} = None)) 
+).
+call (evaluateLagrangePolyOutOfDomain_low_equiv_mid m8 W256.zero (W256.of_int stateZG)).
+skip. progress. smt(@W256). 
+
+(* First evaluateLagrangePolyOutOfDomain REVERT *)
+case (Primops.reverted{1}).
+seq 0 0: (stateZ{2} = stateZG /\ Primops.reverted{1} /\ ((stateZ{2}^Constants.DOMAIN_SIZE) - 1) %% Constants.R = 0 /\ elpodL0{2} = None).
+skip; progress; case H0; by progress.
+rcondt{2} 1. by progress.
+seq 1 1: (#pre /\ r{2} = None).
+wp. call{1} (ConcretePrimops.mstore_pspec_revert). skip. by progress.
+seq 1 0 : (#pre). call{1} (evaluateLagrangePolyOutOfDomain_pspec_revert); skip; by progress.
+seq 1 0 : (#pre). call{1} (ConcretePrimops.mstore_pspec_revert); skip; by progress.
+seq 1 0 : (#pre). call{1} (ConcretePrimops.mload_pspec_revert); skip; by progress.
+seq 1 0 : (#pre). call{1} (ConcretePrimops.mload_pspec_revert); skip; by progress.
+sp. seq 1 0 : (#pre). call{1} (ConcretePrimops.mload_pspec_revert); skip; by progress.
+sp. seq 1 0 : (#pre). call{1} (permutationQuotientContribution_pspec_revert); skip; by progress.
+sp. seq 1 0 : (#pre). call{1} (lookupQuotientContribution_pspec_revert); skip. progress. smt().
+sp. seq 1 0 : (#pre). call{1} (ConcretePrimops.mload_pspec_revert); skip; smt().
+sp. seq 1 0 : (#pre). call{1} (ConcretePrimops.mload_pspec_revert); skip; smt().
+sp. seq 1 0 : (#pre). call{1} (ConcretePrimops.mload_pspec_revert); skip; smt().
+sp. case (bool_of_uint256 (iszero (eq_uint256 lhs{1} result{1}))).
+rcondt{1} 1. by progress.
+call{1} (revertWithMessage_low_pspec). skip. by progress.
+rcondf{1} 1. by progress. skip. by progress.
+
+(* First evaluateLagrangePolyOutOfDomain NOT REVERT *)
+elim*. progress. pose m9 := lagrange_memory_footprint m8 v1 v2 v3.
+seq 0 0: (
+  (stateAlpha{2}, stateBeta{2}, stateBetaLookup{2}, stateGamma{2},
+    stateGammaLookup{2}, stateZ{2}, proofPublicInput{2},
+    proofCopyPermutationPolys0OpeningAtZ{2},
+    proofCopyPermutationPolys1OpeningAtZ{2},
+    proofCopyPermutationPolys2OpeningAtZ{2}, proofStatePolys0OpeningAtZ{2},
+    proofStatePolys1OpeningAtZ{2}, proofStatePolys2OpeningAtZ{2},
+    proofStatePolys3OpeningAtZ{2}, proofLookupSPolyOpeningAtZOmega{2},
+    proofLookupGrandProductOpeningAtZOmega{2},
+    proofGateSelectors0OpeningAtZ{2}, proofLinearisationPolyOpeningAtZ{2},
+    proofCopyPermutationGrandProductOpeningAtZOmega{2},
+    stateZInDomainSize{2}, proofQuotientPolyOpeningAtZ{2}) =
+   (stateAlphaG, stateBetaG, stateBetaLookupG, stateGammaG,
+    stateGammaLookupG, stateZG, proofPublicInputG,
+    proofCopyPermutationPolys0OpeningAtZG,
+    proofCopyPermutationPolys1OpeningAtZG,
+    proofCopyPermutationPolys2OpeningAtZG, proofStatePolys0OpeningAtZG,
+    proofStatePolys1OpeningAtZG, proofStatePolys2OpeningAtZG,
+    proofStatePolys3OpeningAtZG, proofLookupSPolyOpeningAtZOmegaG,
+    proofLookupGrandProductOpeningAtZOmegaG, proofGateSelectors0OpeningAtZG,
+    proofLinearisationPolyOpeningAtZG,
+    proofCopyPermutationGrandProductOpeningAtZOmegaG, stateZInDomainSizeG,
+    proofQuotientPolyOpeningAtZG) /\
+   to_uint (mload m STATE_ALPHA_SLOT) = stateAlphaG /\
+   to_uint (mload m STATE_BETA_SLOT) = stateBetaG /\
+   to_uint (mload m STATE_BETA_LOOKUP_SLOT) = stateBetaLookupG /\
+   to_uint (mload m STATE_GAMMA_SLOT) = stateGammaG /\
+   to_uint (mload m STATE_GAMMA_LOOKUP_SLOT) = stateGammaLookupG /\
+   to_uint (mload m STATE_Z_SLOT) = stateZG /\
+   to_uint (mload m PROOF_PUBLIC_INPUT) = proofPublicInputG /\
+   to_uint (mload m PROOF_COPY_PERMUTATION_POLYS_0_OPENING_AT_Z_SLOT) =
+   proofCopyPermutationPolys0OpeningAtZG /\
+   to_uint (mload m PROOF_COPY_PERMUTATION_POLYS_1_OPENING_AT_Z_SLOT) =
+   proofCopyPermutationPolys1OpeningAtZG /\
+   to_uint (mload m PROOF_COPY_PERMUTATION_POLYS_2_OPENING_AT_Z_SLOT) =
+   proofCopyPermutationPolys2OpeningAtZG /\
+   to_uint (mload m PROOF_STATE_POLYS_0_OPENING_AT_Z_SLOT) =
+   proofStatePolys0OpeningAtZG /\
+   to_uint (mload m PROOF_STATE_POLYS_1_OPENING_AT_Z_SLOT) =
+   proofStatePolys1OpeningAtZG /\
+   to_uint (mload m PROOF_STATE_POLYS_2_OPENING_AT_Z_SLOT) =
+   proofStatePolys2OpeningAtZG /\
+   to_uint (mload m PROOF_STATE_POLYS_3_OPENING_AT_Z_SLOT) =
+   proofStatePolys3OpeningAtZG /\
+   to_uint (mload m PROOF_LOOKUP_S_POLY_OPENING_AT_Z_OMEGA_SLOT) =
+   proofLookupSPolyOpeningAtZOmegaG /\
+   to_uint (mload m PROOF_LOOKUP_GRAND_PRODUCT_OPENING_AT_Z_OMEGA_SLOT) =
+   proofLookupGrandProductOpeningAtZOmegaG /\
+   to_uint (mload m PROOF_GATE_SELECTORS_0_OPENING_AT_Z_SLOT) =
+   proofGateSelectors0OpeningAtZG /\
+   to_uint (mload m PROOF_LINEARISATION_POLY_OPENING_AT_Z_SLOT) =
+   proofLinearisationPolyOpeningAtZG /\
+   to_uint
+     (mload m PROOF_COPY_PERMUTATION_GRAND_PRODUCT_OPENING_AT_Z_OMEGA_SLOT) =
+   proofCopyPermutationGrandProductOpeningAtZOmegaG /\
+   to_uint (mload m STATE_Z_IN_DOMAIN_SIZE) = stateZInDomainSizeG /\
+   to_uint (mload m PROOF_QUOTIENT_POLY_OPENING_AT_Z_SLOT) =
+   proofQuotientPolyOpeningAtZG /\
+   a = stateAlpha{2} /\
+   a2 = statePowerOfAlpha2{2} /\
+   a3 = statePowerOfAlpha3{2} /\
+   a4 = statePowerOfAlpha4{2} /\
+   a5 = statePowerOfAlpha5{2} /\
+   a6 = statePowerOfAlpha6{2} /\
+   a7 = statePowerOfAlpha7{2} /\
+   a8 = statePowerOfAlpha8{2} /\
+   statePowerOfAlpha2{2} = stateAlpha{2} ^ 2 %% Constants.R /\
+   statePowerOfAlpha3{2} = stateAlpha{2} ^ 3 %% Constants.R /\
+   statePowerOfAlpha4{2} = stateAlpha{2} ^ 4 %% Constants.R /\
+   statePowerOfAlpha5{2} = stateAlpha{2} ^ 5 %% Constants.R /\
+   statePowerOfAlpha6{2} = stateAlpha{2} ^ 6 %% Constants.R /\
+   statePowerOfAlpha7{2} = stateAlpha{2} ^ 7 %% Constants.R /\
+   statePowerOfAlpha8{2} = stateAlpha{2} ^ 8 %% Constants.R /\
+   to_uint stateZ{1} = stateZ{2} /\
+   (stateZ{2} ^ Constants.DOMAIN_SIZE - 1) %% Constants.R <> 0 /\
+   elpodL0{2} = Some (to_uint _12{1}) /\
+   0 <= to_uint _12{1} < Constants.R /\
+   !Primops.reverted{1} /\
+   Primops.memory{1} = m9
+). skip; progress; smt().
+
+rcondf{2} 1. by progress.
+exists* _12{1}; elim*=> sl0az. pose m10 := store m9 STATE_L_0_AT_Z_SLOT sl0az.
+seq 1 1: (
+  (stateAlpha{2}, stateBeta{2}, stateBetaLookup{2}, stateGamma{2},
+    stateGammaLookup{2}, stateZ{2}, proofPublicInput{2},
+    proofCopyPermutationPolys0OpeningAtZ{2},
+    proofCopyPermutationPolys1OpeningAtZ{2},
+    proofCopyPermutationPolys2OpeningAtZ{2}, proofStatePolys0OpeningAtZ{2},
+    proofStatePolys1OpeningAtZ{2}, proofStatePolys2OpeningAtZ{2},
+    proofStatePolys3OpeningAtZ{2}, proofLookupSPolyOpeningAtZOmega{2},
+    proofLookupGrandProductOpeningAtZOmega{2},
+    proofGateSelectors0OpeningAtZ{2}, proofLinearisationPolyOpeningAtZ{2},
+    proofCopyPermutationGrandProductOpeningAtZOmega{2},
+    stateZInDomainSize{2}, proofQuotientPolyOpeningAtZ{2}) =
+   (stateAlphaG, stateBetaG, stateBetaLookupG, stateGammaG,
+    stateGammaLookupG, stateZG, proofPublicInputG,
+    proofCopyPermutationPolys0OpeningAtZG,
+    proofCopyPermutationPolys1OpeningAtZG,
+    proofCopyPermutationPolys2OpeningAtZG, proofStatePolys0OpeningAtZG,
+    proofStatePolys1OpeningAtZG, proofStatePolys2OpeningAtZG,
+    proofStatePolys3OpeningAtZG, proofLookupSPolyOpeningAtZOmegaG,
+    proofLookupGrandProductOpeningAtZOmegaG, proofGateSelectors0OpeningAtZG,
+    proofLinearisationPolyOpeningAtZG,
+    proofCopyPermutationGrandProductOpeningAtZOmegaG, stateZInDomainSizeG,
+    proofQuotientPolyOpeningAtZG) /\
+   to_uint (mload m STATE_ALPHA_SLOT) = stateAlphaG /\
+   to_uint (mload m STATE_BETA_SLOT) = stateBetaG /\
+   to_uint (mload m STATE_BETA_LOOKUP_SLOT) = stateBetaLookupG /\
+   to_uint (mload m STATE_GAMMA_SLOT) = stateGammaG /\
+   to_uint (mload m STATE_GAMMA_LOOKUP_SLOT) = stateGammaLookupG /\
+   to_uint (mload m STATE_Z_SLOT) = stateZG /\
+   to_uint (mload m PROOF_PUBLIC_INPUT) = proofPublicInputG /\
+   to_uint (mload m PROOF_COPY_PERMUTATION_POLYS_0_OPENING_AT_Z_SLOT) =
+   proofCopyPermutationPolys0OpeningAtZG /\
+   to_uint (mload m PROOF_COPY_PERMUTATION_POLYS_1_OPENING_AT_Z_SLOT) =
+   proofCopyPermutationPolys1OpeningAtZG /\
+   to_uint (mload m PROOF_COPY_PERMUTATION_POLYS_2_OPENING_AT_Z_SLOT) =
+   proofCopyPermutationPolys2OpeningAtZG /\
+   to_uint (mload m PROOF_STATE_POLYS_0_OPENING_AT_Z_SLOT) =
+   proofStatePolys0OpeningAtZG /\
+   to_uint (mload m PROOF_STATE_POLYS_1_OPENING_AT_Z_SLOT) =
+   proofStatePolys1OpeningAtZG /\
+   to_uint (mload m PROOF_STATE_POLYS_2_OPENING_AT_Z_SLOT) =
+   proofStatePolys2OpeningAtZG /\
+   to_uint (mload m PROOF_STATE_POLYS_3_OPENING_AT_Z_SLOT) =
+   proofStatePolys3OpeningAtZG /\
+   to_uint (mload m PROOF_LOOKUP_S_POLY_OPENING_AT_Z_OMEGA_SLOT) =
+   proofLookupSPolyOpeningAtZOmegaG /\
+   to_uint (mload m PROOF_LOOKUP_GRAND_PRODUCT_OPENING_AT_Z_OMEGA_SLOT) =
+   proofLookupGrandProductOpeningAtZOmegaG /\
+   to_uint (mload m PROOF_GATE_SELECTORS_0_OPENING_AT_Z_SLOT) =
+   proofGateSelectors0OpeningAtZG /\
+   to_uint (mload m PROOF_LINEARISATION_POLY_OPENING_AT_Z_SLOT) =
+   proofLinearisationPolyOpeningAtZG /\
+   to_uint
+     (mload m PROOF_COPY_PERMUTATION_GRAND_PRODUCT_OPENING_AT_Z_OMEGA_SLOT) =
+   proofCopyPermutationGrandProductOpeningAtZOmegaG /\
+   to_uint (mload m STATE_Z_IN_DOMAIN_SIZE) = stateZInDomainSizeG /\
+   to_uint (mload m PROOF_QUOTIENT_POLY_OPENING_AT_Z_SLOT) =
+   proofQuotientPolyOpeningAtZG /\
+   a = stateAlpha{2} /\
+   a2 = statePowerOfAlpha2{2} /\
+   a3 = statePowerOfAlpha3{2} /\
+   a4 = statePowerOfAlpha4{2} /\
+   a5 = statePowerOfAlpha5{2} /\
+   a6 = statePowerOfAlpha6{2} /\
+   a7 = statePowerOfAlpha7{2} /\
+   a8 = statePowerOfAlpha8{2} /\
+   statePowerOfAlpha2{2} = stateAlpha{2} ^ 2 %% Constants.R /\
+   statePowerOfAlpha3{2} = stateAlpha{2} ^ 3 %% Constants.R /\
+   statePowerOfAlpha4{2} = stateAlpha{2} ^ 4 %% Constants.R /\
+   statePowerOfAlpha5{2} = stateAlpha{2} ^ 5 %% Constants.R /\
+   statePowerOfAlpha6{2} = stateAlpha{2} ^ 6 %% Constants.R /\
+   statePowerOfAlpha7{2} = stateAlpha{2} ^ 7 %% Constants.R /\
+   statePowerOfAlpha8{2} = stateAlpha{2} ^ 8 %% Constants.R /\
+   sl0az = _12{1} /\ to_uint _12{1} = stateL0AtZ{2} /\
+   to_uint stateZ{1} = stateZ{2} /\
+   (stateZ{2} ^ Constants.DOMAIN_SIZE - 1) %% Constants.R <> 0 /\
+   elpodL0{2} = Some (to_uint _12{1}) /\
+   0 <= to_uint _12{1} < Constants.R /\
+   !Primops.reverted{1} /\
+   Primops.memory{1} = m10
+). 
+wp. call{1} (ConcretePrimops.mstore_pspec m9 STATE_L_0_AT_Z_SLOT sl0az).
+skip. by progress.
+
+seq 1 1: (
+  (stateAlpha{2}, stateBeta{2}, stateBetaLookup{2}, stateGamma{2},
+    stateGammaLookup{2}, stateZ{2}, proofPublicInput{2},
+    proofCopyPermutationPolys0OpeningAtZ{2},
+    proofCopyPermutationPolys1OpeningAtZ{2},
+    proofCopyPermutationPolys2OpeningAtZ{2}, proofStatePolys0OpeningAtZ{2},
+    proofStatePolys1OpeningAtZ{2}, proofStatePolys2OpeningAtZ{2},
+    proofStatePolys3OpeningAtZ{2}, proofLookupSPolyOpeningAtZOmega{2},
+    proofLookupGrandProductOpeningAtZOmega{2},
+    proofGateSelectors0OpeningAtZ{2}, proofLinearisationPolyOpeningAtZ{2},
+    proofCopyPermutationGrandProductOpeningAtZOmega{2},
+    stateZInDomainSize{2}, proofQuotientPolyOpeningAtZ{2}) =
+   (stateAlphaG, stateBetaG, stateBetaLookupG, stateGammaG,
+    stateGammaLookupG, stateZG, proofPublicInputG,
+    proofCopyPermutationPolys0OpeningAtZG,
+    proofCopyPermutationPolys1OpeningAtZG,
+    proofCopyPermutationPolys2OpeningAtZG, proofStatePolys0OpeningAtZG,
+    proofStatePolys1OpeningAtZG, proofStatePolys2OpeningAtZG,
+    proofStatePolys3OpeningAtZG, proofLookupSPolyOpeningAtZOmegaG,
+    proofLookupGrandProductOpeningAtZOmegaG, proofGateSelectors0OpeningAtZG,
+    proofLinearisationPolyOpeningAtZG,
+    proofCopyPermutationGrandProductOpeningAtZOmegaG, stateZInDomainSizeG,
+    proofQuotientPolyOpeningAtZG) /\
+   to_uint (mload m STATE_ALPHA_SLOT) = stateAlphaG /\
+   to_uint (mload m STATE_BETA_SLOT) = stateBetaG /\
+   to_uint (mload m STATE_BETA_LOOKUP_SLOT) = stateBetaLookupG /\
+   to_uint (mload m STATE_GAMMA_SLOT) = stateGammaG /\
+   to_uint (mload m STATE_GAMMA_LOOKUP_SLOT) = stateGammaLookupG /\
+   to_uint (mload m STATE_Z_SLOT) = stateZG /\
+   to_uint (mload m PROOF_PUBLIC_INPUT) = proofPublicInputG /\
+   to_uint (mload m PROOF_COPY_PERMUTATION_POLYS_0_OPENING_AT_Z_SLOT) =
+   proofCopyPermutationPolys0OpeningAtZG /\
+   to_uint (mload m PROOF_COPY_PERMUTATION_POLYS_1_OPENING_AT_Z_SLOT) =
+   proofCopyPermutationPolys1OpeningAtZG /\
+   to_uint (mload m PROOF_COPY_PERMUTATION_POLYS_2_OPENING_AT_Z_SLOT) =
+   proofCopyPermutationPolys2OpeningAtZG /\
+   to_uint (mload m PROOF_STATE_POLYS_0_OPENING_AT_Z_SLOT) =
+   proofStatePolys0OpeningAtZG /\
+   to_uint (mload m PROOF_STATE_POLYS_1_OPENING_AT_Z_SLOT) =
+   proofStatePolys1OpeningAtZG /\
+   to_uint (mload m PROOF_STATE_POLYS_2_OPENING_AT_Z_SLOT) =
+   proofStatePolys2OpeningAtZG /\
+   to_uint (mload m PROOF_STATE_POLYS_3_OPENING_AT_Z_SLOT) =
+   proofStatePolys3OpeningAtZG /\
+   to_uint (mload m PROOF_LOOKUP_S_POLY_OPENING_AT_Z_OMEGA_SLOT) =
+   proofLookupSPolyOpeningAtZOmegaG /\
+   to_uint (mload m PROOF_LOOKUP_GRAND_PRODUCT_OPENING_AT_Z_OMEGA_SLOT) =
+   proofLookupGrandProductOpeningAtZOmegaG /\
+   to_uint (mload m PROOF_GATE_SELECTORS_0_OPENING_AT_Z_SLOT) =
+   proofGateSelectors0OpeningAtZG /\
+   to_uint (mload m PROOF_LINEARISATION_POLY_OPENING_AT_Z_SLOT) =
+   proofLinearisationPolyOpeningAtZG /\
+   to_uint
+     (mload m PROOF_COPY_PERMUTATION_GRAND_PRODUCT_OPENING_AT_Z_OMEGA_SLOT) =
+   proofCopyPermutationGrandProductOpeningAtZOmegaG /\
+   to_uint (mload m STATE_Z_IN_DOMAIN_SIZE) = stateZInDomainSizeG /\
+   to_uint (mload m PROOF_QUOTIENT_POLY_OPENING_AT_Z_SLOT) =
+   proofQuotientPolyOpeningAtZG /\
+   a = stateAlpha{2} /\
+   a2 = statePowerOfAlpha2{2} /\
+   a3 = statePowerOfAlpha3{2} /\
+   a4 = statePowerOfAlpha4{2} /\
+   a5 = statePowerOfAlpha5{2} /\
+   a6 = statePowerOfAlpha6{2} /\
+   a7 = statePowerOfAlpha7{2} /\
+   a8 = statePowerOfAlpha8{2} /\
+   statePowerOfAlpha2{2} = stateAlpha{2} ^ 2 %% Constants.R /\
+   statePowerOfAlpha3{2} = stateAlpha{2} ^ 3 %% Constants.R /\
+   statePowerOfAlpha4{2} = stateAlpha{2} ^ 4 %% Constants.R /\
+   statePowerOfAlpha5{2} = stateAlpha{2} ^ 5 %% Constants.R /\
+   statePowerOfAlpha6{2} = stateAlpha{2} ^ 6 %% Constants.R /\
+   statePowerOfAlpha7{2} = stateAlpha{2} ^ 7 %% Constants.R /\
+   statePowerOfAlpha8{2} = stateAlpha{2} ^ 8 %% Constants.R /\
+   sl0az = _12{1} /\ to_uint _12{1} = stateL0AtZ{2} /\
+   to_uint stateZ{1} = stateZ{2} /\
+   (stateZ{2} ^ Constants.DOMAIN_SIZE - 1) %% Constants.R <> 0 /\
+   elpodL0{2} = Some (to_uint _12{1}) /\
+   elpodLn{2} = Some (to_uint _17{1}) /\
+   0 <= to_uint _12{1} < Constants.R /\
+   0 <= to_uint _17{1} < Constants.R /\
+   !Primops.reverted{1} /\
+   exists v4 v5 v6, Primops.memory{1} = lagrange_memory_footprint m10 v4 v5 v6
+).
+call (evaluateLagrangePolyOutOfDomain_low_equiv_mid m10 (DOMAIN_SIZE - W256.one) (W256.of_int stateZG)).
+skip. progress. smt(@W256). rewrite /DOMAIN_SIZE. smt(). smt(). smt(). smt(). smt(). smt().
+
+rewrite /lagrange_memory_footprint. elim*. progress.
+pose m11 := lagrange_memory_footprint m10 v4 v5 v6.
+seq 0 0: (
+  (stateAlpha{2}, stateBeta{2}, stateBetaLookup{2}, stateGamma{2},
+    stateGammaLookup{2}, stateZ{2}, proofPublicInput{2},
+    proofCopyPermutationPolys0OpeningAtZ{2},
+    proofCopyPermutationPolys1OpeningAtZ{2},
+    proofCopyPermutationPolys2OpeningAtZ{2}, proofStatePolys0OpeningAtZ{2},
+    proofStatePolys1OpeningAtZ{2}, proofStatePolys2OpeningAtZ{2},
+    proofStatePolys3OpeningAtZ{2}, proofLookupSPolyOpeningAtZOmega{2},
+    proofLookupGrandProductOpeningAtZOmega{2},
+    proofGateSelectors0OpeningAtZ{2}, proofLinearisationPolyOpeningAtZ{2},
+    proofCopyPermutationGrandProductOpeningAtZOmega{2},
+    stateZInDomainSize{2}, proofQuotientPolyOpeningAtZ{2}) =
+   (stateAlphaG, stateBetaG, stateBetaLookupG, stateGammaG,
+    stateGammaLookupG, stateZG, proofPublicInputG,
+    proofCopyPermutationPolys0OpeningAtZG,
+    proofCopyPermutationPolys1OpeningAtZG,
+    proofCopyPermutationPolys2OpeningAtZG, proofStatePolys0OpeningAtZG,
+    proofStatePolys1OpeningAtZG, proofStatePolys2OpeningAtZG,
+    proofStatePolys3OpeningAtZG, proofLookupSPolyOpeningAtZOmegaG,
+    proofLookupGrandProductOpeningAtZOmegaG, proofGateSelectors0OpeningAtZG,
+    proofLinearisationPolyOpeningAtZG,
+    proofCopyPermutationGrandProductOpeningAtZOmegaG, stateZInDomainSizeG,
+    proofQuotientPolyOpeningAtZG) /\
+   to_uint (mload m STATE_ALPHA_SLOT) = stateAlphaG /\
+   to_uint (mload m STATE_BETA_SLOT) = stateBetaG /\
+   to_uint (mload m STATE_BETA_LOOKUP_SLOT) = stateBetaLookupG /\
+   to_uint (mload m STATE_GAMMA_SLOT) = stateGammaG /\
+   to_uint (mload m STATE_GAMMA_LOOKUP_SLOT) = stateGammaLookupG /\
+   to_uint (mload m STATE_Z_SLOT) = stateZG /\
+   to_uint (mload m PROOF_PUBLIC_INPUT) = proofPublicInputG /\
+   to_uint (mload m PROOF_COPY_PERMUTATION_POLYS_0_OPENING_AT_Z_SLOT) =
+   proofCopyPermutationPolys0OpeningAtZG /\
+   to_uint (mload m PROOF_COPY_PERMUTATION_POLYS_1_OPENING_AT_Z_SLOT) =
+   proofCopyPermutationPolys1OpeningAtZG /\
+   to_uint (mload m PROOF_COPY_PERMUTATION_POLYS_2_OPENING_AT_Z_SLOT) =
+   proofCopyPermutationPolys2OpeningAtZG /\
+   to_uint (mload m PROOF_STATE_POLYS_0_OPENING_AT_Z_SLOT) =
+   proofStatePolys0OpeningAtZG /\
+   to_uint (mload m PROOF_STATE_POLYS_1_OPENING_AT_Z_SLOT) =
+   proofStatePolys1OpeningAtZG /\
+   to_uint (mload m PROOF_STATE_POLYS_2_OPENING_AT_Z_SLOT) =
+   proofStatePolys2OpeningAtZG /\
+   to_uint (mload m PROOF_STATE_POLYS_3_OPENING_AT_Z_SLOT) =
+   proofStatePolys3OpeningAtZG /\
+   to_uint (mload m PROOF_LOOKUP_S_POLY_OPENING_AT_Z_OMEGA_SLOT) =
+   proofLookupSPolyOpeningAtZOmegaG /\
+   to_uint (mload m PROOF_LOOKUP_GRAND_PRODUCT_OPENING_AT_Z_OMEGA_SLOT) =
+   proofLookupGrandProductOpeningAtZOmegaG /\
+   to_uint (mload m PROOF_GATE_SELECTORS_0_OPENING_AT_Z_SLOT) =
+   proofGateSelectors0OpeningAtZG /\
+   to_uint (mload m PROOF_LINEARISATION_POLY_OPENING_AT_Z_SLOT) =
+   proofLinearisationPolyOpeningAtZG /\
+   to_uint
+     (mload m PROOF_COPY_PERMUTATION_GRAND_PRODUCT_OPENING_AT_Z_OMEGA_SLOT) =
+   proofCopyPermutationGrandProductOpeningAtZOmegaG /\
+   to_uint (mload m STATE_Z_IN_DOMAIN_SIZE) = stateZInDomainSizeG /\
+   to_uint (mload m PROOF_QUOTIENT_POLY_OPENING_AT_Z_SLOT) =
+   proofQuotientPolyOpeningAtZG /\
+   a = stateAlpha{2} /\
+   a2 = statePowerOfAlpha2{2} /\
+   a3 = statePowerOfAlpha3{2} /\
+   a4 = statePowerOfAlpha4{2} /\
+   a5 = statePowerOfAlpha5{2} /\
+   a6 = statePowerOfAlpha6{2} /\
+   a7 = statePowerOfAlpha7{2} /\
+   a8 = statePowerOfAlpha8{2} /\
+   statePowerOfAlpha2{2} = stateAlpha{2} ^ 2 %% Constants.R /\
+   statePowerOfAlpha3{2} = stateAlpha{2} ^ 3 %% Constants.R /\
+   statePowerOfAlpha4{2} = stateAlpha{2} ^ 4 %% Constants.R /\
+   statePowerOfAlpha5{2} = stateAlpha{2} ^ 5 %% Constants.R /\
+   statePowerOfAlpha6{2} = stateAlpha{2} ^ 6 %% Constants.R /\
+   statePowerOfAlpha7{2} = stateAlpha{2} ^ 7 %% Constants.R /\
+   statePowerOfAlpha8{2} = stateAlpha{2} ^ 8 %% Constants.R /\
+   sl0az = _12{1} /\ to_uint _12{1} = stateL0AtZ{2} /\
+   to_uint stateZ{1} = stateZ{2} /\
+   (stateZ{2} ^ Constants.DOMAIN_SIZE - 1) %% Constants.R <> 0 /\
+   elpodL0{2} = Some (to_uint _12{1}) /\
+   elpodLn{2} = Some (to_uint _17{1}) /\
+   0 <= to_uint _12{1} < Constants.R /\
+   0 <= to_uint _17{1} < Constants.R /\
+   !Primops.reverted{1} /\
+   Primops.memory{1} = m11
+). 
+skip. by progress. 
+
+exists* _17{1}; elim*=> slnm1az. pose m12 := store m11 STATE_L_N_MINUS_ONE_AT_Z_SLOT slnm1az.
+seq 1 1: (
+  (stateAlpha{2}, stateBeta{2}, stateBetaLookup{2}, stateGamma{2},
+    stateGammaLookup{2}, stateZ{2}, proofPublicInput{2},
+    proofCopyPermutationPolys0OpeningAtZ{2},
+    proofCopyPermutationPolys1OpeningAtZ{2},
+    proofCopyPermutationPolys2OpeningAtZ{2}, proofStatePolys0OpeningAtZ{2},
+    proofStatePolys1OpeningAtZ{2}, proofStatePolys2OpeningAtZ{2},
+    proofStatePolys3OpeningAtZ{2}, proofLookupSPolyOpeningAtZOmega{2},
+    proofLookupGrandProductOpeningAtZOmega{2},
+    proofGateSelectors0OpeningAtZ{2}, proofLinearisationPolyOpeningAtZ{2},
+    proofCopyPermutationGrandProductOpeningAtZOmega{2},
+    stateZInDomainSize{2}, proofQuotientPolyOpeningAtZ{2}) =
+   (stateAlphaG, stateBetaG, stateBetaLookupG, stateGammaG,
+    stateGammaLookupG, stateZG, proofPublicInputG,
+    proofCopyPermutationPolys0OpeningAtZG,
+    proofCopyPermutationPolys1OpeningAtZG,
+    proofCopyPermutationPolys2OpeningAtZG, proofStatePolys0OpeningAtZG,
+    proofStatePolys1OpeningAtZG, proofStatePolys2OpeningAtZG,
+    proofStatePolys3OpeningAtZG, proofLookupSPolyOpeningAtZOmegaG,
+    proofLookupGrandProductOpeningAtZOmegaG, proofGateSelectors0OpeningAtZG,
+    proofLinearisationPolyOpeningAtZG,
+    proofCopyPermutationGrandProductOpeningAtZOmegaG, stateZInDomainSizeG,
+    proofQuotientPolyOpeningAtZG) /\
+   to_uint (mload m STATE_ALPHA_SLOT) = stateAlphaG /\
+   to_uint (mload m STATE_BETA_SLOT) = stateBetaG /\
+   to_uint (mload m STATE_BETA_LOOKUP_SLOT) = stateBetaLookupG /\
+   to_uint (mload m STATE_GAMMA_SLOT) = stateGammaG /\
+   to_uint (mload m STATE_GAMMA_LOOKUP_SLOT) = stateGammaLookupG /\
+   to_uint (mload m STATE_Z_SLOT) = stateZG /\
+   to_uint (mload m PROOF_PUBLIC_INPUT) = proofPublicInputG /\
+   to_uint (mload m PROOF_COPY_PERMUTATION_POLYS_0_OPENING_AT_Z_SLOT) =
+   proofCopyPermutationPolys0OpeningAtZG /\
+   to_uint (mload m PROOF_COPY_PERMUTATION_POLYS_1_OPENING_AT_Z_SLOT) =
+   proofCopyPermutationPolys1OpeningAtZG /\
+   to_uint (mload m PROOF_COPY_PERMUTATION_POLYS_2_OPENING_AT_Z_SLOT) =
+   proofCopyPermutationPolys2OpeningAtZG /\
+   to_uint (mload m PROOF_STATE_POLYS_0_OPENING_AT_Z_SLOT) =
+   proofStatePolys0OpeningAtZG /\
+   to_uint (mload m PROOF_STATE_POLYS_1_OPENING_AT_Z_SLOT) =
+   proofStatePolys1OpeningAtZG /\
+   to_uint (mload m PROOF_STATE_POLYS_2_OPENING_AT_Z_SLOT) =
+   proofStatePolys2OpeningAtZG /\
+   to_uint (mload m PROOF_STATE_POLYS_3_OPENING_AT_Z_SLOT) =
+   proofStatePolys3OpeningAtZG /\
+   to_uint (mload m PROOF_LOOKUP_S_POLY_OPENING_AT_Z_OMEGA_SLOT) =
+   proofLookupSPolyOpeningAtZOmegaG /\
+   to_uint (mload m PROOF_LOOKUP_GRAND_PRODUCT_OPENING_AT_Z_OMEGA_SLOT) =
+   proofLookupGrandProductOpeningAtZOmegaG /\
+   to_uint (mload m PROOF_GATE_SELECTORS_0_OPENING_AT_Z_SLOT) =
+   proofGateSelectors0OpeningAtZG /\
+   to_uint (mload m PROOF_LINEARISATION_POLY_OPENING_AT_Z_SLOT) =
+   proofLinearisationPolyOpeningAtZG /\
+   to_uint
+     (mload m PROOF_COPY_PERMUTATION_GRAND_PRODUCT_OPENING_AT_Z_OMEGA_SLOT) =
+   proofCopyPermutationGrandProductOpeningAtZOmegaG /\
+   to_uint (mload m STATE_Z_IN_DOMAIN_SIZE) = stateZInDomainSizeG /\
+   to_uint (mload m PROOF_QUOTIENT_POLY_OPENING_AT_Z_SLOT) =
+   proofQuotientPolyOpeningAtZG /\
+   a = stateAlpha{2} /\
+   a2 = statePowerOfAlpha2{2} /\
+   a3 = statePowerOfAlpha3{2} /\
+   a4 = statePowerOfAlpha4{2} /\
+   a5 = statePowerOfAlpha5{2} /\
+   a6 = statePowerOfAlpha6{2} /\
+   a7 = statePowerOfAlpha7{2} /\
+   a8 = statePowerOfAlpha8{2} /\
+   statePowerOfAlpha2{2} = stateAlpha{2} ^ 2 %% Constants.R /\
+   statePowerOfAlpha3{2} = stateAlpha{2} ^ 3 %% Constants.R /\
+   statePowerOfAlpha4{2} = stateAlpha{2} ^ 4 %% Constants.R /\
+   statePowerOfAlpha5{2} = stateAlpha{2} ^ 5 %% Constants.R /\
+   statePowerOfAlpha6{2} = stateAlpha{2} ^ 6 %% Constants.R /\
+   statePowerOfAlpha7{2} = stateAlpha{2} ^ 7 %% Constants.R /\
+   statePowerOfAlpha8{2} = stateAlpha{2} ^ 8 %% Constants.R /\
+   sl0az = _12{1} /\ to_uint _12{1} = stateL0AtZ{2} /\
+   slnm1az = _17{1} /\ to_uint _17{1} = stateLnMinusOneAtZ{2} /\  
+   to_uint stateZ{1} = stateZ{2} /\
+   (stateZ{2} ^ Constants.DOMAIN_SIZE - 1) %% Constants.R <> 0 /\
+   elpodL0{2} = Some (to_uint _12{1}) /\
+   elpodLn{2} = Some (to_uint _17{1}) /\
+   0 <= to_uint _12{1} < Constants.R /\
+   0 <= to_uint _17{1} < Constants.R /\
+   !Primops.reverted{1} /\
+   Primops.memory{1} = m12
+).
+wp. call{1} (ConcretePrimops.mstore_pspec m11 STATE_L_N_MINUS_ONE_AT_Z_SLOT slnm1az).
+skip. by progress.
+
+seq 1 0: (#pre /\ to_uint _20{1} = proofPublicInput{2}).
+call{1} (ConcretePrimops.mload_pspec m12 PROOF_PUBLIC_INPUT). skip. progress.
+rewrite /m12 /m11 /m10 /m9 /m8 /m7 /m6 /m5 /m4 /m3 /m2 /m1 /lagrange_memory_footprint /modexp_memory_footprint; progress.
+do 22! (rewrite load_store_diff;
+rewrite /STATE_Z_SLOT
+        /STATE_POWER_OF_ALPHA_8_SLOT
+        /STATE_POWER_OF_ALPHA_7_SLOT
+        /STATE_POWER_OF_ALPHA_6_SLOT
+        /STATE_POWER_OF_ALPHA_5_SLOT
+        /STATE_POWER_OF_ALPHA_4_SLOT
+        /STATE_POWER_OF_ALPHA_3_SLOT 
+        /STATE_POWER_OF_ALPHA_2_SLOT
+        /PROOF_PUBLIC_INPUT
+        /STATE_L_N_MINUS_ONE_AT_Z_SLOT
+        /STATE_L_0_AT_Z_SLOT ; try by progress).
+
+seq 1 0: (#pre /\ _21{1} = _12{1}).
+call{1} (ConcretePrimops.mload_pspec m12 STATE_L_0_AT_Z_SLOT).
+skip. progress. 
+rewrite /m12 /m11 /m10 /m9 /m8 /m7 /m6 /m5 /m4 /m3 /m2 /m1 /lagrange_memory_footprint /modexp_memory_footprint; progress.
+do 7! (rewrite load_store_diff;
+rewrite /STATE_Z_SLOT
+        /STATE_POWER_OF_ALPHA_8_SLOT
+        /STATE_POWER_OF_ALPHA_7_SLOT
+        /STATE_POWER_OF_ALPHA_6_SLOT
+        /STATE_POWER_OF_ALPHA_5_SLOT
+        /STATE_POWER_OF_ALPHA_4_SLOT
+        /STATE_POWER_OF_ALPHA_3_SLOT 
+        /STATE_POWER_OF_ALPHA_2_SLOT
+        /PROOF_PUBLIC_INPUT
+        /STATE_L_N_MINUS_ONE_AT_Z_SLOT
+        /STATE_L_0_AT_Z_SLOT ; try by progress).
+rewrite load_store_same; reflexivity.
+
+seq 1 1: (#pre /\
+  to_uint stateT{1} = stateT{2} /\
+  stateT{2} = (stateL0AtZ{2} * proofPublicInput{2}) %% Constants.R).
+wp. skip. progress. rewrite /mulmod -H6. progress.
+rewrite W256.to_uint_small. progress. by smt(@W256 @Utils). by smt(@W256 @Utils). rewrite /R_MOD. smt().
+
+seq 1 0: (#pre /\ to_uint _23{1} = proofGateSelectors0OpeningAtZ{2}).
+call{1} (ConcretePrimops.mload_pspec m12 PROOF_GATE_SELECTORS_0_OPENING_AT_Z_SLOT).
+skip. progress. 
+rewrite /m12 /m11 /m10 /m9 /m8 /m7 /m6 /m5 /m4 /m3 /m2 /m1 /lagrange_memory_footprint /modexp_memory_footprint; progress.
+do 23! (rewrite load_store_diff;
+rewrite /STATE_Z_SLOT
+        /STATE_POWER_OF_ALPHA_8_SLOT
+        /STATE_POWER_OF_ALPHA_7_SLOT
+        /STATE_POWER_OF_ALPHA_6_SLOT
+        /STATE_POWER_OF_ALPHA_5_SLOT
+        /STATE_POWER_OF_ALPHA_4_SLOT
+        /STATE_POWER_OF_ALPHA_3_SLOT 
+        /STATE_POWER_OF_ALPHA_2_SLOT
+        /PROOF_PUBLIC_INPUT
+        /STATE_L_N_MINUS_ONE_AT_Z_SLOT
+        /STATE_L_0_AT_Z_SLOT
+        /PROOF_GATE_SELECTORS_0_OPENING_AT_Z_SLOT ; try by progress).
+
+seq 1 1: (#pre /\
+  to_uint result{1} = pgsT{2} /\
+  pgsT{2} = (stateT{2} * proofGateSelectors0OpeningAtZ{2}) %% Constants.R).
+wp. skip. progress. rewrite /mulmod -H8. progress.
+rewrite W256.to_uint_small. progress. by smt(@W256 @Utils). by smt(@W256 @Utils). rewrite /R_MOD. smt().
+
+seq 1 1: (#pre /\ to_uint _24{1} = pqc{2} /\ 0 <= pqc{2} < Constants.R).
+call (permutationQuotientContribution_low_equiv_mid m12
+      a4 a5
+      proofCopyPermutationGrandProductOpeningAtZOmegaG
+      stateBetaG
+      stateGammaG
+      proofCopyPermutationPolys0OpeningAtZG
+      proofCopyPermutationPolys1OpeningAtZG
+      proofCopyPermutationPolys2OpeningAtZG
+      proofStatePolys0OpeningAtZG
+      proofStatePolys1OpeningAtZG
+      proofStatePolys2OpeningAtZG
+      proofStatePolys3OpeningAtZG
+      (W256.to_uint sl0az)).
+skip. progress.
+rewrite /m12 /m11 /m10 /m9 /m8 /m7 /m6 /m5 /m4 /m3 /m2 /m1 /lagrange_memory_footprint /modexp_memory_footprint; progress.
+do 18! (rewrite load_store_diff;
+rewrite /STATE_Z_SLOT
+        /STATE_POWER_OF_ALPHA_8_SLOT
+        /STATE_POWER_OF_ALPHA_7_SLOT
+        /STATE_POWER_OF_ALPHA_6_SLOT
+        /STATE_POWER_OF_ALPHA_5_SLOT
+        /STATE_POWER_OF_ALPHA_4_SLOT
+        /STATE_POWER_OF_ALPHA_3_SLOT 
+        /STATE_POWER_OF_ALPHA_2_SLOT
+        /PROOF_PUBLIC_INPUT
+        /STATE_L_N_MINUS_ONE_AT_Z_SLOT
+        /STATE_L_0_AT_Z_SLOT
+        /PROOF_GATE_SELECTORS_0_OPENING_AT_Z_SLOT ; try by progress).
+rewrite load_store_same; smt(@W256 @Utils).
+rewrite /m12 /m11 /m10 /m9 /m8 /m7 /m6 /m5 /m4 /m3 /m2 /m1 /lagrange_memory_footprint /modexp_memory_footprint; progress.
+do 17! (rewrite load_store_diff;
+rewrite /STATE_Z_SLOT
+        /STATE_POWER_OF_ALPHA_8_SLOT
+        /STATE_POWER_OF_ALPHA_7_SLOT
+        /STATE_POWER_OF_ALPHA_6_SLOT
+        /STATE_POWER_OF_ALPHA_5_SLOT
+        /STATE_POWER_OF_ALPHA_4_SLOT
+        /STATE_POWER_OF_ALPHA_3_SLOT 
+        /STATE_POWER_OF_ALPHA_2_SLOT
+        /PROOF_PUBLIC_INPUT
+        /STATE_L_N_MINUS_ONE_AT_Z_SLOT
+        /STATE_L_0_AT_Z_SLOT
+        /PROOF_GATE_SELECTORS_0_OPENING_AT_Z_SLOT ; try by progress).
+rewrite load_store_same; smt(@W256 @Utils).
+rewrite /m12 /m11 /m10 /m9 /m8 /m7 /m6 /m5 /m4 /m3 /m2 /m1 /lagrange_memory_footprint /modexp_memory_footprint; progress.
+do 22! (rewrite load_store_diff;
+rewrite /STATE_Z_SLOT
+        /STATE_POWER_OF_ALPHA_8_SLOT
+        /STATE_POWER_OF_ALPHA_7_SLOT
+        /STATE_POWER_OF_ALPHA_6_SLOT
+        /STATE_POWER_OF_ALPHA_5_SLOT
+        /STATE_POWER_OF_ALPHA_4_SLOT
+        /STATE_POWER_OF_ALPHA_3_SLOT 
+        /STATE_POWER_OF_ALPHA_2_SLOT
+        /STATE_ALPHA_SLOT
+        /PROOF_PUBLIC_INPUT
+        /STATE_L_N_MINUS_ONE_AT_Z_SLOT
+        /STATE_L_0_AT_Z_SLOT
+        /PROOF_GATE_SELECTORS_0_OPENING_AT_Z_SLOT
+        /PROOF_COPY_PERMUTATION_GRAND_PRODUCT_OPENING_AT_Z_OMEGA_SLOT ; try by progress).
+rewrite /m12 /m11 /m10 /m9 /m8 /m7 /m6 /m5 /m4 /m3 /m2 /m1 /lagrange_memory_footprint /modexp_memory_footprint; progress.
+do 22! (rewrite load_store_diff;
+rewrite /STATE_Z_SLOT
+        /STATE_POWER_OF_ALPHA_8_SLOT
+        /STATE_POWER_OF_ALPHA_7_SLOT
+        /STATE_POWER_OF_ALPHA_6_SLOT
+        /STATE_POWER_OF_ALPHA_5_SLOT
+        /STATE_POWER_OF_ALPHA_4_SLOT
+        /STATE_POWER_OF_ALPHA_3_SLOT 
+        /STATE_POWER_OF_ALPHA_2_SLOT
+        /STATE_ALPHA_SLOT
+        /STATE_GAMMA_SLOT
+        /PROOF_PUBLIC_INPUT
+        /STATE_L_N_MINUS_ONE_AT_Z_SLOT
+        /STATE_L_0_AT_Z_SLOT
+        /PROOF_GATE_SELECTORS_0_OPENING_AT_Z_SLOT
+        /PROOF_COPY_PERMUTATION_GRAND_PRODUCT_OPENING_AT_Z_OMEGA_SLOT ; try by progress).
+rewrite /m12 /m11 /m10 /m9 /m8 /m7 /m6 /m5 /m4 /m3 /m2 /m1 /lagrange_memory_footprint /modexp_memory_footprint; progress.
+do 22! (rewrite load_store_diff;
+rewrite /STATE_Z_SLOT
+        /STATE_POWER_OF_ALPHA_8_SLOT
+        /STATE_POWER_OF_ALPHA_7_SLOT
+        /STATE_POWER_OF_ALPHA_6_SLOT
+        /STATE_POWER_OF_ALPHA_5_SLOT
+        /STATE_POWER_OF_ALPHA_4_SLOT
+        /STATE_POWER_OF_ALPHA_3_SLOT 
+        /STATE_POWER_OF_ALPHA_2_SLOT
+        /STATE_ALPHA_SLOT
+        /STATE_BETA_SLOT
+        /STATE_GAMMA_SLOT
+        /PROOF_PUBLIC_INPUT
+        /STATE_L_N_MINUS_ONE_AT_Z_SLOT
+        /STATE_L_0_AT_Z_SLOT
+        /PROOF_GATE_SELECTORS_0_OPENING_AT_Z_SLOT
+        /PROOF_COPY_PERMUTATION_POLYS_0_OPENING_AT_Z_SLOT
+        /PROOF_COPY_PERMUTATION_GRAND_PRODUCT_OPENING_AT_Z_OMEGA_SLOT ; try by progress).
+rewrite /m12 /m11 /m10 /m9 /m8 /m7 /m6 /m5 /m4 /m3 /m2 /m1 /lagrange_memory_footprint /modexp_memory_footprint; progress.
+do 22! (rewrite load_store_diff;
+rewrite /STATE_Z_SLOT
+        /STATE_POWER_OF_ALPHA_8_SLOT
+        /STATE_POWER_OF_ALPHA_7_SLOT
+        /STATE_POWER_OF_ALPHA_6_SLOT
+        /STATE_POWER_OF_ALPHA_5_SLOT
+        /STATE_POWER_OF_ALPHA_4_SLOT
+        /STATE_POWER_OF_ALPHA_3_SLOT 
+        /STATE_POWER_OF_ALPHA_2_SLOT
+        /STATE_ALPHA_SLOT
+        /STATE_BETA_SLOT
+        /STATE_GAMMA_SLOT
+        /PROOF_PUBLIC_INPUT
+        /STATE_L_N_MINUS_ONE_AT_Z_SLOT
+        /STATE_L_0_AT_Z_SLOT
+        /PROOF_GATE_SELECTORS_0_OPENING_AT_Z_SLOT
+        /PROOF_COPY_PERMUTATION_POLYS_0_OPENING_AT_Z_SLOT
+        /PROOF_COPY_PERMUTATION_POLYS_1_OPENING_AT_Z_SLOT
+        /PROOF_COPY_PERMUTATION_POLYS_2_OPENING_AT_Z_SLOT
+        /PROOF_COPY_PERMUTATION_GRAND_PRODUCT_OPENING_AT_Z_OMEGA_SLOT ; try by progress).
+rewrite /m12 /m11 /m10 /m9 /m8 /m7 /m6 /m5 /m4 /m3 /m2 /m1 /lagrange_memory_footprint /modexp_memory_footprint; progress.
+do 22! (rewrite load_store_diff;
+rewrite /STATE_Z_SLOT
+        /STATE_POWER_OF_ALPHA_8_SLOT
+        /STATE_POWER_OF_ALPHA_7_SLOT
+        /STATE_POWER_OF_ALPHA_6_SLOT
+        /STATE_POWER_OF_ALPHA_5_SLOT
+        /STATE_POWER_OF_ALPHA_4_SLOT
+        /STATE_POWER_OF_ALPHA_3_SLOT 
+        /STATE_POWER_OF_ALPHA_2_SLOT
+        /STATE_ALPHA_SLOT
+        /STATE_BETA_SLOT
+        /STATE_GAMMA_SLOT
+        /PROOF_PUBLIC_INPUT
+        /STATE_L_N_MINUS_ONE_AT_Z_SLOT
+        /STATE_L_0_AT_Z_SLOT
+        /PROOF_GATE_SELECTORS_0_OPENING_AT_Z_SLOT
+        /PROOF_COPY_PERMUTATION_POLYS_0_OPENING_AT_Z_SLOT
+        /PROOF_COPY_PERMUTATION_POLYS_1_OPENING_AT_Z_SLOT
+        /PROOF_COPY_PERMUTATION_POLYS_2_OPENING_AT_Z_SLOT
+        /PROOF_COPY_PERMUTATION_GRAND_PRODUCT_OPENING_AT_Z_OMEGA_SLOT ; try by progress).
+rewrite /m12 /m11 /m10 /m9 /m8 /m7 /m6 /m5 /m4 /m3 /m2 /m1 /lagrange_memory_footprint /modexp_memory_footprint; progress.
+do 22! (rewrite load_store_diff;
+rewrite /STATE_Z_SLOT
+        /STATE_POWER_OF_ALPHA_8_SLOT
+        /STATE_POWER_OF_ALPHA_7_SLOT
+        /STATE_POWER_OF_ALPHA_6_SLOT
+        /STATE_POWER_OF_ALPHA_5_SLOT
+        /STATE_POWER_OF_ALPHA_4_SLOT
+        /STATE_POWER_OF_ALPHA_3_SLOT 
+        /STATE_POWER_OF_ALPHA_2_SLOT
+        /STATE_ALPHA_SLOT
+        /STATE_BETA_SLOT
+        /STATE_GAMMA_SLOT
+        /PROOF_PUBLIC_INPUT
+        /STATE_L_N_MINUS_ONE_AT_Z_SLOT
+        /STATE_L_0_AT_Z_SLOT
+        /PROOF_GATE_SELECTORS_0_OPENING_AT_Z_SLOT
+        /PROOF_COPY_PERMUTATION_POLYS_0_OPENING_AT_Z_SLOT
+        /PROOF_COPY_PERMUTATION_POLYS_1_OPENING_AT_Z_SLOT
+        /PROOF_COPY_PERMUTATION_POLYS_2_OPENING_AT_Z_SLOT
+        /PROOF_COPY_PERMUTATION_GRAND_PRODUCT_OPENING_AT_Z_OMEGA_SLOT ; try by progress).
+rewrite /m12 /m11 /m10 /m9 /m8 /m7 /m6 /m5 /m4 /m3 /m2 /m1 /lagrange_memory_footprint /modexp_memory_footprint; progress.
+do 22! (rewrite load_store_diff;
+rewrite /STATE_Z_SLOT
+        /STATE_POWER_OF_ALPHA_8_SLOT
+        /STATE_POWER_OF_ALPHA_7_SLOT
+        /STATE_POWER_OF_ALPHA_6_SLOT
+        /STATE_POWER_OF_ALPHA_5_SLOT
+        /STATE_POWER_OF_ALPHA_4_SLOT
+        /STATE_POWER_OF_ALPHA_3_SLOT 
+        /STATE_POWER_OF_ALPHA_2_SLOT
+        /STATE_ALPHA_SLOT
+        /STATE_BETA_SLOT
+        /STATE_GAMMA_SLOT
+        /PROOF_PUBLIC_INPUT
+        /STATE_L_N_MINUS_ONE_AT_Z_SLOT
+        /STATE_L_0_AT_Z_SLOT
+        /PROOF_GATE_SELECTORS_0_OPENING_AT_Z_SLOT
+        /PROOF_STATE_POLYS_0_OPENING_AT_Z_SLOT
+        /PROOF_STATE_POLYS_1_OPENING_AT_Z_SLOT
+        /PROOF_STATE_POLYS_2_OPENING_AT_Z_SLOT
+        /PROOF_COPY_PERMUTATION_POLYS_0_OPENING_AT_Z_SLOT
+        /PROOF_COPY_PERMUTATION_POLYS_1_OPENING_AT_Z_SLOT
+        /PROOF_COPY_PERMUTATION_POLYS_2_OPENING_AT_Z_SLOT
+        /PROOF_COPY_PERMUTATION_GRAND_PRODUCT_OPENING_AT_Z_OMEGA_SLOT ; try by progress).
+rewrite /m12 /m11 /m10 /m9 /m8 /m7 /m6 /m5 /m4 /m3 /m2 /m1 /lagrange_memory_footprint /modexp_memory_footprint; progress.
+do 22! (rewrite load_store_diff;
+rewrite /STATE_Z_SLOT
+        /STATE_POWER_OF_ALPHA_8_SLOT
+        /STATE_POWER_OF_ALPHA_7_SLOT
+        /STATE_POWER_OF_ALPHA_6_SLOT
+        /STATE_POWER_OF_ALPHA_5_SLOT
+        /STATE_POWER_OF_ALPHA_4_SLOT
+        /STATE_POWER_OF_ALPHA_3_SLOT 
+        /STATE_POWER_OF_ALPHA_2_SLOT
+        /STATE_ALPHA_SLOT
+        /STATE_BETA_SLOT
+        /STATE_GAMMA_SLOT
+        /PROOF_PUBLIC_INPUT
+        /STATE_L_N_MINUS_ONE_AT_Z_SLOT
+        /STATE_L_0_AT_Z_SLOT
+        /PROOF_GATE_SELECTORS_0_OPENING_AT_Z_SLOT
+        /PROOF_STATE_POLYS_0_OPENING_AT_Z_SLOT
+        /PROOF_STATE_POLYS_1_OPENING_AT_Z_SLOT
+        /PROOF_STATE_POLYS_2_OPENING_AT_Z_SLOT
+        /PROOF_COPY_PERMUTATION_POLYS_0_OPENING_AT_Z_SLOT
+        /PROOF_COPY_PERMUTATION_POLYS_1_OPENING_AT_Z_SLOT
+        /PROOF_COPY_PERMUTATION_POLYS_2_OPENING_AT_Z_SLOT
+        /PROOF_COPY_PERMUTATION_GRAND_PRODUCT_OPENING_AT_Z_OMEGA_SLOT ; try by progress).
+rewrite /m12 /m11 /m10 /m9 /m8 /m7 /m6 /m5 /m4 /m3 /m2 /m1 /lagrange_memory_footprint /modexp_memory_footprint; progress.
+do 22! (rewrite load_store_diff;
+rewrite /STATE_Z_SLOT
+        /STATE_POWER_OF_ALPHA_8_SLOT
+        /STATE_POWER_OF_ALPHA_7_SLOT
+        /STATE_POWER_OF_ALPHA_6_SLOT
+        /STATE_POWER_OF_ALPHA_5_SLOT
+        /STATE_POWER_OF_ALPHA_4_SLOT
+        /STATE_POWER_OF_ALPHA_3_SLOT 
+        /STATE_POWER_OF_ALPHA_2_SLOT
+        /STATE_ALPHA_SLOT
+        /STATE_BETA_SLOT
+        /STATE_GAMMA_SLOT
+        /PROOF_PUBLIC_INPUT
+        /STATE_L_N_MINUS_ONE_AT_Z_SLOT
+        /STATE_L_0_AT_Z_SLOT
+        /PROOF_GATE_SELECTORS_0_OPENING_AT_Z_SLOT
+        /PROOF_STATE_POLYS_0_OPENING_AT_Z_SLOT
+        /PROOF_STATE_POLYS_1_OPENING_AT_Z_SLOT
+        /PROOF_STATE_POLYS_2_OPENING_AT_Z_SLOT
+        /PROOF_STATE_POLYS_3_OPENING_AT_Z_SLOT
+        /PROOF_COPY_PERMUTATION_POLYS_0_OPENING_AT_Z_SLOT
+        /PROOF_COPY_PERMUTATION_POLYS_1_OPENING_AT_Z_SLOT
+        /PROOF_COPY_PERMUTATION_POLYS_2_OPENING_AT_Z_SLOT
+        /PROOF_COPY_PERMUTATION_GRAND_PRODUCT_OPENING_AT_Z_OMEGA_SLOT ; try by progress).
+rewrite /m12 /m11 /m10 /m9 /m8 /m7 /m6 /m5 /m4 /m3 /m2 /m1 /lagrange_memory_footprint /modexp_memory_footprint; progress.
+do 22! (rewrite load_store_diff;
+rewrite /STATE_Z_SLOT
+        /STATE_POWER_OF_ALPHA_8_SLOT
+        /STATE_POWER_OF_ALPHA_7_SLOT
+        /STATE_POWER_OF_ALPHA_6_SLOT
+        /STATE_POWER_OF_ALPHA_5_SLOT
+        /STATE_POWER_OF_ALPHA_4_SLOT
+        /STATE_POWER_OF_ALPHA_3_SLOT 
+        /STATE_POWER_OF_ALPHA_2_SLOT
+        /STATE_ALPHA_SLOT
+        /STATE_BETA_SLOT
+        /STATE_GAMMA_SLOT
+        /PROOF_PUBLIC_INPUT
+        /STATE_L_N_MINUS_ONE_AT_Z_SLOT
+        /STATE_L_0_AT_Z_SLOT
+        /PROOF_GATE_SELECTORS_0_OPENING_AT_Z_SLOT
+        /PROOF_STATE_POLYS_0_OPENING_AT_Z_SLOT
+        /PROOF_STATE_POLYS_1_OPENING_AT_Z_SLOT
+        /PROOF_STATE_POLYS_2_OPENING_AT_Z_SLOT
+        /PROOF_STATE_POLYS_3_OPENING_AT_Z_SLOT
+        /PROOF_COPY_PERMUTATION_POLYS_0_OPENING_AT_Z_SLOT
+        /PROOF_COPY_PERMUTATION_POLYS_1_OPENING_AT_Z_SLOT
+        /PROOF_COPY_PERMUTATION_POLYS_2_OPENING_AT_Z_SLOT
+        /PROOF_COPY_PERMUTATION_GRAND_PRODUCT_OPENING_AT_Z_OMEGA_SLOT ; try by progress).
+rewrite /m12 /m11 /m10 /m9 /m8 /m7 /m6 /m5 /m4 /m3 /m2 /m1 /lagrange_memory_footprint /modexp_memory_footprint; progress.
+do 7! (rewrite load_store_diff;
+rewrite /STATE_Z_SLOT
+        /STATE_POWER_OF_ALPHA_8_SLOT
+        /STATE_POWER_OF_ALPHA_7_SLOT
+        /STATE_POWER_OF_ALPHA_6_SLOT
+        /STATE_POWER_OF_ALPHA_5_SLOT
+        /STATE_POWER_OF_ALPHA_4_SLOT
+        /STATE_POWER_OF_ALPHA_3_SLOT 
+        /STATE_POWER_OF_ALPHA_2_SLOT
+        /STATE_ALPHA_SLOT
+        /STATE_BETA_SLOT
+        /STATE_GAMMA_SLOT
+        /PROOF_PUBLIC_INPUT
+        /STATE_L_N_MINUS_ONE_AT_Z_SLOT
+        /STATE_L_0_AT_Z_SLOT
+        /PROOF_GATE_SELECTORS_0_OPENING_AT_Z_SLOT
+        /PROOF_STATE_POLYS_0_OPENING_AT_Z_SLOT
+        /PROOF_STATE_POLYS_1_OPENING_AT_Z_SLOT
+        /PROOF_STATE_POLYS_2_OPENING_AT_Z_SLOT
+        /PROOF_STATE_POLYS_3_OPENING_AT_Z_SLOT
+        /PROOF_COPY_PERMUTATION_POLYS_0_OPENING_AT_Z_SLOT
+        /PROOF_COPY_PERMUTATION_POLYS_1_OPENING_AT_Z_SLOT
+        /PROOF_COPY_PERMUTATION_POLYS_2_OPENING_AT_Z_SLOT
+        /PROOF_COPY_PERMUTATION_GRAND_PRODUCT_OPENING_AT_Z_OMEGA_SLOT ; try by progress).
+rewrite load_store_same; reflexivity.
+
+seq 1 1: (
+  (stateAlpha{2}, stateBeta{2}, stateBetaLookup{2}, stateGamma{2},
+         stateGammaLookup{2}, stateZ{2}, proofPublicInput{2},
+         proofCopyPermutationPolys0OpeningAtZ{2},
+         proofCopyPermutationPolys1OpeningAtZ{2},
+         proofCopyPermutationPolys2OpeningAtZ{2},
+         proofStatePolys0OpeningAtZ{2}, proofStatePolys1OpeningAtZ{2},
+         proofStatePolys2OpeningAtZ{2}, proofStatePolys3OpeningAtZ{2},
+         proofLookupSPolyOpeningAtZOmega{2},
+         proofLookupGrandProductOpeningAtZOmega{2},
+         proofGateSelectors0OpeningAtZ{2},
+         proofLinearisationPolyOpeningAtZ{2},
+         proofCopyPermutationGrandProductOpeningAtZOmega{2},
+         stateZInDomainSize{2}, proofQuotientPolyOpeningAtZ{2}) =
+        (stateAlphaG, stateBetaG, stateBetaLookupG, stateGammaG,
+         stateGammaLookupG, stateZG, proofPublicInputG,
+         proofCopyPermutationPolys0OpeningAtZG,
+         proofCopyPermutationPolys1OpeningAtZG,
+         proofCopyPermutationPolys2OpeningAtZG, proofStatePolys0OpeningAtZG,
+         proofStatePolys1OpeningAtZG, proofStatePolys2OpeningAtZG,
+         proofStatePolys3OpeningAtZG, proofLookupSPolyOpeningAtZOmegaG,
+         proofLookupGrandProductOpeningAtZOmegaG,
+         proofGateSelectors0OpeningAtZG, proofLinearisationPolyOpeningAtZG,
+         proofCopyPermutationGrandProductOpeningAtZOmegaG,
+         stateZInDomainSizeG, proofQuotientPolyOpeningAtZG) /\
+        to_uint (mload m STATE_ALPHA_SLOT) = stateAlphaG /\
+        to_uint (mload m STATE_BETA_SLOT) = stateBetaG /\
+        to_uint (mload m STATE_BETA_LOOKUP_SLOT) = stateBetaLookupG /\
+        to_uint (mload m STATE_GAMMA_SLOT) = stateGammaG /\
+        to_uint (mload m STATE_GAMMA_LOOKUP_SLOT) = stateGammaLookupG /\
+        to_uint (mload m STATE_Z_SLOT) = stateZG /\
+        to_uint (mload m PROOF_PUBLIC_INPUT) = proofPublicInputG /\
+        to_uint (mload m PROOF_COPY_PERMUTATION_POLYS_0_OPENING_AT_Z_SLOT) =
+        proofCopyPermutationPolys0OpeningAtZG /\
+        to_uint (mload m PROOF_COPY_PERMUTATION_POLYS_1_OPENING_AT_Z_SLOT) =
+        proofCopyPermutationPolys1OpeningAtZG /\
+        to_uint (mload m PROOF_COPY_PERMUTATION_POLYS_2_OPENING_AT_Z_SLOT) =
+        proofCopyPermutationPolys2OpeningAtZG /\
+        to_uint (mload m PROOF_STATE_POLYS_0_OPENING_AT_Z_SLOT) =
+        proofStatePolys0OpeningAtZG /\
+        to_uint (mload m PROOF_STATE_POLYS_1_OPENING_AT_Z_SLOT) =
+        proofStatePolys1OpeningAtZG /\
+        to_uint (mload m PROOF_STATE_POLYS_2_OPENING_AT_Z_SLOT) =
+        proofStatePolys2OpeningAtZG /\
+        to_uint (mload m PROOF_STATE_POLYS_3_OPENING_AT_Z_SLOT) =
+        proofStatePolys3OpeningAtZG /\
+        to_uint (mload m PROOF_LOOKUP_S_POLY_OPENING_AT_Z_OMEGA_SLOT) =
+        proofLookupSPolyOpeningAtZOmegaG /\
+        to_uint (mload m PROOF_LOOKUP_GRAND_PRODUCT_OPENING_AT_Z_OMEGA_SLOT) =
+        proofLookupGrandProductOpeningAtZOmegaG /\
+        to_uint (mload m PROOF_GATE_SELECTORS_0_OPENING_AT_Z_SLOT) =
+        proofGateSelectors0OpeningAtZG /\
+        to_uint (mload m PROOF_LINEARISATION_POLY_OPENING_AT_Z_SLOT) =
+        proofLinearisationPolyOpeningAtZG /\
+        to_uint
+          (mload m
+             PROOF_COPY_PERMUTATION_GRAND_PRODUCT_OPENING_AT_Z_OMEGA_SLOT) =
+        proofCopyPermutationGrandProductOpeningAtZOmegaG /\
+        to_uint (mload m STATE_Z_IN_DOMAIN_SIZE) = stateZInDomainSizeG /\
+        to_uint (mload m PROOF_QUOTIENT_POLY_OPENING_AT_Z_SLOT) =
+        proofQuotientPolyOpeningAtZG /\
+        a = stateAlpha{2} /\
+        a2 = statePowerOfAlpha2{2} /\
+        a3 = statePowerOfAlpha3{2} /\
+        a4 = statePowerOfAlpha4{2} /\
+        a5 = statePowerOfAlpha5{2} /\
+        a6 = statePowerOfAlpha6{2} /\
+        a7 = statePowerOfAlpha7{2} /\
+        a8 = statePowerOfAlpha8{2} /\
+        statePowerOfAlpha2{2} = stateAlpha{2} ^ 2 %% Constants.R /\
+        statePowerOfAlpha3{2} = stateAlpha{2} ^ 3 %% Constants.R /\
+        statePowerOfAlpha4{2} = stateAlpha{2} ^ 4 %% Constants.R /\
+        statePowerOfAlpha5{2} = stateAlpha{2} ^ 5 %% Constants.R /\
+        statePowerOfAlpha6{2} = stateAlpha{2} ^ 6 %% Constants.R /\
+        statePowerOfAlpha7{2} = stateAlpha{2} ^ 7 %% Constants.R /\
+        statePowerOfAlpha8{2} = stateAlpha{2} ^ 8 %% Constants.R /\
+        sl0az = _12{1} /\
+        to_uint _12{1} = stateL0AtZ{2} /\
+        slnm1az = _17{1} /\
+        to_uint _17{1} = stateLnMinusOneAtZ{2} /\
+        to_uint stateZ{1} = stateZ{2} /\
+        (stateZ{2} ^ Constants.DOMAIN_SIZE - 1) %% Constants.R <> 0 /\
+        elpodL0{2} = Some (to_uint _12{1}) /\
+        elpodLn{2} = Some (to_uint _17{1}) /\
+        (0 <= to_uint _12{1} && to_uint _12{1} < Constants.R) /\
+        (0 <= to_uint _17{1} && to_uint _17{1} < Constants.R) /\
+        !Primops.reverted{1} /\ Primops.memory{1} = m12 /\
+       to_uint _20{1} = proofPublicInput{2} /\
+      _21{1} = _12{1} /\
+     to_uint stateT{1} = stateT{2} /\
+     stateT{2} = stateL0AtZ{2} * proofPublicInput{2} %% Constants.R /\
+    to_uint _23{1} = proofGateSelectors0OpeningAtZ{2} /\
+   pgsT{2} = stateT{2} * proofGateSelectors0OpeningAtZ{2} %% Constants.R /\
+  to_uint _24{1} = pqc{2} /\ 0 <= pqc{2} && pqc{2} < Constants.R /\
+  to_uint result{1} = pqcR{2} /\ pqcR{2} = (pgsT{2} + pqc{2}) %% Constants.R).
+wp. skip. progress. rewrite /addmod. progress. 
+rewrite W256.to_uint_small. progress. by smt(@W256 @Utils). by smt(@W256 @Utils). rewrite /R_MOD. smt().
+
+seq 1 1:(
+  (stateAlpha{2}, stateBeta{2}, stateBetaLookup{2}, stateGamma{2},
+   stateGammaLookup{2}, stateZ{2}, proofPublicInput{2},
+   proofCopyPermutationPolys0OpeningAtZ{2},
+   proofCopyPermutationPolys1OpeningAtZ{2},
+   proofCopyPermutationPolys2OpeningAtZ{2}, proofStatePolys0OpeningAtZ{2},
+   proofStatePolys1OpeningAtZ{2}, proofStatePolys2OpeningAtZ{2},
+   proofStatePolys3OpeningAtZ{2}, proofLookupSPolyOpeningAtZOmega{2},
+   proofLookupGrandProductOpeningAtZOmega{2},
+   proofGateSelectors0OpeningAtZ{2}, proofLinearisationPolyOpeningAtZ{2},
+   proofCopyPermutationGrandProductOpeningAtZOmega{2}, stateZInDomainSize{2},
+   proofQuotientPolyOpeningAtZ{2}) =
+  (stateAlphaG, stateBetaG, stateBetaLookupG, stateGammaG, stateGammaLookupG,
+   stateZG, proofPublicInputG, proofCopyPermutationPolys0OpeningAtZG,
+   proofCopyPermutationPolys1OpeningAtZG,
+   proofCopyPermutationPolys2OpeningAtZG, proofStatePolys0OpeningAtZG,
+   proofStatePolys1OpeningAtZG, proofStatePolys2OpeningAtZG,
+   proofStatePolys3OpeningAtZG, proofLookupSPolyOpeningAtZOmegaG,
+   proofLookupGrandProductOpeningAtZOmegaG, proofGateSelectors0OpeningAtZG,
+   proofLinearisationPolyOpeningAtZG,
+   proofCopyPermutationGrandProductOpeningAtZOmegaG, stateZInDomainSizeG,
+   proofQuotientPolyOpeningAtZG) /\
+  to_uint (mload m STATE_ALPHA_SLOT) = stateAlphaG /\
+  to_uint (mload m STATE_BETA_SLOT) = stateBetaG /\
+  to_uint (mload m STATE_BETA_LOOKUP_SLOT) = stateBetaLookupG /\
+  to_uint (mload m STATE_GAMMA_SLOT) = stateGammaG /\
+  to_uint (mload m STATE_GAMMA_LOOKUP_SLOT) = stateGammaLookupG /\
+  to_uint (mload m STATE_Z_SLOT) = stateZG /\
+  to_uint (mload m PROOF_PUBLIC_INPUT) = proofPublicInputG /\
+  to_uint (mload m PROOF_COPY_PERMUTATION_POLYS_0_OPENING_AT_Z_SLOT) =
+  proofCopyPermutationPolys0OpeningAtZG /\
+  to_uint (mload m PROOF_COPY_PERMUTATION_POLYS_1_OPENING_AT_Z_SLOT) =
+  proofCopyPermutationPolys1OpeningAtZG /\
+  to_uint (mload m PROOF_COPY_PERMUTATION_POLYS_2_OPENING_AT_Z_SLOT) =
+  proofCopyPermutationPolys2OpeningAtZG /\
+  to_uint (mload m PROOF_STATE_POLYS_0_OPENING_AT_Z_SLOT) =
+  proofStatePolys0OpeningAtZG /\
+  to_uint (mload m PROOF_STATE_POLYS_1_OPENING_AT_Z_SLOT) =
+  proofStatePolys1OpeningAtZG /\
+  to_uint (mload m PROOF_STATE_POLYS_2_OPENING_AT_Z_SLOT) =
+  proofStatePolys2OpeningAtZG /\
+  to_uint (mload m PROOF_STATE_POLYS_3_OPENING_AT_Z_SLOT) =
+  proofStatePolys3OpeningAtZG /\
+  to_uint (mload m PROOF_LOOKUP_S_POLY_OPENING_AT_Z_OMEGA_SLOT) =
+  proofLookupSPolyOpeningAtZOmegaG /\
+  to_uint (mload m PROOF_LOOKUP_GRAND_PRODUCT_OPENING_AT_Z_OMEGA_SLOT) =
+  proofLookupGrandProductOpeningAtZOmegaG /\
+  to_uint (mload m PROOF_GATE_SELECTORS_0_OPENING_AT_Z_SLOT) =
+  proofGateSelectors0OpeningAtZG /\
+  to_uint (mload m PROOF_LINEARISATION_POLY_OPENING_AT_Z_SLOT) =
+  proofLinearisationPolyOpeningAtZG /\
+  to_uint
+    (mload m PROOF_COPY_PERMUTATION_GRAND_PRODUCT_OPENING_AT_Z_OMEGA_SLOT) =
+  proofCopyPermutationGrandProductOpeningAtZOmegaG /\
+  to_uint (mload m STATE_Z_IN_DOMAIN_SIZE) = stateZInDomainSizeG /\
+  to_uint (mload m PROOF_QUOTIENT_POLY_OPENING_AT_Z_SLOT) =
+  proofQuotientPolyOpeningAtZG /\
+  a = stateAlpha{2} /\
+  a2 = statePowerOfAlpha2{2} /\
+  a3 = statePowerOfAlpha3{2} /\
+  a4 = statePowerOfAlpha4{2} /\
+  a5 = statePowerOfAlpha5{2} /\
+  a6 = statePowerOfAlpha6{2} /\
+  a7 = statePowerOfAlpha7{2} /\
+  a8 = statePowerOfAlpha8{2} /\
+  statePowerOfAlpha2{2} = stateAlpha{2} ^ 2 %% Constants.R /\
+  statePowerOfAlpha3{2} = stateAlpha{2} ^ 3 %% Constants.R /\
+  statePowerOfAlpha4{2} = stateAlpha{2} ^ 4 %% Constants.R /\
+  statePowerOfAlpha5{2} = stateAlpha{2} ^ 5 %% Constants.R /\
+  statePowerOfAlpha6{2} = stateAlpha{2} ^ 6 %% Constants.R /\
+  statePowerOfAlpha7{2} = stateAlpha{2} ^ 7 %% Constants.R /\
+  statePowerOfAlpha8{2} = stateAlpha{2} ^ 8 %% Constants.R /\
+  sl0az = _12{1} /\
+  to_uint _12{1} = stateL0AtZ{2} /\
+  slnm1az = _17{1} /\
+  to_uint _17{1} = stateLnMinusOneAtZ{2} /\
+  to_uint stateZ{1} = stateZ{2} /\
+  (stateZ{2} ^ Constants.DOMAIN_SIZE - 1) %% Constants.R <> 0 /\
+  elpodL0{2} = Some (to_uint _12{1}) /\
+  elpodLn{2} = Some (to_uint _17{1}) /\
+  (0 <= to_uint _12{1} && to_uint _12{1} < Constants.R) /\
+  (0 <= to_uint _17{1} && to_uint _17{1} < Constants.R) /\
+  !Primops.reverted{1} /\
+  to_uint _20{1} = proofPublicInput{2} /\
+  _21{1} = _12{1} /\
+  to_uint stateT{1} = stateT{2} /\
+  stateT{2} = stateL0AtZ{2} * proofPublicInput{2} %% Constants.R /\
+  to_uint _23{1} = proofGateSelectors0OpeningAtZ{2} /\
+  pgsT{2} = stateT{2} * proofGateSelectors0OpeningAtZ{2} %% Constants.R /\
+  to_uint _24{1} = pqc{2} /\
+  0 <= pqc{2} &&
+  pqc{2} < Constants.R /\
+  to_uint result{1} = pqcR{2} /\ pqcR{2} = (pgsT{2} + pqc{2}) %% Constants.R /\
+  to_uint _25{1} = lqc{2} /\ 0 <= lqc{2} < Constants.R /\
+  0 <= stateBetaPlusOne{2} < Constants.R /\
+  0 <= stateBetaGammaPlusGamma{2} < Constants.R /\
+  0 <= stateZMinusLastOmega{2} < Constants.R /\
+  exists v7 v8, Primops.memory{1} = lookupQuotientContribution_memory_footprint m12 v7 (W256.of_int stateBetaPlusOne{2}) (W256.of_int stateBetaGammaPlusGamma{2}) (W256.of_int stateZMinusLastOmega{2}) v8
+).
+call (LookupQuotientContribution_low_equiv_mid m12
+        stateBetaLookupG stateGammaLookupG
+        a6 a7 a8
+        proofLookupSPolyOpeningAtZOmegaG
+        proofLookupGrandProductOpeningAtZOmegaG
+        stateZG
+        (W256.to_uint sl0az) (W256.to_uint slnm1az)).
+skip. progress.
+rewrite /m12 /m11 /m10 /m9 /m8 /m7 /m6 /m5 /m4 /m3 /m2 /m1 /lagrange_memory_footprint /modexp_memory_footprint; progress.
+do 22! (rewrite load_store_diff;
+rewrite /STATE_Z_SLOT
+        /STATE_POWER_OF_ALPHA_8_SLOT
+        /STATE_POWER_OF_ALPHA_7_SLOT
+        /STATE_POWER_OF_ALPHA_6_SLOT
+        /STATE_POWER_OF_ALPHA_5_SLOT
+        /STATE_POWER_OF_ALPHA_4_SLOT
+        /STATE_POWER_OF_ALPHA_3_SLOT 
+        /STATE_POWER_OF_ALPHA_2_SLOT
+        /STATE_ALPHA_SLOT
+        /STATE_BETA_SLOT
+        /STATE_GAMMA_SLOT
+        /STATE_BETA_LOOKUP_SLOT
+        /STATE_GAMMA_LOOKUP_SLOT
+        /PROOF_PUBLIC_INPUT
+        /STATE_L_N_MINUS_ONE_AT_Z_SLOT
+        /STATE_L_0_AT_Z_SLOT
+        /PROOF_GATE_SELECTORS_0_OPENING_AT_Z_SLOT
+        /PROOF_STATE_POLYS_0_OPENING_AT_Z_SLOT
+        /PROOF_STATE_POLYS_1_OPENING_AT_Z_SLOT
+        /PROOF_STATE_POLYS_2_OPENING_AT_Z_SLOT
+        /PROOF_STATE_POLYS_3_OPENING_AT_Z_SLOT
+        /PROOF_COPY_PERMUTATION_POLYS_0_OPENING_AT_Z_SLOT
+        /PROOF_COPY_PERMUTATION_POLYS_1_OPENING_AT_Z_SLOT
+        /PROOF_COPY_PERMUTATION_POLYS_2_OPENING_AT_Z_SLOT
+        /PROOF_COPY_PERMUTATION_GRAND_PRODUCT_OPENING_AT_Z_OMEGA_SLOT ; try by progress).
+rewrite /m12 /m11 /m10 /m9 /m8 /m7 /m6 /m5 /m4 /m3 /m2 /m1 /lagrange_memory_footprint /modexp_memory_footprint; progress.
+do 22! (rewrite load_store_diff;
+rewrite /STATE_Z_SLOT
+        /STATE_POWER_OF_ALPHA_8_SLOT
+        /STATE_POWER_OF_ALPHA_7_SLOT
+        /STATE_POWER_OF_ALPHA_6_SLOT
+        /STATE_POWER_OF_ALPHA_5_SLOT
+        /STATE_POWER_OF_ALPHA_4_SLOT
+        /STATE_POWER_OF_ALPHA_3_SLOT 
+        /STATE_POWER_OF_ALPHA_2_SLOT
+        /STATE_ALPHA_SLOT
+        /STATE_BETA_SLOT
+        /STATE_GAMMA_SLOT
+        /STATE_BETA_LOOKUP_SLOT
+        /STATE_GAMMA_LOOKUP_SLOT
+        /PROOF_PUBLIC_INPUT
+        /STATE_L_N_MINUS_ONE_AT_Z_SLOT
+        /STATE_L_0_AT_Z_SLOT
+        /PROOF_GATE_SELECTORS_0_OPENING_AT_Z_SLOT
+        /PROOF_STATE_POLYS_0_OPENING_AT_Z_SLOT
+        /PROOF_STATE_POLYS_1_OPENING_AT_Z_SLOT
+        /PROOF_STATE_POLYS_2_OPENING_AT_Z_SLOT
+        /PROOF_STATE_POLYS_3_OPENING_AT_Z_SLOT
+        /PROOF_COPY_PERMUTATION_POLYS_0_OPENING_AT_Z_SLOT
+        /PROOF_COPY_PERMUTATION_POLYS_1_OPENING_AT_Z_SLOT
+        /PROOF_COPY_PERMUTATION_POLYS_2_OPENING_AT_Z_SLOT
+        /PROOF_COPY_PERMUTATION_GRAND_PRODUCT_OPENING_AT_Z_OMEGA_SLOT ; try by progress).
+rewrite /m12 /m11 /m10 /m9 /m8 /m7 /m6 /m5 /m4 /m3 /m2 /m1 /lagrange_memory_footprint /modexp_memory_footprint; progress.
+do 16! (rewrite load_store_diff;
+rewrite /STATE_Z_SLOT
+        /STATE_POWER_OF_ALPHA_8_SLOT
+        /STATE_POWER_OF_ALPHA_7_SLOT
+        /STATE_POWER_OF_ALPHA_6_SLOT
+        /STATE_POWER_OF_ALPHA_5_SLOT
+        /STATE_POWER_OF_ALPHA_4_SLOT
+        /STATE_POWER_OF_ALPHA_3_SLOT 
+        /STATE_POWER_OF_ALPHA_2_SLOT
+        /STATE_ALPHA_SLOT
+        /STATE_BETA_SLOT
+        /STATE_GAMMA_SLOT
+        /STATE_BETA_LOOKUP_SLOT
+        /STATE_GAMMA_LOOKUP_SLOT
+        /PROOF_PUBLIC_INPUT
+        /STATE_L_N_MINUS_ONE_AT_Z_SLOT
+        /STATE_L_0_AT_Z_SLOT
+        /PROOF_GATE_SELECTORS_0_OPENING_AT_Z_SLOT
+        /PROOF_STATE_POLYS_0_OPENING_AT_Z_SLOT
+        /PROOF_STATE_POLYS_1_OPENING_AT_Z_SLOT
+        /PROOF_STATE_POLYS_2_OPENING_AT_Z_SLOT
+        /PROOF_STATE_POLYS_3_OPENING_AT_Z_SLOT
+        /PROOF_COPY_PERMUTATION_POLYS_0_OPENING_AT_Z_SLOT
+        /PROOF_COPY_PERMUTATION_POLYS_1_OPENING_AT_Z_SLOT
+        /PROOF_COPY_PERMUTATION_POLYS_2_OPENING_AT_Z_SLOT
+        /PROOF_COPY_PERMUTATION_GRAND_PRODUCT_OPENING_AT_Z_OMEGA_SLOT ; try by progress).
+rewrite load_store_same. smt(@W256 @Utils).
+rewrite /m12 /m11 /m10 /m9 /m8 /m7 /m6 /m5 /m4 /m3 /m2 /m1 /lagrange_memory_footprint /modexp_memory_footprint; progress.
+do 15! (rewrite load_store_diff;
+rewrite /STATE_Z_SLOT
+        /STATE_POWER_OF_ALPHA_8_SLOT
+        /STATE_POWER_OF_ALPHA_7_SLOT
+        /STATE_POWER_OF_ALPHA_6_SLOT
+        /STATE_POWER_OF_ALPHA_5_SLOT
+        /STATE_POWER_OF_ALPHA_4_SLOT
+        /STATE_POWER_OF_ALPHA_3_SLOT 
+        /STATE_POWER_OF_ALPHA_2_SLOT
+        /STATE_ALPHA_SLOT
+        /STATE_BETA_SLOT
+        /STATE_GAMMA_SLOT
+        /STATE_BETA_LOOKUP_SLOT
+        /STATE_GAMMA_LOOKUP_SLOT
+        /PROOF_PUBLIC_INPUT
+        /STATE_L_N_MINUS_ONE_AT_Z_SLOT
+        /STATE_L_0_AT_Z_SLOT
+        /PROOF_GATE_SELECTORS_0_OPENING_AT_Z_SLOT
+        /PROOF_STATE_POLYS_0_OPENING_AT_Z_SLOT
+        /PROOF_STATE_POLYS_1_OPENING_AT_Z_SLOT
+        /PROOF_STATE_POLYS_2_OPENING_AT_Z_SLOT
+        /PROOF_STATE_POLYS_3_OPENING_AT_Z_SLOT
+        /PROOF_COPY_PERMUTATION_POLYS_0_OPENING_AT_Z_SLOT
+        /PROOF_COPY_PERMUTATION_POLYS_1_OPENING_AT_Z_SLOT
+        /PROOF_COPY_PERMUTATION_POLYS_2_OPENING_AT_Z_SLOT
+        /PROOF_COPY_PERMUTATION_GRAND_PRODUCT_OPENING_AT_Z_OMEGA_SLOT ; try by progress).
+rewrite load_store_same. smt(@W256 @Utils).
+rewrite /m12 /m11 /m10 /m9 /m8 /m7 /m6 /m5 /m4 /m3 /m2 /m1 /lagrange_memory_footprint /modexp_memory_footprint; progress.
+do 14! (rewrite load_store_diff;
+rewrite /STATE_Z_SLOT
+        /STATE_POWER_OF_ALPHA_8_SLOT
+        /STATE_POWER_OF_ALPHA_7_SLOT
+        /STATE_POWER_OF_ALPHA_6_SLOT
+        /STATE_POWER_OF_ALPHA_5_SLOT
+        /STATE_POWER_OF_ALPHA_4_SLOT
+        /STATE_POWER_OF_ALPHA_3_SLOT 
+        /STATE_POWER_OF_ALPHA_2_SLOT
+        /STATE_ALPHA_SLOT
+        /STATE_BETA_SLOT
+        /STATE_GAMMA_SLOT
+        /STATE_BETA_LOOKUP_SLOT
+        /STATE_GAMMA_LOOKUP_SLOT
+        /PROOF_PUBLIC_INPUT
+        /STATE_L_N_MINUS_ONE_AT_Z_SLOT
+        /STATE_L_0_AT_Z_SLOT
+        /PROOF_GATE_SELECTORS_0_OPENING_AT_Z_SLOT
+        /PROOF_STATE_POLYS_0_OPENING_AT_Z_SLOT
+        /PROOF_STATE_POLYS_1_OPENING_AT_Z_SLOT
+        /PROOF_STATE_POLYS_2_OPENING_AT_Z_SLOT
+        /PROOF_STATE_POLYS_3_OPENING_AT_Z_SLOT
+        /PROOF_COPY_PERMUTATION_POLYS_0_OPENING_AT_Z_SLOT
+        /PROOF_COPY_PERMUTATION_POLYS_1_OPENING_AT_Z_SLOT
+        /PROOF_COPY_PERMUTATION_POLYS_2_OPENING_AT_Z_SLOT
+        /PROOF_COPY_PERMUTATION_GRAND_PRODUCT_OPENING_AT_Z_OMEGA_SLOT ; try by progress).
+rewrite load_store_same. smt(@W256 @Utils).
+
+rewrite /m12 /m11 /m10 /m9 /m8 /m7 /m6 /m5 /m4 /m3 /m2 /m1 /lagrange_memory_footprint /modexp_memory_footprint; progress.
+do 22! (rewrite load_store_diff;
+rewrite /STATE_Z_SLOT
+        /STATE_POWER_OF_ALPHA_8_SLOT
+        /STATE_POWER_OF_ALPHA_7_SLOT
+        /STATE_POWER_OF_ALPHA_6_SLOT
+        /STATE_POWER_OF_ALPHA_5_SLOT
+        /STATE_POWER_OF_ALPHA_4_SLOT
+        /STATE_POWER_OF_ALPHA_3_SLOT 
+        /STATE_POWER_OF_ALPHA_2_SLOT
+        /STATE_ALPHA_SLOT
+        /STATE_BETA_SLOT
+        /STATE_GAMMA_SLOT
+        /STATE_BETA_LOOKUP_SLOT
+        /STATE_GAMMA_LOOKUP_SLOT
+        /PROOF_PUBLIC_INPUT
+        /STATE_L_N_MINUS_ONE_AT_Z_SLOT
+        /STATE_L_0_AT_Z_SLOT
+        /PROOF_GATE_SELECTORS_0_OPENING_AT_Z_SLOT
+        /PROOF_LOOKUP_S_POLY_OPENING_AT_Z_OMEGA_SLOT
+        /PROOF_STATE_POLYS_0_OPENING_AT_Z_SLOT
+        /PROOF_STATE_POLYS_1_OPENING_AT_Z_SLOT
+        /PROOF_STATE_POLYS_2_OPENING_AT_Z_SLOT
+        /PROOF_STATE_POLYS_3_OPENING_AT_Z_SLOT
+        /PROOF_COPY_PERMUTATION_POLYS_0_OPENING_AT_Z_SLOT
+        /PROOF_COPY_PERMUTATION_POLYS_1_OPENING_AT_Z_SLOT
+        /PROOF_COPY_PERMUTATION_POLYS_2_OPENING_AT_Z_SLOT
+        /PROOF_COPY_PERMUTATION_GRAND_PRODUCT_OPENING_AT_Z_OMEGA_SLOT ; try by progress).
+
+rewrite /m12 /m11 /m10 /m9 /m8 /m7 /m6 /m5 /m4 /m3 /m2 /m1 /lagrange_memory_footprint /modexp_memory_footprint; progress.
+do 22! (rewrite load_store_diff;
+rewrite /STATE_Z_SLOT
+        /STATE_POWER_OF_ALPHA_8_SLOT
+        /STATE_POWER_OF_ALPHA_7_SLOT
+        /STATE_POWER_OF_ALPHA_6_SLOT
+        /STATE_POWER_OF_ALPHA_5_SLOT
+        /STATE_POWER_OF_ALPHA_4_SLOT
+        /STATE_POWER_OF_ALPHA_3_SLOT 
+        /STATE_POWER_OF_ALPHA_2_SLOT
+        /STATE_ALPHA_SLOT
+        /STATE_BETA_SLOT
+        /STATE_GAMMA_SLOT
+        /STATE_BETA_LOOKUP_SLOT
+        /STATE_GAMMA_LOOKUP_SLOT
+        /PROOF_PUBLIC_INPUT
+        /STATE_L_N_MINUS_ONE_AT_Z_SLOT
+        /STATE_L_0_AT_Z_SLOT
+        /PROOF_GATE_SELECTORS_0_OPENING_AT_Z_SLOT
+        /PROOF_LOOKUP_S_POLY_OPENING_AT_Z_OMEGA_SLOT
+        /PROOF_STATE_POLYS_0_OPENING_AT_Z_SLOT
+        /PROOF_STATE_POLYS_1_OPENING_AT_Z_SLOT
+        /PROOF_STATE_POLYS_2_OPENING_AT_Z_SLOT
+        /PROOF_STATE_POLYS_3_OPENING_AT_Z_SLOT
+        /PROOF_COPY_PERMUTATION_POLYS_0_OPENING_AT_Z_SLOT
+        /PROOF_COPY_PERMUTATION_POLYS_1_OPENING_AT_Z_SLOT
+        /PROOF_COPY_PERMUTATION_POLYS_2_OPENING_AT_Z_SLOT
+        /PROOF_COPY_PERMUTATION_GRAND_PRODUCT_OPENING_AT_Z_OMEGA_SLOT
+        /PROOF_LOOKUP_GRAND_PRODUCT_OPENING_AT_Z_OMEGA_SLOT ; try by progress).
+rewrite /m12 /m11 /m10 /m9 /m8 /m7 /m6 /m5 /m4 /m3 /m2 /m1 /lagrange_memory_footprint /modexp_memory_footprint; progress.
+do 22! (rewrite load_store_diff;
+rewrite /STATE_Z_SLOT
+        /STATE_POWER_OF_ALPHA_8_SLOT
+        /STATE_POWER_OF_ALPHA_7_SLOT
+        /STATE_POWER_OF_ALPHA_6_SLOT
+        /STATE_POWER_OF_ALPHA_5_SLOT
+        /STATE_POWER_OF_ALPHA_4_SLOT
+        /STATE_POWER_OF_ALPHA_3_SLOT 
+        /STATE_POWER_OF_ALPHA_2_SLOT
+        /STATE_ALPHA_SLOT
+        /STATE_BETA_SLOT
+        /STATE_GAMMA_SLOT
+        /STATE_BETA_LOOKUP_SLOT
+        /STATE_GAMMA_LOOKUP_SLOT
+        /PROOF_PUBLIC_INPUT
+        /STATE_L_N_MINUS_ONE_AT_Z_SLOT
+        /STATE_L_0_AT_Z_SLOT
+        /PROOF_GATE_SELECTORS_0_OPENING_AT_Z_SLOT
+        /PROOF_LOOKUP_S_POLY_OPENING_AT_Z_OMEGA_SLOT
+        /PROOF_STATE_POLYS_0_OPENING_AT_Z_SLOT
+        /PROOF_STATE_POLYS_1_OPENING_AT_Z_SLOT
+        /PROOF_STATE_POLYS_2_OPENING_AT_Z_SLOT
+        /PROOF_STATE_POLYS_3_OPENING_AT_Z_SLOT
+        /PROOF_COPY_PERMUTATION_POLYS_0_OPENING_AT_Z_SLOT
+        /PROOF_COPY_PERMUTATION_POLYS_1_OPENING_AT_Z_SLOT
+        /PROOF_COPY_PERMUTATION_POLYS_2_OPENING_AT_Z_SLOT
+        /PROOF_COPY_PERMUTATION_GRAND_PRODUCT_OPENING_AT_Z_OMEGA_SLOT
+        /PROOF_LOOKUP_GRAND_PRODUCT_OPENING_AT_Z_OMEGA_SLOT ; try by progress).
+rewrite /m12 /m11 /m10 /m9 /m8 /m7 /m6 /m5 /m4 /m3 /m2 /m1 /lagrange_memory_footprint /modexp_memory_footprint; progress.
+do 7! (rewrite load_store_diff;
+rewrite /STATE_Z_SLOT
+        /STATE_POWER_OF_ALPHA_8_SLOT
+        /STATE_POWER_OF_ALPHA_7_SLOT
+        /STATE_POWER_OF_ALPHA_6_SLOT
+        /STATE_POWER_OF_ALPHA_5_SLOT
+        /STATE_POWER_OF_ALPHA_4_SLOT
+        /STATE_POWER_OF_ALPHA_3_SLOT 
+        /STATE_POWER_OF_ALPHA_2_SLOT
+        /STATE_ALPHA_SLOT
+        /STATE_BETA_SLOT
+        /STATE_GAMMA_SLOT
+        /STATE_BETA_LOOKUP_SLOT
+        /STATE_GAMMA_LOOKUP_SLOT
+        /PROOF_PUBLIC_INPUT
+        /STATE_L_N_MINUS_ONE_AT_Z_SLOT
+        /STATE_L_0_AT_Z_SLOT
+        /PROOF_GATE_SELECTORS_0_OPENING_AT_Z_SLOT
+        /PROOF_LOOKUP_S_POLY_OPENING_AT_Z_OMEGA_SLOT
+        /PROOF_STATE_POLYS_0_OPENING_AT_Z_SLOT
+        /PROOF_STATE_POLYS_1_OPENING_AT_Z_SLOT
+        /PROOF_STATE_POLYS_2_OPENING_AT_Z_SLOT
+        /PROOF_STATE_POLYS_3_OPENING_AT_Z_SLOT
+        /PROOF_COPY_PERMUTATION_POLYS_0_OPENING_AT_Z_SLOT
+        /PROOF_COPY_PERMUTATION_POLYS_1_OPENING_AT_Z_SLOT
+        /PROOF_COPY_PERMUTATION_POLYS_2_OPENING_AT_Z_SLOT
+        /PROOF_COPY_PERMUTATION_GRAND_PRODUCT_OPENING_AT_Z_OMEGA_SLOT
+        /PROOF_LOOKUP_GRAND_PRODUCT_OPENING_AT_Z_OMEGA_SLOT ; try by progress).
+rewrite load_store_same. reflexivity.
+rewrite /m12 /m11 /m10 /m9 /m8 /m7 /m6 /m5 /m4 /m3 /m2 /m1 /lagrange_memory_footprint /modexp_memory_footprint; progress.
+rewrite load_store_same. reflexivity. smt().
+exists (of_int v10)%W256 (of_int v20)%W256. reflexivity.
+
+seq 0 0:(
+  exists (v7 v8 : uint256),
+    Primops.memory{1} =
+    lookupQuotientContribution_memory_footprint m12 v7 (W256.of_int stateBetaPlusOne{2})
+      (W256.of_int stateBetaGammaPlusGamma{2}) (W256.of_int stateZMinusLastOmega{2}) v8 /\        
+  (stateAlpha{2}, stateBeta{2}, stateBetaLookup{2}, stateGamma{2},
+   stateGammaLookup{2}, stateZ{2}, proofPublicInput{2},
+   proofCopyPermutationPolys0OpeningAtZ{2},
+   proofCopyPermutationPolys1OpeningAtZ{2},
+   proofCopyPermutationPolys2OpeningAtZ{2}, proofStatePolys0OpeningAtZ{2},
+   proofStatePolys1OpeningAtZ{2}, proofStatePolys2OpeningAtZ{2},
+   proofStatePolys3OpeningAtZ{2}, proofLookupSPolyOpeningAtZOmega{2},
+   proofLookupGrandProductOpeningAtZOmega{2},
+   proofGateSelectors0OpeningAtZ{2}, proofLinearisationPolyOpeningAtZ{2},
+   proofCopyPermutationGrandProductOpeningAtZOmega{2}, stateZInDomainSize{2},
+   proofQuotientPolyOpeningAtZ{2}) =
+  (stateAlphaG, stateBetaG, stateBetaLookupG, stateGammaG, stateGammaLookupG,
+   stateZG, proofPublicInputG, proofCopyPermutationPolys0OpeningAtZG,
+   proofCopyPermutationPolys1OpeningAtZG,
+   proofCopyPermutationPolys2OpeningAtZG, proofStatePolys0OpeningAtZG,
+   proofStatePolys1OpeningAtZG, proofStatePolys2OpeningAtZG,
+   proofStatePolys3OpeningAtZG, proofLookupSPolyOpeningAtZOmegaG,
+   proofLookupGrandProductOpeningAtZOmegaG, proofGateSelectors0OpeningAtZG,
+   proofLinearisationPolyOpeningAtZG,
+   proofCopyPermutationGrandProductOpeningAtZOmegaG, stateZInDomainSizeG,
+   proofQuotientPolyOpeningAtZG) /\
+  to_uint (mload m STATE_ALPHA_SLOT) = stateAlphaG /\
+  to_uint (mload m STATE_BETA_SLOT) = stateBetaG /\
+  to_uint (mload m STATE_BETA_LOOKUP_SLOT) = stateBetaLookupG /\
+  to_uint (mload m STATE_GAMMA_SLOT) = stateGammaG /\
+  to_uint (mload m STATE_GAMMA_LOOKUP_SLOT) = stateGammaLookupG /\
+  to_uint (mload m STATE_Z_SLOT) = stateZG /\
+  to_uint (mload m PROOF_PUBLIC_INPUT) = proofPublicInputG /\
+  to_uint (mload m PROOF_COPY_PERMUTATION_POLYS_0_OPENING_AT_Z_SLOT) =
+  proofCopyPermutationPolys0OpeningAtZG /\
+  to_uint (mload m PROOF_COPY_PERMUTATION_POLYS_1_OPENING_AT_Z_SLOT) =
+  proofCopyPermutationPolys1OpeningAtZG /\
+  to_uint (mload m PROOF_COPY_PERMUTATION_POLYS_2_OPENING_AT_Z_SLOT) =
+  proofCopyPermutationPolys2OpeningAtZG /\
+  to_uint (mload m PROOF_STATE_POLYS_0_OPENING_AT_Z_SLOT) =
+  proofStatePolys0OpeningAtZG /\
+  to_uint (mload m PROOF_STATE_POLYS_1_OPENING_AT_Z_SLOT) =
+  proofStatePolys1OpeningAtZG /\
+  to_uint (mload m PROOF_STATE_POLYS_2_OPENING_AT_Z_SLOT) =
+  proofStatePolys2OpeningAtZG /\
+  to_uint (mload m PROOF_STATE_POLYS_3_OPENING_AT_Z_SLOT) =
+  proofStatePolys3OpeningAtZG /\
+  to_uint (mload m PROOF_LOOKUP_S_POLY_OPENING_AT_Z_OMEGA_SLOT) =
+  proofLookupSPolyOpeningAtZOmegaG /\
+  to_uint (mload m PROOF_LOOKUP_GRAND_PRODUCT_OPENING_AT_Z_OMEGA_SLOT) =
+  proofLookupGrandProductOpeningAtZOmegaG /\
+  to_uint (mload m PROOF_GATE_SELECTORS_0_OPENING_AT_Z_SLOT) =
+  proofGateSelectors0OpeningAtZG /\
+  to_uint (mload m PROOF_LINEARISATION_POLY_OPENING_AT_Z_SLOT) =
+  proofLinearisationPolyOpeningAtZG /\
+  to_uint
+    (mload m PROOF_COPY_PERMUTATION_GRAND_PRODUCT_OPENING_AT_Z_OMEGA_SLOT) =
+  proofCopyPermutationGrandProductOpeningAtZOmegaG /\
+  to_uint (mload m STATE_Z_IN_DOMAIN_SIZE) = stateZInDomainSizeG /\
+  to_uint (mload m PROOF_QUOTIENT_POLY_OPENING_AT_Z_SLOT) =
+  proofQuotientPolyOpeningAtZG /\
+  a = stateAlpha{2} /\
+  a2 = statePowerOfAlpha2{2} /\
+  a3 = statePowerOfAlpha3{2} /\
+  a4 = statePowerOfAlpha4{2} /\
+  a5 = statePowerOfAlpha5{2} /\
+  a6 = statePowerOfAlpha6{2} /\
+  a7 = statePowerOfAlpha7{2} /\
+  a8 = statePowerOfAlpha8{2} /\
+  statePowerOfAlpha2{2} = stateAlpha{2} ^ 2 %% Constants.R /\
+  statePowerOfAlpha3{2} = stateAlpha{2} ^ 3 %% Constants.R /\
+  statePowerOfAlpha4{2} = stateAlpha{2} ^ 4 %% Constants.R /\
+  statePowerOfAlpha5{2} = stateAlpha{2} ^ 5 %% Constants.R /\
+  statePowerOfAlpha6{2} = stateAlpha{2} ^ 6 %% Constants.R /\
+  statePowerOfAlpha7{2} = stateAlpha{2} ^ 7 %% Constants.R /\
+  statePowerOfAlpha8{2} = stateAlpha{2} ^ 8 %% Constants.R /\
+  sl0az = _12{1} /\
+  to_uint _12{1} = stateL0AtZ{2} /\
+  slnm1az = _17{1} /\
+  to_uint _17{1} = stateLnMinusOneAtZ{2} /\
+  to_uint stateZ{1} = stateZ{2} /\
+  (stateZ{2} ^ Constants.DOMAIN_SIZE - 1) %% Constants.R <> 0 /\
+  elpodL0{2} = Some (to_uint _12{1}) /\
+  elpodLn{2} = Some (to_uint _17{1}) /\
+  (0 <= to_uint _12{1} && to_uint _12{1} < Constants.R) /\
+  (0 <= to_uint _17{1} && to_uint _17{1} < Constants.R) /\
+  !Primops.reverted{1} /\
+  to_uint _20{1} = proofPublicInput{2} /\
+  _21{1} = _12{1} /\
+  to_uint stateT{1} = stateT{2} /\
+  stateT{2} = stateL0AtZ{2} * proofPublicInput{2} %% Constants.R /\
+  to_uint _23{1} = proofGateSelectors0OpeningAtZ{2} /\
+  pgsT{2} = stateT{2} * proofGateSelectors0OpeningAtZ{2} %% Constants.R /\
+  to_uint _24{1} = pqc{2} /\
+  0 <= pqc{2} &&
+  pqc{2} < Constants.R /\
+  to_uint result{1} = pqcR{2} /\
+  pqcR{2} = (pgsT{2} + pqc{2}) %% Constants.R /\
+  to_uint _25{1} = lqc{2} /\
+  (0 <= lqc{2} && lqc{2} < Constants.R) /\
+  (0 <= stateBetaPlusOne{2} && stateBetaPlusOne{2} < Constants.R) /\
+  (0 <= stateBetaGammaPlusGamma{2} &&
+   stateBetaGammaPlusGamma{2} < Constants.R) /\
+  (0 <= stateZMinusLastOmega{2} && stateZMinusLastOmega{2} < Constants.R)
+).
+skip. progress. exists v7 v8. progress. elim*. progress.
+exists* stateBetaPlusOne{2}, stateBetaGammaPlusGamma{2}, stateZMinusLastOmega{2}.
+elim*=> sbpo sbgpg szmlo.
+pose m13 := lookupQuotientContribution_memory_footprint m12 v7 (W256.of_int sbpo) (W256.of_int sbgpg) (W256.of_int szmlo) v8.
+
+seq 0 0:(
+  (stateAlpha{2}, stateBeta{2}, stateBetaLookup{2}, stateGamma{2},
+   stateGammaLookup{2}, stateZ{2}, proofPublicInput{2},
+   proofCopyPermutationPolys0OpeningAtZ{2},
+   proofCopyPermutationPolys1OpeningAtZ{2},
+   proofCopyPermutationPolys2OpeningAtZ{2}, proofStatePolys0OpeningAtZ{2},
+   proofStatePolys1OpeningAtZ{2}, proofStatePolys2OpeningAtZ{2},
+   proofStatePolys3OpeningAtZ{2}, proofLookupSPolyOpeningAtZOmega{2},
+   proofLookupGrandProductOpeningAtZOmega{2},
+   proofGateSelectors0OpeningAtZ{2}, proofLinearisationPolyOpeningAtZ{2},
+   proofCopyPermutationGrandProductOpeningAtZOmega{2}, stateZInDomainSize{2},
+   proofQuotientPolyOpeningAtZ{2}) =
+  (stateAlphaG, stateBetaG, stateBetaLookupG, stateGammaG, stateGammaLookupG,
+   stateZG, proofPublicInputG, proofCopyPermutationPolys0OpeningAtZG,
+   proofCopyPermutationPolys1OpeningAtZG,
+   proofCopyPermutationPolys2OpeningAtZG, proofStatePolys0OpeningAtZG,
+   proofStatePolys1OpeningAtZG, proofStatePolys2OpeningAtZG,
+   proofStatePolys3OpeningAtZG, proofLookupSPolyOpeningAtZOmegaG,
+   proofLookupGrandProductOpeningAtZOmegaG, proofGateSelectors0OpeningAtZG,
+   proofLinearisationPolyOpeningAtZG,
+   proofCopyPermutationGrandProductOpeningAtZOmegaG, stateZInDomainSizeG,
+   proofQuotientPolyOpeningAtZG) /\
+  to_uint (mload m STATE_ALPHA_SLOT) = stateAlphaG /\
+  to_uint (mload m STATE_BETA_SLOT) = stateBetaG /\
+  to_uint (mload m STATE_BETA_LOOKUP_SLOT) = stateBetaLookupG /\
+  to_uint (mload m STATE_GAMMA_SLOT) = stateGammaG /\
+  to_uint (mload m STATE_GAMMA_LOOKUP_SLOT) = stateGammaLookupG /\
+  to_uint (mload m STATE_Z_SLOT) = stateZG /\
+  to_uint (mload m PROOF_PUBLIC_INPUT) = proofPublicInputG /\
+  to_uint (mload m PROOF_COPY_PERMUTATION_POLYS_0_OPENING_AT_Z_SLOT) =
+  proofCopyPermutationPolys0OpeningAtZG /\
+  to_uint (mload m PROOF_COPY_PERMUTATION_POLYS_1_OPENING_AT_Z_SLOT) =
+  proofCopyPermutationPolys1OpeningAtZG /\
+  to_uint (mload m PROOF_COPY_PERMUTATION_POLYS_2_OPENING_AT_Z_SLOT) =
+  proofCopyPermutationPolys2OpeningAtZG /\
+  to_uint (mload m PROOF_STATE_POLYS_0_OPENING_AT_Z_SLOT) =
+  proofStatePolys0OpeningAtZG /\
+  to_uint (mload m PROOF_STATE_POLYS_1_OPENING_AT_Z_SLOT) =
+  proofStatePolys1OpeningAtZG /\
+  to_uint (mload m PROOF_STATE_POLYS_2_OPENING_AT_Z_SLOT) =
+  proofStatePolys2OpeningAtZG /\
+  to_uint (mload m PROOF_STATE_POLYS_3_OPENING_AT_Z_SLOT) =
+  proofStatePolys3OpeningAtZG /\
+  to_uint (mload m PROOF_LOOKUP_S_POLY_OPENING_AT_Z_OMEGA_SLOT) =
+  proofLookupSPolyOpeningAtZOmegaG /\
+  to_uint (mload m PROOF_LOOKUP_GRAND_PRODUCT_OPENING_AT_Z_OMEGA_SLOT) =
+  proofLookupGrandProductOpeningAtZOmegaG /\
+  to_uint (mload m PROOF_GATE_SELECTORS_0_OPENING_AT_Z_SLOT) =
+  proofGateSelectors0OpeningAtZG /\
+  to_uint (mload m PROOF_LINEARISATION_POLY_OPENING_AT_Z_SLOT) =
+  proofLinearisationPolyOpeningAtZG /\
+  to_uint
+    (mload m PROOF_COPY_PERMUTATION_GRAND_PRODUCT_OPENING_AT_Z_OMEGA_SLOT) =
+  proofCopyPermutationGrandProductOpeningAtZOmegaG /\
+  to_uint (mload m STATE_Z_IN_DOMAIN_SIZE) = stateZInDomainSizeG /\
+  to_uint (mload m PROOF_QUOTIENT_POLY_OPENING_AT_Z_SLOT) =
+  proofQuotientPolyOpeningAtZG /\
+  a = stateAlpha{2} /\
+  a2 = statePowerOfAlpha2{2} /\
+  a3 = statePowerOfAlpha3{2} /\
+  a4 = statePowerOfAlpha4{2} /\
+  a5 = statePowerOfAlpha5{2} /\
+  a6 = statePowerOfAlpha6{2} /\
+  a7 = statePowerOfAlpha7{2} /\
+  a8 = statePowerOfAlpha8{2} /\
+  statePowerOfAlpha2{2} = stateAlpha{2} ^ 2 %% Constants.R /\
+  statePowerOfAlpha3{2} = stateAlpha{2} ^ 3 %% Constants.R /\
+  statePowerOfAlpha4{2} = stateAlpha{2} ^ 4 %% Constants.R /\
+  statePowerOfAlpha5{2} = stateAlpha{2} ^ 5 %% Constants.R /\
+  statePowerOfAlpha6{2} = stateAlpha{2} ^ 6 %% Constants.R /\
+  statePowerOfAlpha7{2} = stateAlpha{2} ^ 7 %% Constants.R /\
+  statePowerOfAlpha8{2} = stateAlpha{2} ^ 8 %% Constants.R /\
+  sbpo = stateBetaPlusOne{2} /\
+  sbgpg = stateBetaGammaPlusGamma{2} /\
+  szmlo = stateZMinusLastOmega{2} /\  
+  sl0az = _12{1} /\
+  to_uint _12{1} = stateL0AtZ{2} /\
+  slnm1az = _17{1} /\
+  to_uint _17{1} = stateLnMinusOneAtZ{2} /\
+  to_uint stateZ{1} = stateZ{2} /\
+  (stateZ{2} ^ Constants.DOMAIN_SIZE - 1) %% Constants.R <> 0 /\
+  elpodL0{2} = Some (to_uint _12{1}) /\
+  elpodLn{2} = Some (to_uint _17{1}) /\
+  (0 <= to_uint _12{1} && to_uint _12{1} < Constants.R) /\
+  (0 <= to_uint _17{1} && to_uint _17{1} < Constants.R) /\
+  !Primops.reverted{1} /\
+  to_uint _20{1} = proofPublicInput{2} /\
+  _21{1} = _12{1} /\
+  to_uint stateT{1} = stateT{2} /\
+  stateT{2} = stateL0AtZ{2} * proofPublicInput{2} %% Constants.R /\
+  to_uint _23{1} = proofGateSelectors0OpeningAtZ{2} /\
+  pgsT{2} = stateT{2} * proofGateSelectors0OpeningAtZ{2} %% Constants.R /\
+  to_uint _24{1} = pqc{2} /\
+  0 <= pqc{2} &&
+  pqc{2} < Constants.R /\
+  to_uint result{1} = pqcR{2} /\
+  pqcR{2} = (pgsT{2} + pqc{2}) %% Constants.R /\
+  to_uint _25{1} = lqc{2} /\
+  (0 <= lqc{2} && lqc{2} < Constants.R) /\
+  (0 <= stateBetaPlusOne{2} && stateBetaPlusOne{2} < Constants.R) /\
+  (0 <= stateBetaGammaPlusGamma{2} &&
+   stateBetaGammaPlusGamma{2} < Constants.R) /\
+  (0 <= stateZMinusLastOmega{2} && stateZMinusLastOmega{2} < Constants.R) /\
+  Primops.memory{1} = m13
+).
+skip. by progress. 
+
+seq 2 1:(
+  (stateAlpha{2}, stateBeta{2}, stateBetaLookup{2}, stateGamma{2},
+   stateGammaLookup{2}, stateZ{2}, proofPublicInput{2},
+   proofCopyPermutationPolys0OpeningAtZ{2},
+   proofCopyPermutationPolys1OpeningAtZ{2},
+   proofCopyPermutationPolys2OpeningAtZ{2}, proofStatePolys0OpeningAtZ{2},
+   proofStatePolys1OpeningAtZ{2}, proofStatePolys2OpeningAtZ{2},
+   proofStatePolys3OpeningAtZ{2}, proofLookupSPolyOpeningAtZOmega{2},
+   proofLookupGrandProductOpeningAtZOmega{2},
+   proofGateSelectors0OpeningAtZ{2}, proofLinearisationPolyOpeningAtZ{2},
+   proofCopyPermutationGrandProductOpeningAtZOmega{2}, stateZInDomainSize{2},
+   proofQuotientPolyOpeningAtZ{2}) =
+  (stateAlphaG, stateBetaG, stateBetaLookupG, stateGammaG, stateGammaLookupG,
+   stateZG, proofPublicInputG, proofCopyPermutationPolys0OpeningAtZG,
+   proofCopyPermutationPolys1OpeningAtZG,
+   proofCopyPermutationPolys2OpeningAtZG, proofStatePolys0OpeningAtZG,
+   proofStatePolys1OpeningAtZG, proofStatePolys2OpeningAtZG,
+   proofStatePolys3OpeningAtZG, proofLookupSPolyOpeningAtZOmegaG,
+   proofLookupGrandProductOpeningAtZOmegaG, proofGateSelectors0OpeningAtZG,
+   proofLinearisationPolyOpeningAtZG,
+   proofCopyPermutationGrandProductOpeningAtZOmegaG, stateZInDomainSizeG,
+   proofQuotientPolyOpeningAtZG) /\
+  to_uint (mload m STATE_ALPHA_SLOT) = stateAlphaG /\
+  to_uint (mload m STATE_BETA_SLOT) = stateBetaG /\
+  to_uint (mload m STATE_BETA_LOOKUP_SLOT) = stateBetaLookupG /\
+  to_uint (mload m STATE_GAMMA_SLOT) = stateGammaG /\
+  to_uint (mload m STATE_GAMMA_LOOKUP_SLOT) = stateGammaLookupG /\
+  to_uint (mload m STATE_Z_SLOT) = stateZG /\
+  to_uint (mload m PROOF_PUBLIC_INPUT) = proofPublicInputG /\
+  to_uint (mload m PROOF_COPY_PERMUTATION_POLYS_0_OPENING_AT_Z_SLOT) =
+  proofCopyPermutationPolys0OpeningAtZG /\
+  to_uint (mload m PROOF_COPY_PERMUTATION_POLYS_1_OPENING_AT_Z_SLOT) =
+  proofCopyPermutationPolys1OpeningAtZG /\
+  to_uint (mload m PROOF_COPY_PERMUTATION_POLYS_2_OPENING_AT_Z_SLOT) =
+  proofCopyPermutationPolys2OpeningAtZG /\
+  to_uint (mload m PROOF_STATE_POLYS_0_OPENING_AT_Z_SLOT) =
+  proofStatePolys0OpeningAtZG /\
+  to_uint (mload m PROOF_STATE_POLYS_1_OPENING_AT_Z_SLOT) =
+  proofStatePolys1OpeningAtZG /\
+  to_uint (mload m PROOF_STATE_POLYS_2_OPENING_AT_Z_SLOT) =
+  proofStatePolys2OpeningAtZG /\
+  to_uint (mload m PROOF_STATE_POLYS_3_OPENING_AT_Z_SLOT) =
+  proofStatePolys3OpeningAtZG /\
+  to_uint (mload m PROOF_LOOKUP_S_POLY_OPENING_AT_Z_OMEGA_SLOT) =
+  proofLookupSPolyOpeningAtZOmegaG /\
+  to_uint (mload m PROOF_LOOKUP_GRAND_PRODUCT_OPENING_AT_Z_OMEGA_SLOT) =
+  proofLookupGrandProductOpeningAtZOmegaG /\
+  to_uint (mload m PROOF_GATE_SELECTORS_0_OPENING_AT_Z_SLOT) =
+  proofGateSelectors0OpeningAtZG /\
+  to_uint (mload m PROOF_LINEARISATION_POLY_OPENING_AT_Z_SLOT) =
+  proofLinearisationPolyOpeningAtZG /\
+  to_uint
+    (mload m PROOF_COPY_PERMUTATION_GRAND_PRODUCT_OPENING_AT_Z_OMEGA_SLOT) =
+  proofCopyPermutationGrandProductOpeningAtZOmegaG /\
+  to_uint (mload m STATE_Z_IN_DOMAIN_SIZE) = stateZInDomainSizeG /\
+  to_uint (mload m PROOF_QUOTIENT_POLY_OPENING_AT_Z_SLOT) =
+  proofQuotientPolyOpeningAtZG /\
+  a = stateAlpha{2} /\
+  a2 = statePowerOfAlpha2{2} /\
+  a3 = statePowerOfAlpha3{2} /\
+  a4 = statePowerOfAlpha4{2} /\
+  a5 = statePowerOfAlpha5{2} /\
+  a6 = statePowerOfAlpha6{2} /\
+  a7 = statePowerOfAlpha7{2} /\
+  a8 = statePowerOfAlpha8{2} /\
+  statePowerOfAlpha2{2} = stateAlpha{2} ^ 2 %% Constants.R /\
+  statePowerOfAlpha3{2} = stateAlpha{2} ^ 3 %% Constants.R /\
+  statePowerOfAlpha4{2} = stateAlpha{2} ^ 4 %% Constants.R /\
+  statePowerOfAlpha5{2} = stateAlpha{2} ^ 5 %% Constants.R /\
+  statePowerOfAlpha6{2} = stateAlpha{2} ^ 6 %% Constants.R /\
+  statePowerOfAlpha7{2} = stateAlpha{2} ^ 7 %% Constants.R /\
+  statePowerOfAlpha8{2} = stateAlpha{2} ^ 8 %% Constants.R /\
+  sbpo = stateBetaPlusOne{2} /\
+  sbgpg = stateBetaGammaPlusGamma{2} /\
+  szmlo = stateZMinusLastOmega{2} /\
+  sl0az = _12{1} /\
+  to_uint _12{1} = stateL0AtZ{2} /\
+  slnm1az = _17{1} /\
+  to_uint _17{1} = stateLnMinusOneAtZ{2} /\
+  to_uint stateZ{1} = stateZ{2} /\
+  (stateZ{2} ^ Constants.DOMAIN_SIZE - 1) %% Constants.R <> 0 /\
+  elpodL0{2} = Some (to_uint _12{1}) /\
+  elpodLn{2} = Some (to_uint _17{1}) /\
+  (0 <= to_uint _12{1} && to_uint _12{1} < Constants.R) /\
+  (0 <= to_uint _17{1} && to_uint _17{1} < Constants.R) /\
+  !Primops.reverted{1} /\
+  to_uint _20{1} = proofPublicInput{2} /\
+  _21{1} = _12{1} /\
+  to_uint stateT{1} = stateT{2} /\
+  stateT{2} = stateL0AtZ{2} * proofPublicInput{2} %% Constants.R /\
+  to_uint _23{1} = proofGateSelectors0OpeningAtZ{2} /\
+  pgsT{2} = stateT{2} * proofGateSelectors0OpeningAtZ{2} %% Constants.R /\
+  to_uint _24{1} = pqc{2} /\
+  0 <= pqc{2} &&
+  pqc{2} < Constants.R /\
+  pqcR{2} = (pgsT{2} + pqc{2}) %% Constants.R /\
+  to_uint _25{1} = lqc{2} /\
+  (0 <= lqc{2} && lqc{2} < Constants.R) /\
+  (0 <= stateBetaPlusOne{2} && stateBetaPlusOne{2} < Constants.R) /\
+  (0 <= stateBetaGammaPlusGamma{2} &&
+   stateBetaGammaPlusGamma{2} < Constants.R) /\
+  (0 <= stateZMinusLastOmega{2} && stateZMinusLastOmega{2} < Constants.R) /\
+  Primops.memory{1} = m13 /\
+  to_uint result{1} = lqcR{2} /\ lqcR{2} = (pqcR{2} + lqc{2}) %% Constants.R /\
+  to_uint _27{1} = proofLinearisationPolyOpeningAtZ{2}
+).
+sp. 
+call{1} (ConcretePrimops.mload_pspec m13 PROOF_LINEARISATION_POLY_OPENING_AT_Z_SLOT).
+skip. progress. rewrite /addmod. progress. 
+rewrite W256.to_uint_small. progress. by smt(@W256 @Utils). by smt(@W256 @Utils). rewrite /R_MOD. smt().
+rewrite /m13 /m12 /m11 /m10 /m9 /m8 /m7 /m6 /m5 /m4 /m3 /m2 /m1 /lookupQuotientContribution_memory_footprint /lagrange_memory_footprint /modexp_memory_footprint; progress.
+do 36! (rewrite load_store_diff;
+rewrite /STATE_Z_SLOT
+        /STATE_POWER_OF_ALPHA_8_SLOT
+        /STATE_POWER_OF_ALPHA_7_SLOT
+        /STATE_POWER_OF_ALPHA_6_SLOT
+        /STATE_POWER_OF_ALPHA_5_SLOT
+        /STATE_POWER_OF_ALPHA_4_SLOT
+        /STATE_POWER_OF_ALPHA_3_SLOT 
+        /STATE_POWER_OF_ALPHA_2_SLOT
+        /STATE_ALPHA_SLOT
+        /STATE_BETA_SLOT
+        /STATE_GAMMA_SLOT
+        /STATE_BETA_LOOKUP_SLOT
+        /STATE_GAMMA_LOOKUP_SLOT
+        /PROOF_PUBLIC_INPUT
+        /STATE_L_N_MINUS_ONE_AT_Z_SLOT
+        /STATE_L_0_AT_Z_SLOT
+        /PROOF_GATE_SELECTORS_0_OPENING_AT_Z_SLOT
+        /PROOF_LOOKUP_S_POLY_OPENING_AT_Z_OMEGA_SLOT
+        /PROOF_STATE_POLYS_0_OPENING_AT_Z_SLOT
+        /PROOF_STATE_POLYS_1_OPENING_AT_Z_SLOT
+        /PROOF_STATE_POLYS_2_OPENING_AT_Z_SLOT
+        /PROOF_STATE_POLYS_3_OPENING_AT_Z_SLOT
+        /PROOF_COPY_PERMUTATION_POLYS_0_OPENING_AT_Z_SLOT
+        /PROOF_COPY_PERMUTATION_POLYS_1_OPENING_AT_Z_SLOT
+        /PROOF_COPY_PERMUTATION_POLYS_2_OPENING_AT_Z_SLOT
+        /PROOF_COPY_PERMUTATION_GRAND_PRODUCT_OPENING_AT_Z_OMEGA_SLOT
+        /PROOF_LOOKUP_GRAND_PRODUCT_OPENING_AT_Z_OMEGA_SLOT
+        /PROOF_LINEARISATION_POLY_OPENING_AT_Z_SLOT
+        /STATE_Z_MINUS_LAST_OMEGA_SLOT
+        /STATE_BETA_PLUS_ONE_SLOT
+        /STATE_BETA_GAMMA_PLUS_GAMMA_SLOT ; try by progress).
+
+seq 3 1:(
+  (stateAlpha{2}, stateBeta{2}, stateBetaLookup{2}, stateGamma{2},
+   stateGammaLookup{2}, stateZ{2}, proofPublicInput{2},
+   proofCopyPermutationPolys0OpeningAtZ{2},
+   proofCopyPermutationPolys1OpeningAtZ{2},
+   proofCopyPermutationPolys2OpeningAtZ{2}, proofStatePolys0OpeningAtZ{2},
+   proofStatePolys1OpeningAtZ{2}, proofStatePolys2OpeningAtZ{2},
+   proofStatePolys3OpeningAtZ{2}, proofLookupSPolyOpeningAtZOmega{2},
+   proofLookupGrandProductOpeningAtZOmega{2},
+   proofGateSelectors0OpeningAtZ{2}, proofLinearisationPolyOpeningAtZ{2},
+   proofCopyPermutationGrandProductOpeningAtZOmega{2}, stateZInDomainSize{2},
+   proofQuotientPolyOpeningAtZ{2}) =
+  (stateAlphaG, stateBetaG, stateBetaLookupG, stateGammaG, stateGammaLookupG,
+   stateZG, proofPublicInputG, proofCopyPermutationPolys0OpeningAtZG,
+   proofCopyPermutationPolys1OpeningAtZG,
+   proofCopyPermutationPolys2OpeningAtZG, proofStatePolys0OpeningAtZG,
+   proofStatePolys1OpeningAtZG, proofStatePolys2OpeningAtZG,
+   proofStatePolys3OpeningAtZG, proofLookupSPolyOpeningAtZOmegaG,
+   proofLookupGrandProductOpeningAtZOmegaG, proofGateSelectors0OpeningAtZG,
+   proofLinearisationPolyOpeningAtZG,
+   proofCopyPermutationGrandProductOpeningAtZOmegaG, stateZInDomainSizeG,
+   proofQuotientPolyOpeningAtZG) /\
+  to_uint (mload m STATE_ALPHA_SLOT) = stateAlphaG /\
+  to_uint (mload m STATE_BETA_SLOT) = stateBetaG /\
+  to_uint (mload m STATE_BETA_LOOKUP_SLOT) = stateBetaLookupG /\
+  to_uint (mload m STATE_GAMMA_SLOT) = stateGammaG /\
+  to_uint (mload m STATE_GAMMA_LOOKUP_SLOT) = stateGammaLookupG /\
+  to_uint (mload m STATE_Z_SLOT) = stateZG /\
+  to_uint (mload m PROOF_PUBLIC_INPUT) = proofPublicInputG /\
+  to_uint (mload m PROOF_COPY_PERMUTATION_POLYS_0_OPENING_AT_Z_SLOT) =
+  proofCopyPermutationPolys0OpeningAtZG /\
+  to_uint (mload m PROOF_COPY_PERMUTATION_POLYS_1_OPENING_AT_Z_SLOT) =
+  proofCopyPermutationPolys1OpeningAtZG /\
+  to_uint (mload m PROOF_COPY_PERMUTATION_POLYS_2_OPENING_AT_Z_SLOT) =
+  proofCopyPermutationPolys2OpeningAtZG /\
+  to_uint (mload m PROOF_STATE_POLYS_0_OPENING_AT_Z_SLOT) =
+  proofStatePolys0OpeningAtZG /\
+  to_uint (mload m PROOF_STATE_POLYS_1_OPENING_AT_Z_SLOT) =
+  proofStatePolys1OpeningAtZG /\
+  to_uint (mload m PROOF_STATE_POLYS_2_OPENING_AT_Z_SLOT) =
+  proofStatePolys2OpeningAtZG /\
+  to_uint (mload m PROOF_STATE_POLYS_3_OPENING_AT_Z_SLOT) =
+  proofStatePolys3OpeningAtZG /\
+  to_uint (mload m PROOF_LOOKUP_S_POLY_OPENING_AT_Z_OMEGA_SLOT) =
+  proofLookupSPolyOpeningAtZOmegaG /\
+  to_uint (mload m PROOF_LOOKUP_GRAND_PRODUCT_OPENING_AT_Z_OMEGA_SLOT) =
+  proofLookupGrandProductOpeningAtZOmegaG /\
+  to_uint (mload m PROOF_GATE_SELECTORS_0_OPENING_AT_Z_SLOT) =
+  proofGateSelectors0OpeningAtZG /\
+  to_uint (mload m PROOF_LINEARISATION_POLY_OPENING_AT_Z_SLOT) =
+  proofLinearisationPolyOpeningAtZG /\
+  to_uint
+    (mload m PROOF_COPY_PERMUTATION_GRAND_PRODUCT_OPENING_AT_Z_OMEGA_SLOT) =
+  proofCopyPermutationGrandProductOpeningAtZOmegaG /\
+  to_uint (mload m STATE_Z_IN_DOMAIN_SIZE) = stateZInDomainSizeG /\
+  to_uint (mload m PROOF_QUOTIENT_POLY_OPENING_AT_Z_SLOT) =
+  proofQuotientPolyOpeningAtZG /\
+  a = stateAlpha{2} /\
+  a2 = statePowerOfAlpha2{2} /\
+  a3 = statePowerOfAlpha3{2} /\
+  a4 = statePowerOfAlpha4{2} /\
+  a5 = statePowerOfAlpha5{2} /\
+  a6 = statePowerOfAlpha6{2} /\
+  a7 = statePowerOfAlpha7{2} /\
+  a8 = statePowerOfAlpha8{2} /\
+  statePowerOfAlpha2{2} = stateAlpha{2} ^ 2 %% Constants.R /\
+  statePowerOfAlpha3{2} = stateAlpha{2} ^ 3 %% Constants.R /\
+  statePowerOfAlpha4{2} = stateAlpha{2} ^ 4 %% Constants.R /\
+  statePowerOfAlpha5{2} = stateAlpha{2} ^ 5 %% Constants.R /\
+  statePowerOfAlpha6{2} = stateAlpha{2} ^ 6 %% Constants.R /\
+  statePowerOfAlpha7{2} = stateAlpha{2} ^ 7 %% Constants.R /\
+  statePowerOfAlpha8{2} = stateAlpha{2} ^ 8 %% Constants.R /\
+  sbpo = stateBetaPlusOne{2} /\
+  sbgpg = stateBetaGammaPlusGamma{2} /\
+  szmlo = stateZMinusLastOmega{2} /\
+  sl0az = _12{1} /\
+  to_uint _12{1} = stateL0AtZ{2} /\
+  slnm1az = _17{1} /\
+  to_uint _17{1} = stateLnMinusOneAtZ{2} /\
+  to_uint stateZ{1} = stateZ{2} /\
+  (stateZ{2} ^ Constants.DOMAIN_SIZE - 1) %% Constants.R <> 0 /\
+  elpodL0{2} = Some (to_uint _12{1}) /\
+  elpodLn{2} = Some (to_uint _17{1}) /\
+  (0 <= to_uint _12{1} && to_uint _12{1} < Constants.R) /\
+  (0 <= to_uint _17{1} && to_uint _17{1} < Constants.R) /\
+  !Primops.reverted{1} /\
+  to_uint _20{1} = proofPublicInput{2} /\
+  _21{1} = _12{1} /\
+  to_uint stateT{1} = stateT{2} /\
+  stateT{2} = stateL0AtZ{2} * proofPublicInput{2} %% Constants.R /\
+  to_uint _23{1} = proofGateSelectors0OpeningAtZ{2} /\
+  pgsT{2} = stateT{2} * proofGateSelectors0OpeningAtZ{2} %% Constants.R /\
+  to_uint _24{1} = pqc{2} /\
+  0 <= pqc{2} &&
+  pqc{2} < Constants.R /\
+  pqcR{2} = (pgsT{2} + pqc{2}) %% Constants.R /\
+  to_uint _25{1} = lqc{2} /\
+  (0 <= lqc{2} && lqc{2} < Constants.R) /\
+  (0 <= stateBetaPlusOne{2} && stateBetaPlusOne{2} < Constants.R) /\
+  (0 <= stateBetaGammaPlusGamma{2} &&
+   stateBetaGammaPlusGamma{2} < Constants.R) /\
+  (0 <= stateZMinusLastOmega{2} && stateZMinusLastOmega{2} < Constants.R) /\
+  Primops.memory{1} = m13 /\
+  lqcR{2} = (pqcR{2} + lqc{2}) %% Constants.R /\
+  to_uint _27{1} = proofLinearisationPolyOpeningAtZ{2} /\
+  to_uint result{1} = plpo{2} /\ plpo{2} = (proofLinearisationPolyOpeningAtZ{2} + lqcR{2}) %% Constants.R /\
+  to_uint _28{1} = (Constants.R - 1) /\
+  to_uint _30{1} = stateZInDomainSize{2}
+).
+sp.
+call{1} (ConcretePrimops.mload_pspec m13 STATE_Z_IN_DOMAIN_SIZE).
+skip. progress. rewrite /addmod. progress. 
+rewrite W256.to_uint_small. progress. by smt(@W256 @Utils). by smt(@W256 @Utils). rewrite /R_MOD. smt().
+rewrite /R_MOD. smt().
+rewrite /m13 /m12 /m11 /m10 /m9 /m8 /m7 /m6 /m5 /m4 /m3 /m2 /m1 /lookupQuotientContribution_memory_footprint /lagrange_memory_footprint /modexp_memory_footprint; progress.
+do 36! (rewrite load_store_diff;
+rewrite /STATE_Z_SLOT
+        /STATE_POWER_OF_ALPHA_8_SLOT
+        /STATE_POWER_OF_ALPHA_7_SLOT
+        /STATE_POWER_OF_ALPHA_6_SLOT
+        /STATE_POWER_OF_ALPHA_5_SLOT
+        /STATE_POWER_OF_ALPHA_4_SLOT
+        /STATE_POWER_OF_ALPHA_3_SLOT 
+        /STATE_POWER_OF_ALPHA_2_SLOT
+        /STATE_ALPHA_SLOT
+        /STATE_BETA_SLOT
+        /STATE_GAMMA_SLOT
+        /STATE_BETA_LOOKUP_SLOT
+        /STATE_GAMMA_LOOKUP_SLOT
+        /PROOF_PUBLIC_INPUT
+        /STATE_L_N_MINUS_ONE_AT_Z_SLOT
+        /STATE_L_0_AT_Z_SLOT
+        /PROOF_GATE_SELECTORS_0_OPENING_AT_Z_SLOT
+        /PROOF_LOOKUP_S_POLY_OPENING_AT_Z_OMEGA_SLOT
+        /PROOF_STATE_POLYS_0_OPENING_AT_Z_SLOT
+        /PROOF_STATE_POLYS_1_OPENING_AT_Z_SLOT
+        /PROOF_STATE_POLYS_2_OPENING_AT_Z_SLOT
+        /PROOF_STATE_POLYS_3_OPENING_AT_Z_SLOT
+        /PROOF_COPY_PERMUTATION_POLYS_0_OPENING_AT_Z_SLOT
+        /PROOF_COPY_PERMUTATION_POLYS_1_OPENING_AT_Z_SLOT
+        /PROOF_COPY_PERMUTATION_POLYS_2_OPENING_AT_Z_SLOT
+        /PROOF_COPY_PERMUTATION_GRAND_PRODUCT_OPENING_AT_Z_OMEGA_SLOT
+        /PROOF_LOOKUP_GRAND_PRODUCT_OPENING_AT_Z_OMEGA_SLOT
+        /PROOF_LINEARISATION_POLY_OPENING_AT_Z_SLOT
+        /STATE_Z_MINUS_LAST_OMEGA_SLOT
+        /STATE_BETA_PLUS_ONE_SLOT
+        /STATE_BETA_GAMMA_PLUS_GAMMA_SLOT
+        /STATE_Z_IN_DOMAIN_SIZE ; try by progress).
+
+seq 1 1:(#pre /\
+  to_uint vanishing{1} = vanishing{2} /\
+  vanishing{2} = (stateZInDomainSize{2} + (Constants.R - 1)) %% Constants.R).
+wp. skip. progress. rewrite /addmod -H22. progress.
+rewrite W256.to_uint_small. progress. by smt(@W256 @Utils). by smt(@W256 @Utils). rewrite /R_MOD. smt().
+
+seq 2 1: (#pre /\
+  to_uint _32{1} = proofQuotientPolyOpeningAtZ{2} /\
+  to_uint lhs{1} = lhs{2} /\
+  lhs{2} = (proofQuotientPolyOpeningAtZ{2} * vanishing{2}) %% Constants.R).
+wp. 
+call{1} (ConcretePrimops.mload_pspec m13 PROOF_QUOTIENT_POLY_OPENING_AT_Z_SLOT).
+skip. progress.       
+rewrite /m13 /m12 /m11 /m10 /m9 /m8 /m7 /m6 /m5 /m4 /m3 /m2 /m1 /lookupQuotientContribution_memory_footprint /lagrange_memory_footprint /modexp_memory_footprint; progress.
+do 36! (rewrite load_store_diff;
+rewrite /STATE_Z_SLOT
+        /STATE_POWER_OF_ALPHA_8_SLOT
+        /STATE_POWER_OF_ALPHA_7_SLOT
+        /STATE_POWER_OF_ALPHA_6_SLOT
+        /STATE_POWER_OF_ALPHA_5_SLOT
+        /STATE_POWER_OF_ALPHA_4_SLOT
+        /STATE_POWER_OF_ALPHA_3_SLOT 
+        /STATE_POWER_OF_ALPHA_2_SLOT
+        /STATE_ALPHA_SLOT
+        /STATE_BETA_SLOT
+        /STATE_GAMMA_SLOT
+        /STATE_BETA_LOOKUP_SLOT
+        /STATE_GAMMA_LOOKUP_SLOT
+        /PROOF_PUBLIC_INPUT
+        /STATE_L_N_MINUS_ONE_AT_Z_SLOT
+        /STATE_L_0_AT_Z_SLOT
+        /PROOF_GATE_SELECTORS_0_OPENING_AT_Z_SLOT
+        /PROOF_LOOKUP_S_POLY_OPENING_AT_Z_OMEGA_SLOT
+        /PROOF_STATE_POLYS_0_OPENING_AT_Z_SLOT
+        /PROOF_STATE_POLYS_1_OPENING_AT_Z_SLOT
+        /PROOF_STATE_POLYS_2_OPENING_AT_Z_SLOT
+        /PROOF_STATE_POLYS_3_OPENING_AT_Z_SLOT
+        /PROOF_COPY_PERMUTATION_POLYS_0_OPENING_AT_Z_SLOT
+        /PROOF_COPY_PERMUTATION_POLYS_1_OPENING_AT_Z_SLOT
+        /PROOF_COPY_PERMUTATION_POLYS_2_OPENING_AT_Z_SLOT
+        /PROOF_COPY_PERMUTATION_GRAND_PRODUCT_OPENING_AT_Z_OMEGA_SLOT
+        /PROOF_LOOKUP_GRAND_PRODUCT_OPENING_AT_Z_OMEGA_SLOT
+        /PROOF_LINEARISATION_POLY_OPENING_AT_Z_SLOT
+        /STATE_Z_MINUS_LAST_OMEGA_SLOT
+        /STATE_BETA_PLUS_ONE_SLOT
+        /STATE_BETA_GAMMA_PLUS_GAMMA_SLOT
+        /STATE_Z_IN_DOMAIN_SIZE
+        /PROOF_QUOTIENT_POLY_OPENING_AT_Z_SLOT ; try by progress).
+rewrite /m13 /m12 /m11 /m10 /m9 /m8 /m7 /m6 /m5 /m4 /m3 /m2 /m1 /lookupQuotientContribution_memory_footprint /lagrange_memory_footprint /modexp_memory_footprint; progress.
+do 36! (rewrite load_store_diff;
+rewrite /STATE_Z_SLOT
+        /STATE_POWER_OF_ALPHA_8_SLOT
+        /STATE_POWER_OF_ALPHA_7_SLOT
+        /STATE_POWER_OF_ALPHA_6_SLOT
+        /STATE_POWER_OF_ALPHA_5_SLOT
+        /STATE_POWER_OF_ALPHA_4_SLOT
+        /STATE_POWER_OF_ALPHA_3_SLOT 
+        /STATE_POWER_OF_ALPHA_2_SLOT
+        /STATE_ALPHA_SLOT
+        /STATE_BETA_SLOT
+        /STATE_GAMMA_SLOT
+        /STATE_BETA_LOOKUP_SLOT
+        /STATE_GAMMA_LOOKUP_SLOT
+        /PROOF_PUBLIC_INPUT
+        /STATE_L_N_MINUS_ONE_AT_Z_SLOT
+        /STATE_L_0_AT_Z_SLOT
+        /PROOF_GATE_SELECTORS_0_OPENING_AT_Z_SLOT
+        /PROOF_LOOKUP_S_POLY_OPENING_AT_Z_OMEGA_SLOT
+        /PROOF_STATE_POLYS_0_OPENING_AT_Z_SLOT
+        /PROOF_STATE_POLYS_1_OPENING_AT_Z_SLOT
+        /PROOF_STATE_POLYS_2_OPENING_AT_Z_SLOT
+        /PROOF_STATE_POLYS_3_OPENING_AT_Z_SLOT
+        /PROOF_COPY_PERMUTATION_POLYS_0_OPENING_AT_Z_SLOT
+        /PROOF_COPY_PERMUTATION_POLYS_1_OPENING_AT_Z_SLOT
+        /PROOF_COPY_PERMUTATION_POLYS_2_OPENING_AT_Z_SLOT
+        /PROOF_COPY_PERMUTATION_GRAND_PRODUCT_OPENING_AT_Z_OMEGA_SLOT
+        /PROOF_LOOKUP_GRAND_PRODUCT_OPENING_AT_Z_OMEGA_SLOT
+        /PROOF_LINEARISATION_POLY_OPENING_AT_Z_SLOT
+        /STATE_Z_MINUS_LAST_OMEGA_SLOT
+        /STATE_BETA_PLUS_ONE_SLOT
+        /STATE_BETA_GAMMA_PLUS_GAMMA_SLOT
+        /STATE_Z_IN_DOMAIN_SIZE
+        /PROOF_QUOTIENT_POLY_OPENING_AT_Z_SLOT ; try by progress).
+rewrite /mulmod. progress.
+rewrite W256.to_uint_small. progress. by smt(@W256 @Utils). by smt(@W256 @Utils).
+rewrite /R_MOD. smt().
+
+case (bool_of_uint256 (iszero (eq_uint256 lhs{1} result{1}))).
+rcondt{1} 1. by progress.
+seq 0 0: (
+(stateZG ^ Constants.DOMAIN_SIZE - 1) %% Constants.R <> 0 /\ bool_of_uint256 (iszero (eq_uint256 lhs{1} result{1})) /\ to_uint lhs{1} = lhs{2} /\ to_uint result{1} = plpo{2}).
+skip. progress. wp.
+call{1} (revertWithMessage_low_pspec).
+skip. progress. left. progress.
+rewrite /eq_uint256 /iszero /bool_of_uint256 in H0. smt(@W256).
+
+rcondf{1} 1. by progress.
+wp. skip. progress. right. progress.
+exists v1 v2 v3 v4 v5 v6 v7 v8. progress.
+rewrite /eq_uint256 /iszero /bool_of_uint256 in H26. smt(@W256).
+smt(). smt(). smt(). smt(). smt(). smt(). smt(). smt(). smt(). smt(). smt(). smt(). smt(). smt().
+qed.
